@prefix : <https://w3id.org/pmd/co/2.0.7#> .
@prefix owl: <http://www.w3.org/2002/07/owl#> .
@prefix rdf: <http://www.w3.org/1999/02/22-rdf-syntax-ns#> .
@prefix xml: <http://www.w3.org/XML/1998/namespace> .
@prefix xsd: <http://www.w3.org/2001/XMLSchema#> .
@prefix rdfs: <http://www.w3.org/2000/01/rdf-schema#> .
@base <https://w3id.org/pmd/co/2.0.7#> .

<https://w3id.org/pmd/co/2.0.7> rdf:type owl:Ontology ;
                                 owl:versionIRI <https://w3id.org/pmd/mo/1.1> ;
                                 owl:imports <https://w3id.org/pmd/co/> ;
                                 <http://purl.org/dc/elements/1.1/creator> <https://orcid.org/0000-0002-3717-7104> ,
                                                                           <https://orcid.org/0000-0002-7094-5371> ;
                                 <http://purl.org/dc/elements/1.1/license> <http://creativecommons.org/licenses/by/4.0> ;
                                 <http://purl.org/dc/terms/bibliographicCitation> "Markus Schilling, June Lau, Bernd Bayerlein. (July 22th, 2024) MO: microscopy ontology. Version 1.1, https://w3id.org/pmd/mo/"@en ;
                                 <http://purl.org/dc/terms/title> "Microscopy Ontology (MO)"@en ;
                                 rdfs:isDefinedBy <https://w3id.org/pmd/mo> ;
                                 owl:versionInfo 1.1 ;
                                 <http://www.w3.org/2004/02/skos/core#definition> "Die Mikroskopie-Ontologie (MO) baut auf der PMD Core Ontology (PMDco) auf und bietet Konzepte für die semantische (Meta-)Datendarstellung im Bereich der Mikroskopie und Mikroanalyse. Mithilfe eines NLP-Ansatzes wird aus einem großen Korpus von Abstracts aus zwei Jahrzehnten Mikroskopie- und Mikroanalyse-Konferenzbeiträgen die zugrunde liegende Sprache der Community halbautomatisch abgeleitet und in die MO integriert. Die MO ermöglicht die semantische Integration und Verknüpfung von heterogenen Mikroskopie- und Mikroanalysedaten."@de ,
                                                                                  "The Microscopy Ontology (MO) is built on the PMD Core Ontology (PMDco) and provides concepts for semantic (meta)data representation within the domains of microscopy and microanalysis. Using an NLP approach on a large corpus of abstracts from 2 decades of Microscopy and Microanalysis Conference Proceedings, the underlying language of the community is semiautomatically derived and incorporated in the MO. The MO enables semantic integration and linkage of heterogeneous microscopy and microanalysis data."@en .

#################################################################
#    Annotation properties
#################################################################

###  http://purl.org/dc/elements/1.1/creator
<http://purl.org/dc/elements/1.1/creator> rdf:type owl:AnnotationProperty .


###  http://purl.org/dc/elements/1.1/license
<http://purl.org/dc/elements/1.1/license> rdf:type owl:AnnotationProperty .


###  http://purl.org/dc/terms/bibliographicCitation
<http://purl.org/dc/terms/bibliographicCitation> rdf:type owl:AnnotationProperty .


###  http://purl.org/dc/terms/title
<http://purl.org/dc/terms/title> rdf:type owl:AnnotationProperty .


###  http://www.w3.org/2004/02/skos/core#altLabel
<http://www.w3.org/2004/02/skos/core#altLabel> rdf:type owl:AnnotationProperty .


###  http://www.w3.org/2004/02/skos/core#definition
<http://www.w3.org/2004/02/skos/core#definition> rdf:type owl:AnnotationProperty .


###  http://www.w3.org/2004/02/skos/core#example
<http://www.w3.org/2004/02/skos/core#example> rdf:type owl:AnnotationProperty .


###  http://www.w3.org/2004/02/skos/core#prefLabel
<http://www.w3.org/2004/02/skos/core#prefLabel> rdf:type owl:AnnotationProperty .


###  https://w3id.org/pmd/co/abbreviation
<https://w3id.org/pmd/co/abbreviation> rdf:type owl:AnnotationProperty .


###  https://w3id.org/pmd/co/definitionSource
<https://w3id.org/pmd/co/definitionSource> rdf:type owl:AnnotationProperty .


###  https://w3id.org/pmd/mo/abbreviation
<https://w3id.org/pmd/mo/abbreviation> rdf:type owl:AnnotationProperty .


#################################################################
#    Classes
#################################################################

###  https://w3id.org/pmd/co/AnalysingProcess
<https://w3id.org/pmd/co/AnalysingProcess> rdf:type owl:Class .


###  https://w3id.org/pmd/co/Area
<https://w3id.org/pmd/co/Area> rdf:type owl:Class .


###  https://w3id.org/pmd/co/Component
<https://w3id.org/pmd/co/Component> rdf:type owl:Class .


###  https://w3id.org/pmd/co/Coordinates
<https://w3id.org/pmd/co/Coordinates> rdf:type owl:Class .


###  https://w3id.org/pmd/co/CrossSectionArea
<https://w3id.org/pmd/co/CrossSectionArea> rdf:type owl:Class .


###  https://w3id.org/pmd/co/Date
<https://w3id.org/pmd/co/Date> rdf:type owl:Class .


###  https://w3id.org/pmd/co/DigitalEntity
<https://w3id.org/pmd/co/DigitalEntity> rdf:type owl:Class .


###  https://w3id.org/pmd/co/Distance
<https://w3id.org/pmd/co/Distance> rdf:type owl:Class .


###  https://w3id.org/pmd/co/Duration
<https://w3id.org/pmd/co/Duration> rdf:type owl:Class .


###  https://w3id.org/pmd/co/ElectronMicroscope
<https://w3id.org/pmd/co/ElectronMicroscope> rdf:type owl:Class .


###  https://w3id.org/pmd/co/ElectronMicroscopy
<https://w3id.org/pmd/co/ElectronMicroscopy> rdf:type owl:Class .


###  https://w3id.org/pmd/co/Identifier
<https://w3id.org/pmd/co/Identifier> rdf:type owl:Class .


###  https://w3id.org/pmd/co/Length
<https://w3id.org/pmd/co/Length> rdf:type owl:Class .


###  https://w3id.org/pmd/co/ManufacturingProcess
<https://w3id.org/pmd/co/ManufacturingProcess> rdf:type owl:Class .


###  https://w3id.org/pmd/co/Micropscope
<https://w3id.org/pmd/co/Micropscope> rdf:type owl:Class .


###  https://w3id.org/pmd/co/MicroscopyProcess
<https://w3id.org/pmd/co/MicroscopyProcess> rdf:type owl:Class .


###  https://w3id.org/pmd/co/Object
<https://w3id.org/pmd/co/Object> rdf:type owl:Class .


###  https://w3id.org/pmd/co/OpticalMicroscopy
<https://w3id.org/pmd/co/OpticalMicroscopy> rdf:type owl:Class .


###  https://w3id.org/pmd/co/Process
<https://w3id.org/pmd/co/Process> rdf:type owl:Class .


###  https://w3id.org/pmd/co/ProcessingNode
<https://w3id.org/pmd/co/ProcessingNode> rdf:type owl:Class .


###  https://w3id.org/pmd/co/TestingRate
<https://w3id.org/pmd/co/TestingRate> rdf:type owl:Class .


###  https://w3id.org/pmd/co/Time
<https://w3id.org/pmd/co/Time> rdf:type owl:Class .


###  https://w3id.org/pmd/co/ValueObject
<https://w3id.org/pmd/co/ValueObject> rdf:type owl:Class .


###  https://w3id.org/pmd/mo/Aberration
<https://w3id.org/pmd/mo/Aberration> rdf:type owl:Class ;
                                     rdfs:subClassOf <https://w3id.org/pmd/co/ValueObject> ;
                                     rdfs:isDefinedBy <https://w3id.org/pmd/mo> ;
                                     rdfs:label "Aberration"@de ,
                                                "Aberration"@en ;
                                     <http://www.w3.org/2004/02/skos/core#definition> "Abweichung vom idealen oder erwarteten Verhalten, häufig im Zusammenhang mit optischen Systemen verwendet."@de ,
                                                                                      "Deviation from the ideal or expected behavior, often used in the context of optical systems."@en ;
                                     <https://w3id.org/pmd/co/definitionSource> "ChatGPT 3.5"@en .


###  https://w3id.org/pmd/mo/AccelerationVoltage
<https://w3id.org/pmd/mo/AccelerationVoltage> rdf:type owl:Class ;
                                              rdfs:subClassOf <https://w3id.org/pmd/mo/Voltage> ;
                                              rdfs:comment "Die Beschleunigungsspannung bestimmt die kinetische Energie der Elektronen und beeinflusst die Auflösung und die Eindringtiefe in die Probe."@de ,
                                                           "The acceleration voltage determines the kinetic energy of the electrons and affects the resolution and depth of penetration in the sample."@en ;
                                              rdfs:isDefinedBy <https://w3id.org/pmd/mo> ;
                                              rdfs:label "Acceleration Voltage"@en ,
                                                         "Beschleunigungsspannung"@de ;
                                              <http://www.w3.org/2004/02/skos/core#definition> "Diese Klasse beschreibt die Spannung, die an ein Elektronenmikroskop angelegt wird, um die von der Elektronenquelle (in der Regel eine Kathode) emittierten Elektronen auf die Probe zu beschleunigen."@de ,
                                                                                               "This class decribes the voltage applied to an electron microscope to accelerate the electrons emitted from the electron source (usually a cathode) towards the specimen."@en ;
                                              <https://w3id.org/pmd/co/definitionSource> "ChatGPT 3.5" .


###  https://w3id.org/pmd/mo/AcquisitionDate
<https://w3id.org/pmd/mo/AcquisitionDate> rdf:type owl:Class ;
                                          rdfs:subClassOf <https://w3id.org/pmd/co/Date> ;
                                          rdfs:isDefinedBy <https://w3id.org/pmd/mo> ;
                                          rdfs:label "Acquisition Date"@en ,
                                                     "Erfassungsdatum"@de ;
                                          <http://www.w3.org/2004/02/skos/core#definition> "The date when the image or data was acquired."@en ;
                                          <https://w3id.org/pmd/co/definitionSource> "ChatGPT 3.5"@en .


###  https://w3id.org/pmd/mo/AcquisitionTime
<https://w3id.org/pmd/mo/AcquisitionTime> rdf:type owl:Class ;
                                          rdfs:subClassOf <https://w3id.org/pmd/co/Time> ;
                                          rdfs:isDefinedBy <https://w3id.org/pmd/mo> ;
                                          rdfs:label "Acquisition Time"@en ,
                                                     "Erfassungszeit"@de ;
                                          <http://www.w3.org/2004/02/skos/core#definition> "The time when the image or data was acquired."@en ;
                                          <https://w3id.org/pmd/co/definitionSource> "ChatGPT 3.5"@en .


###  https://w3id.org/pmd/mo/ActualMagnification
<https://w3id.org/pmd/mo/ActualMagnification> rdf:type owl:Class ;
                                              rdfs:subClassOf <https://w3id.org/pmd/mo/Magnification> ;
                                              <http://purl.obolibrary.org/obo/IAO_0000117> "PMDco Team"@en ;
                                              <http://purl.obolibrary.org/obo/IAO_0000119> "ChatGPT 3.5"@en ;
                                              rdfs:label "Actual Magnification"@en ,
                                                         "Tatsächliche Vergrößerung"@de ;
                                              <http://www.w3.org/2004/02/skos/core#definition> "Actual Magnification refers to the true magnification level achieved in an electron microscope, which may differ from the indicated magnification."@en ,
                                                                                               "Tatsächliche Vergrößerung bezieht sich auf den tatsächlichen Vergrößerungsgrad, der in einem Elektronenmikroskop erreicht wird und sich von der angegebenen Vergrößerung unterscheiden kann."@de .


###  https://w3id.org/pmd/mo/Age
<https://w3id.org/pmd/mo/Age> rdf:type owl:Class ;
                              rdfs:subClassOf <https://w3id.org/pmd/co/Duration> ;
                              rdfs:isDefinedBy <https://w3id.org/pmd/mo> ;
                              rdfs:label "Age"@en ,
                                         "Alter"@de ;
                              <http://www.w3.org/2004/02/skos/core#definition> "Die Dauer, die ein Objekt oder Organismus existiert hat."@de ,
                                                                               "The duration that an object or organism has existed."@en ;
                              <https://w3id.org/pmd/co/definitionSource> "ChatGPT 3.5"@en .


###  https://w3id.org/pmd/mo/Angle
<https://w3id.org/pmd/mo/Angle> rdf:type owl:Class ;
                                rdfs:subClassOf <https://w3id.org/pmd/co/ValueObject> ;
                                rdfs:label <https://w3id.org/pmd/mo> ,
                                           "Angle"@en ,
                                           "Winkel"@de ;
                                <http://www.w3.org/2004/02/skos/core#definition> """In der Geometrie und Trigonometrie ist ein Winkel ein Maß für eine Drehung, das erforderlich ist, um eine Linie oder Ebene mit einer anderen zur Deckung zu bringen. Ein Winkel wird durch zwei Strahlen gebildet, die einen gemeinsamen Endpunkt haben, der als Scheitelpunkt des Winkels bezeichnet wird. Die Strahlen werden als die Seiten des Winkels bezeichnet. 

Hinweis: Das Konzept des Winkels ist in der Geometrie von grundlegender Bedeutung und wird häufig verwendet, um die relative Ausrichtung von Linien, Ebenen oder Flächen zu beschreiben. Winkel werden in der Regel in Grad (°) oder Bogenmaß (rad) gemessen."""@de ,
                                                                                 """In geometry and trigonometry, an angle is a measure of the amount of rotation needed to bring one line or plane into coincidence with another. An angle is formed by two rays that share a common endpoint, known as the vertex of the angle. The rays are referred to as the sides of the angle. 

Note: The concept of an angle is fundamental in geometry and is often used to describe the relative orientation of lines, planes, or surfaces. Angles are typically measured in degrees (°) or radians (rad)."""@en ;
                                <https://w3id.org/pmd/co/definitionSource> "ChatGPT 3.5"@en .


###  https://w3id.org/pmd/mo/AnnularBrightFieldScanningTransmissionElectronMicroscopy
<https://w3id.org/pmd/mo/AnnularBrightFieldScanningTransmissionElectronMicroscopy> rdf:type owl:Class ;
                                                                                   rdfs:subClassOf <https://w3id.org/pmd/mo/ScanningTransmissionElectronMicroscopy> ;
                                                                                   rdfs:isDefinedBy <https://w3id.org/pmd/mo> ;
                                                                                   rdfs:label "Annular Bright Field Scanning Transmission Electron Microscopy"@en ,
                                                                                              "Ringförmige Hellfeld-Rastertransmissionselektronenmikroskopie"@de ;
                                                                                   <http://www.w3.org/2004/02/skos/core#definition> "ABF STEM is a technique that utilizes a specific arrangement of detectors to enhance contrast in STEM images, particularly for heavy elements."@en ;
                                                                                   <https://w3id.org/pmd/co/definitionSource> "ChatGPT 3.5"@en ;
                                                                                   <https://w3id.org/pmd/mo/abbreviation> "ABF-STEM"@en .


###  https://w3id.org/pmd/mo/AnnularDarkFieldScanningTransmissionElectronMicroscopy
<https://w3id.org/pmd/mo/AnnularDarkFieldScanningTransmissionElectronMicroscopy> rdf:type owl:Class ;
                                                                                 rdfs:subClassOf <https://w3id.org/pmd/mo/ScanningTransmissionElectronMicroscopy> ;
                                                                                 rdfs:isDefinedBy <https://w3id.org/pmd/mo> ;
                                                                                 rdfs:label "Annular Dark Field Scanning Transmission Electron Microscopy"@en ,
                                                                                            "Ringförmige Dunkelfeld-Rastertransmissionselektronenmikroskopie"@de ;
                                                                                 <http://www.w3.org/2004/02/skos/core#definition> "ADF STEM is a technique that utilizes a specific arrangement of detectors to create contrast in STEM images based on the scattered electrons."@en ;
                                                                                 <https://w3id.org/pmd/co/definitionSource> "ChatGPT 3.5"@en ;
                                                                                 <https://w3id.org/pmd/mo/abbreviation> "ADF-STEM"@en .


###  https://w3id.org/pmd/mo/Anode
<https://w3id.org/pmd/mo/Anode> rdf:type owl:Class ;
                                rdfs:subClassOf <https://w3id.org/pmd/mo/Electrode> ;
                                rdfs:isDefinedBy <https://w3id.org/pmd/mo> ;
                                rdfs:label "Anode"@de ,
                                           "Anode"@en ;
                                <http://www.w3.org/2004/02/skos/core#definition> "The anode is the positively charged electrode in an electrochemical cell or other electrically driven systems. It serves as the site where oxidation occurs, meaning electrons are released from the anode, typically moving towards the cathode. In devices like batteries, the anode is where electrons are produced during the discharge process."@en ;
                                <https://w3id.org/pmd/co/definitionSource> "ChatGPT 3.5"@en .


###  https://w3id.org/pmd/mo/Aperture
<https://w3id.org/pmd/mo/Aperture> rdf:type owl:Class ;
                                   rdfs:subClassOf <https://w3id.org/pmd/co/Component> ;
                                   rdfs:isDefinedBy <https://w3id.org/pmd/mo> ;
                                   rdfs:label "Aperturblende"@de ,
                                              "Aperture"@en ;
                                   <http://www.w3.org/2004/02/skos/core#altLabel> "Pinhole"@en ;
                                   <http://www.w3.org/2004/02/skos/core#definition> "An opening through which light or other radiation enters a camera or other optical instrument."@en ,
                                                                                    "Eine Öffnung, durch die Licht oder andere Strahlung in eine Kamera oder ein anderes optisches Instrument eintritt."@de ;
                                   <https://w3id.org/pmd/co/definitionSource> "ChatGPT 3.5"@en .


###  https://w3id.org/pmd/mo/ApertureSize
<https://w3id.org/pmd/mo/ApertureSize> rdf:type owl:Class ;
                                       rdfs:subClassOf <https://w3id.org/pmd/co/ValueObject> ;
                                       rdfs:isDefinedBy <https://w3id.org/pmd/mo> ;
                                       rdfs:label "Aperture Size"@en ,
                                                  "Blendengröße"@de ;
                                       <http://www.w3.org/2004/02/skos/core#definition> "Die Größe der Öffnung in einer Blende, die die Menge des durchgehenden Lichts oder der Strahlung beeinflusst."@de ,
                                                                                        "The size of the opening in an aperture, affecting the amount of light or radiation passing through."@en ;
                                       <https://w3id.org/pmd/co/definitionSource> "ChatGPT 3.5"@en .


###  https://w3id.org/pmd/mo/AtmosphericScanningElectronMicroscopy
<https://w3id.org/pmd/mo/AtmosphericScanningElectronMicroscopy> rdf:type owl:Class ;
                                                                rdfs:subClassOf <https://w3id.org/pmd/mo/ScanningElectronMicroscopy> ;
                                                                rdfs:isDefinedBy <https://w3id.org/pmd/mo> ;
                                                                rdfs:label "Atmospheric Scanning Electron Microscopy"@en ,
                                                                           "Atmosphärische Rasterelektronenmikroskopie"@de ;
                                                                <http://www.w3.org/2004/02/skos/core#definition> "Atmospheric Scanning Electron Microscopy is a technique that allows samples to be imaged in their natural, hydrated state at atmospheric pressure. It enables the observation of biological and other hydrated specimens without the need for dehydration or coating."@en ;
                                                                <https://w3id.org/pmd/co/definitionSource> "ChatGPT 3.5"@en ;
                                                                <https://w3id.org/pmd/mo/abbreviation> "ASEM"@en .


###  https://w3id.org/pmd/mo/AtomicResolution
<https://w3id.org/pmd/mo/AtomicResolution> rdf:type owl:Class ;
                                           rdfs:subClassOf <https://w3id.org/pmd/mo/Resolution> ;
                                           rdfs:isDefinedBy <https://w3id.org/pmd/mo> ;
                                           rdfs:label "Atomare Auflösung"@de ,
                                                      "Atomic Resolution"@en ;
                                           <http://www.w3.org/2004/02/skos/core#definition> "Die Fähigkeit, einzelne Atome in einem Bild oder einer Struktur aufzulösen."@de ,
                                                                                            "The ability to resolve individual atoms in an image or structure."@en ;
                                           <https://w3id.org/pmd/co/definitionSource> "ChatGPT 3.5"@en .


###  https://w3id.org/pmd/mo/AugerElectronSpectroscopy
<https://w3id.org/pmd/mo/AugerElectronSpectroscopy> rdf:type owl:Class ;
                                                    rdfs:subClassOf <https://w3id.org/pmd/mo/Spectroscopy> ;
                                                    rdfs:isDefinedBy <https://w3id.org/pmd/mo> ;
                                                    rdfs:label "Auger Electron Spectroscopy"@en ,
                                                               "Auger-Elektronen-Spektroskopie"@de ;
                                                    <http://www.w3.org/2004/02/skos/core#definition> """Auger Electron Spectroscopy (AES) is a surface analysis technique used in the field of materials science and surface chemistry. It involves the study of the interactions between high-energy electrons and atoms on the surface of a material. The process is named after Pierre Auger, who made significant contributions to the understanding of this phenomenon.
In AES, a sample's surface is bombarded with a beam of high-energy electrons, which causes inner-shell electrons to be ejected from the atoms in the sample. These vacancies are then filled by higher-energy electrons from outer shells, leading to the emission of Auger electrons. The energy of these emitted Auger electrons is characteristic of the specific elements present in the sample and their chemical states.
By analyzing the energy spectrum of the emitted Auger electrons, researchers can identify the elements present on the surface of the material and determine their relative concentrations. Auger Electron Spectroscopy provides valuable information about the elemental composition and chemical bonding of the top few atomic layers of a material, making it a powerful tool for studying surface properties, thin films, and interfaces in various scientific and industrial applications."""@en ;
                                                    <https://w3id.org/pmd/co/definitionSource> "ChatGPT 3.5"@en ;
                                                    <https://w3id.org/pmd/mo/abbreviation> "AES"@en .


###  https://w3id.org/pmd/mo/Beam
<https://w3id.org/pmd/mo/Beam> rdf:type owl:Class ;
                               rdfs:subClassOf <https://w3id.org/pmd/co/Object> ;
                               rdfs:isDefinedBy <https://w3id.org/pmd/mo> ;
                               rdfs:label "Beam"@en ,
                                          "Strahl"@de ;
                               <http://www.w3.org/2004/02/skos/core#definition> "A stream of electrons emitted from the electron source and directed towards the specimen in an electron microscope."@en ,
                                                                                "Ein Strom von Elektronen, der von der Elektronenquelle emittiert und auf die Probe in einem Elektronenmikroskop gerichtet wird."@de ;
                               <https://w3id.org/pmd/co/definitionSource> "ChatGPT 3.5" .


###  https://w3id.org/pmd/mo/BeamCurrent
<https://w3id.org/pmd/mo/BeamCurrent> rdf:type owl:Class ;
                                      rdfs:subClassOf <https://w3id.org/pmd/mo/Current> ;
                                      rdfs:isDefinedBy <https://w3id.org/pmd/mo> ;
                                      rdfs:label "Beam Current"@en ,
                                                 "Strahlstrom"@de ;
                                      <http://www.w3.org/2004/02/skos/core#definition> "Die Intensität des Elektronenstrahls, gemessen als Anzahl der Elektronen, die eine bestimmte Fläche pro Zeiteinheit durchdringen."@de ,
                                                                                       "The intensity of the electron beam, measured as the number of electrons passing through a given area per unit time."@en ;
                                      <https://w3id.org/pmd/co/definitionSource> "ChatGPT 3.5" .


###  https://w3id.org/pmd/mo/BeamEnergy
<https://w3id.org/pmd/mo/BeamEnergy> rdf:type owl:Class ;
                                     rdfs:subClassOf <https://w3id.org/pmd/mo/Energy> ;
                                     rdfs:isDefinedBy <https://w3id.org/pmd/mo> ;
                                     rdfs:label "Beam Energy"@en ,
                                                "Strahlungsenergie"@de ;
                                     <http://www.w3.org/2004/02/skos/core#definition> "Die Energie eines Teilchen- oder Photonenstrahls, der in verschiedenen Analyseverfahren verwendet wird."@de ,
                                                                                      "The energy of a particle or photon beam used in various analytical techniques."@en ;
                                     <https://w3id.org/pmd/co/definitionSource> "ChatGPT 3.5"@en .


###  https://w3id.org/pmd/mo/BeamOffsetX
<https://w3id.org/pmd/mo/BeamOffsetX> rdf:type owl:Class ;
                                      rdfs:subClassOf <https://w3id.org/pmd/co/ValueObject> ;
                                      rdfs:isDefinedBy <https://w3id.org/pmd/mo> ;
                                      rdfs:label "Beam Offset X"@en ,
                                                 "Strahlversatz X"@de ;
                                      <http://www.w3.org/2004/02/skos/core#definition> "Der Versatz des Elektronenstrahls entlang der X-Achse in der Elektronenmikroskopie."@de ,
                                                                                       "The offset of the electron beam along the X-axis in electron microscopy."@en ;
                                      <https://w3id.org/pmd/co/definitionSource> "ChatGPT 3.5"@en .


###  https://w3id.org/pmd/mo/BeamOffsetY
<https://w3id.org/pmd/mo/BeamOffsetY> rdf:type owl:Class ;
                                      rdfs:subClassOf <https://w3id.org/pmd/co/ValueObject> ;
                                      rdfs:isDefinedBy <https://w3id.org/pmd/mo> ;
                                      rdfs:label "Beam Offset Y"@en ,
                                                 "Strahlversatz Y"@de ;
                                      <http://www.w3.org/2004/02/skos/core#definition> "Der Versatz des Elektronenstrahls entlang der Y-Achse in der Elektronenmikroskopie."@de ,
                                                                                       "The offset of the electron beam along the Y-axis in electron microscopy."@en ;
                                      <https://w3id.org/pmd/co/definitionSource> "ChatGPT 3.5"@en .


###  https://w3id.org/pmd/mo/BeamPath
<https://w3id.org/pmd/mo/BeamPath> rdf:type owl:Class ;
                                   rdfs:subClassOf <https://w3id.org/pmd/co/Object> ;
                                   rdfs:isDefinedBy <https://w3id.org/pmd/mo> ;
                                   rdfs:label "Beam Path"@en ,
                                              "Strahlengang"@de ;
                                   <http://www.w3.org/2004/02/skos/core#altLabel> "Strahlenweg"@de ;
                                   <http://www.w3.org/2004/02/skos/core#definition> "Die Flugbahn des Elektronenstrahls auf seinem Weg durch das Elektronenmikroskop von der Elektronenquelle zur Probe und dann zum Detektor."@de ,
                                                                                    "The trajectory followed by the electron beam as it travels through the electron microscope, from the electron source to the specimen and then to the detector."@en ;
                                   <https://w3id.org/pmd/co/definitionSource> "ChatGPT 3.5" .


###  https://w3id.org/pmd/mo/BeamShiftX
<https://w3id.org/pmd/mo/BeamShiftX> rdf:type owl:Class ;
                                     rdfs:subClassOf <https://w3id.org/pmd/co/ValueObject> ;
                                     rdfs:isDefinedBy <https://w3id.org/pmd/mo> ;
                                     rdfs:label "Beam Shift X"@en ,
                                                "Strahlverschiebung X"@de ;
                                     <http://www.w3.org/2004/02/skos/core#definition> "Die Verschiebung des Elektronenstrahls entlang der X-Achse in der Elektronenmikroskopie."@de ,
                                                                                      "The shift of the electron beam along the X-axis in electron microscopy."@en ;
                                     <https://w3id.org/pmd/co/definitionSource> "ChatGPT 3.5"@en .


###  https://w3id.org/pmd/mo/BeamShiftY
<https://w3id.org/pmd/mo/BeamShiftY> rdf:type owl:Class ;
                                     rdfs:subClassOf <https://w3id.org/pmd/co/ValueObject> ;
                                     rdfs:isDefinedBy <https://w3id.org/pmd/mo> ;
                                     rdfs:label "Beam Shift Y"@en ,
                                                "Strahlverschiebung Y"@de ;
                                     <http://www.w3.org/2004/02/skos/core#definition> "Die Verschiebung des Elektronenstrahls entlang der Y-Achse in der Elektronenmikroskopie."@de ,
                                                                                      "The shift of the electron beam along the Y-axis in electron microscopy."@en ;
                                     <https://w3id.org/pmd/co/definitionSource> "ChatGPT 3.5"@en .


###  https://w3id.org/pmd/mo/BeamTiltX
<https://w3id.org/pmd/mo/BeamTiltX> rdf:type owl:Class ;
                                    rdfs:subClassOf <https://w3id.org/pmd/co/ValueObject> ;
                                    <http://purl.obolibrary.org/obo/IAO_0000117> "PMDco Team"@en ;
                                    <http://purl.obolibrary.org/obo/IAO_0000119> "ChatGPT 3.5"@en ;
                                    rdfs:label "Beam Tilt X"@en ,
                                               "Strahlneigung X"@de ,
                                               "Strahlneigung X-Richtung"@de ;
                                    <http://www.w3.org/2004/02/skos/core#definition> "Beam Tilt X refers to the tilting of the electron beam in the X-axis direction within an electron microscope."@en ,
                                                                                     "Strahlneigung X bezieht sich auf die Neigung des Elektronenstrahls in Richtung der X-Achse innerhalb eines Elektronenmikroskops."@de .


###  https://w3id.org/pmd/mo/BeamTiltY
<https://w3id.org/pmd/mo/BeamTiltY> rdf:type owl:Class ;
                                    rdfs:subClassOf <https://w3id.org/pmd/co/ValueObject> ;
                                    <http://purl.obolibrary.org/obo/IAO_0000117> "PMDco Team"@en ;
                                    <http://purl.obolibrary.org/obo/IAO_0000119> "ChatGPT 3.5"@en ;
                                    rdfs:label "Beam Tilt Y"@en ,
                                               "Strahlneigung Y"@de ,
                                               "Strahlneigung Y-Richtung"@de ;
                                    <http://www.w3.org/2004/02/skos/core#definition> "Beam Tilt Y refers to the tilting of the electron beam in the Y-axis direction within an electron microscope."@en ,
                                                                                     "Strahlneigung Y bezieht sich auf die Neigung des Elektronenstrahls in Richtung der Y-Achse innerhalb eines Elektronenmikroskops."@de .


###  https://w3id.org/pmd/mo/Bias
<https://w3id.org/pmd/mo/Bias> rdf:type owl:Class ;
                               rdfs:subClassOf <https://w3id.org/pmd/co/ValueObject> ;
                               rdfs:isDefinedBy <https://w3id.org/pmd/mo> ;
                               rdfs:label "Bias"@en ,
                                          "Vorspannung"@de ;
                               <http://www.w3.org/2004/02/skos/core#definition> "A voltage or other value that influences the operation of an electronic component."@en ,
                                                                                "Eine Spannung oder ein anderer Wert, der den Betrieb eines elektronischen Bauteils beeinflusst."@de ;
                               <https://w3id.org/pmd/co/definitionSource> "ChatGPT 3.5"@en .


###  https://w3id.org/pmd/mo/BrightFieldTransmissionElectronMicroscopy
<https://w3id.org/pmd/mo/BrightFieldTransmissionElectronMicroscopy> rdf:type owl:Class ;
                                                                    rdfs:subClassOf <https://w3id.org/pmd/mo/TransmissionElectronMicroscopy> ;
                                                                    rdfs:isDefinedBy <https://w3id.org/pmd/mo> ;
                                                                    rdfs:label "Bright Field Transmission Electron Microscopy"@en ,
                                                                               "Hellfeld-Transmissionselektronenmikroskopie"@de ;
                                                                    <http://www.w3.org/2004/02/skos/core#definition> "Bright Field TEM is an imaging mode in transmission electron microscopy where regions of the sample that scatter electrons less appear brighter in the resulting image."@en ;
                                                                    <https://w3id.org/pmd/co/definitionSource> "ChatGPT 3.5"@en ;
                                                                    <https://w3id.org/pmd/mo/abbreviation> "BFTEM"@en .


###  https://w3id.org/pmd/mo/Brightness
<https://w3id.org/pmd/mo/Brightness> rdf:type owl:Class ;
                                     rdfs:subClassOf <https://w3id.org/pmd/co/ValueObject> ;
                                     rdfs:isDefinedBy <https://w3id.org/pmd/mo> ;
                                     rdfs:label "Brightness"@en ,
                                                "Helligkeit"@de ;
                                     <http://www.w3.org/2004/02/skos/core#definition> "Der Grad der Lichtintensität in einem Bild."@de ,
                                                                                      "The level of light intensity in an image."@en ;
                                     <https://w3id.org/pmd/co/definitionSource> "ChatGPT 3.5"@en .


###  https://w3id.org/pmd/mo/CEOS-CEFIDfilter
<https://w3id.org/pmd/mo/CEOS-CEFIDfilter> rdf:type owl:Class ;
                                           rdfs:subClassOf <https://w3id.org/pmd/mo/EnergyFilter> ,
                                                           <https://w3id.org/pmd/mo/ImageFilter> ;
                                           <http://purl.obolibrary.org/obo/IAO_0000117> "PMDco Team"@en ;
                                           <http://purl.obolibrary.org/obo/IAO_0000119> "ChatGPT 3.5"@en ;
                                           rdfs:label "CEOS-CEFID Filter"@de ,
                                                      "CEOS-CEFID Filter"@en ;
                                           <http://www.w3.org/2004/02/skos/core#definition> "A CEOS-CEFID Filter is a specialized energy filter used in electron microscopes for enhancing image contrast and resolution."@en ,
                                                                                            "Ein CEOS-CEFID Filter ist ein spezialisierter Energiefilter, der in Elektronenmikroskopen verwendet wird, um den Bildkontrast und die Auflösung zu verbessern."@de .


###  https://w3id.org/pmd/mo/CameraLength
<https://w3id.org/pmd/mo/CameraLength> rdf:type owl:Class ;
                                       rdfs:subClassOf <https://w3id.org/pmd/co/Length> ;
                                       rdfs:isDefinedBy <https://w3id.org/pmd/mo> ;
                                       rdfs:label "Camera Length"@en ;
                                       <http://www.w3.org/2004/02/skos/core#definition> "Der Abstand zwischen der Probe und der Kamera, die zur Aufnahme von Bildern in einem Elektronenmikroskop verwendet wird."@de ,
                                                                                        "The distance between the specimen and the camera used to capture images in an electron microscope."@en ;
                                       <http://www.w3.org/2004/02/skos/core#example> "STEM camera length"@en ;
                                       <https://w3id.org/pmd/co/definitionSource> "Camera Length"@en ,
                                                                                  "Kameralänge"@de ,
                                                                                  "ChatGPT 3.5" .


###  https://w3id.org/pmd/mo/Cathode
<https://w3id.org/pmd/mo/Cathode> rdf:type owl:Class ;
                                  rdfs:subClassOf <https://w3id.org/pmd/mo/Electrode> ;
                                  rdfs:isDefinedBy <https://w3id.org/pmd/mo> ;
                                  rdfs:label "Cathode"@en ,
                                             "Kathode"@de ;
                                  <http://www.w3.org/2004/02/skos/core#definition> "The cathode is the negatively charged electrode in an electrochemical cell or other electrical systems. It is the site where reduction occurs, leading to the acceptance of electrons from the external circuit. In batteries, for instance, the cathode is where electrons are consumed during the discharge process."@en ;
                                  <https://w3id.org/pmd/co/definitionSource> "ChatGPT 3.5"@en .


###  https://w3id.org/pmd/mo/Chamber
<https://w3id.org/pmd/mo/Chamber> rdf:type owl:Class ;
                                  rdfs:subClassOf <https://w3id.org/pmd/co/Object> ;
                                  <http://purl.obolibrary.org/obo/IAO_0000117> "PMDco Team"@en ;
                                  <http://purl.obolibrary.org/obo/IAO_0000119> "ChatGPT 3.5"@en ;
                                  rdfs:label "Chamber"@en ,
                                             "Kammer"@de ;
                                  <http://www.w3.org/2004/02/skos/core#definition> "Chamber refers to the enclosed space within an electron microscope where the sample is placed and vacuum conditions are maintained."@en ,
                                                                                   "Kammer bezieht sich auf den abgeschlossenen Raum in einem Elektronenmikroskop, in dem die Probe platziert wird und Vakuumbedingungen aufrechterhalten werden."@de .


###  https://w3id.org/pmd/mo/ChamberVacuum
<https://w3id.org/pmd/mo/ChamberVacuum> rdf:type owl:Class ;
                                        rdfs:subClassOf <https://w3id.org/pmd/mo/Vacuum> ;
                                        rdfs:isDefinedBy <https://w3id.org/pmd/mo> ;
                                        rdfs:label "Chamber Vacuum"@en ,
                                                   "Kammervakuum"@de ;
                                        <http://www.w3.org/2004/02/skos/core#definition> "Das Vakuumniveau im Inneren der Kammer eines Elektronenmikroskops oder eines anderen Geräts."@de ,
                                                                                         "The vacuum level inside the chamber of an electron microscope or other device."@en ;
                                        <https://w3id.org/pmd/co/definitionSource> "ChatGPT 3.5"@en .


###  https://w3id.org/pmd/mo/Channel
<https://w3id.org/pmd/mo/Channel> rdf:type owl:Class ;
                                  rdfs:subClassOf <https://w3id.org/pmd/co/Object> ;
                                  rdfs:isDefinedBy <https://w3id.org/pmd/mo> ;
                                  rdfs:label "Channel"@en ,
                                             "Kanal"@de ;
                                  <http://www.w3.org/2004/02/skos/core#definition> "A path along which signals such as data or electrical impulses are transmitted."@en ,
                                                                                   "Ein Pfad, entlang dem Signale wie Daten oder elektrische Impulse übertragen werden."@de ;
                                  <https://w3id.org/pmd/co/definitionSource> "ChatGPT 3.5"@en .


###  https://w3id.org/pmd/mo/ChromaticAberration
<https://w3id.org/pmd/mo/ChromaticAberration> rdf:type owl:Class ;
                                              rdfs:subClassOf <https://w3id.org/pmd/mo/Aberration> ;
                                              rdfs:isDefinedBy <https://w3id.org/pmd/mo> ;
                                              rdfs:label "Chromatic Aberration"@en ,
                                                         "Chromatische Aberration"@de ;
                                              <http://www.w3.org/2004/02/skos/core#definition> "Die Unfähigkeit eines Objektivs, alle Farben auf denselben Konvergenzpunkt zu fokussieren."@de ,
                                                                                               "The failure of a lens to focus all colors to the same convergence point."@en ;
                                              <https://w3id.org/pmd/co/definitionSource> "ChatGPT 3.5"@en .


###  https://w3id.org/pmd/mo/CoherentBeam
<https://w3id.org/pmd/mo/CoherentBeam> rdf:type owl:Class ;
                                       rdfs:subClassOf <https://w3id.org/pmd/mo/Beam> ;
                                       rdfs:isDefinedBy <https://w3id.org/pmd/mo> ;
                                       rdfs:label "Coherent Beam"@en ,
                                                  "Kohärenter Strahl"@de ;
                                       <http://www.w3.org/2004/02/skos/core#definition> "An electron beam in which the individual electrons maintain a constant phase relationship with each other, resulting in interference patterns when interacting with a sample."@en ,
                                                                                        "Ein Elektronenstrahl, bei dem die einzelnen Elektronen eine konstante Phasenbeziehung zueinander haben, was bei der Wechselwirkung mit einer Probe zu Interferenzmustern führt."@de ;
                                       <https://w3id.org/pmd/co/definitionSource> "ChatGPT 3.5" .


###  https://w3id.org/pmd/mo/CollectionEfficiency
<https://w3id.org/pmd/mo/CollectionEfficiency> rdf:type owl:Class ;
                                               rdfs:subClassOf <https://w3id.org/pmd/mo/Efficiency> ;
                                               rdfs:isDefinedBy <https://w3id.org/pmd/mo> ;
                                               rdfs:label "Collection Efficiency"@en ,
                                                          "Kollektoreffizienz"@de ;
                                               <http://www.w3.org/2004/02/skos/core#definition> "Die Fähigkeit eines Detektors oder Systems, relevante Signale oder Daten zu erfassen und aufzuzeichnen."@de ,
                                                                                                "The ability of a detector or system to capture and record relevant signals or data."@en ;
                                               <https://w3id.org/pmd/co/definitionSource> "ChatGPT 3.5"@en .


###  https://w3id.org/pmd/mo/Collector
<https://w3id.org/pmd/mo/Collector> rdf:type owl:Class ;
                                    rdfs:subClassOf <https://w3id.org/pmd/co/ProcessingNode> ;
                                    rdfs:isDefinedBy <https://w3id.org/pmd/mo> ;
                                    rdfs:label "Collector"@en ,
                                               "Kollektor"@de ;
                                    <http://www.w3.org/2004/02/skos/core#definition> "A device that collects charged particles or radiation in a microscope or other instrument."@en ,
                                                                                     "Ein Gerät, das geladene Teilchen oder Strahlung in einem Mikroskop oder einem anderen Instrument sammelt."@de ;
                                    <https://w3id.org/pmd/co/definitionSource> "ChatGPT 3.5"@en .


###  https://w3id.org/pmd/mo/CondensorAperture
<https://w3id.org/pmd/mo/CondensorAperture> rdf:type owl:Class ;
                                            rdfs:subClassOf <https://w3id.org/pmd/mo/Aperture> ;
                                            rdfs:isDefinedBy <https://w3id.org/pmd/mo> ;
                                            rdfs:label "Condensor Aperture"@en ,
                                                       "Kondensorblende"@de ;
                                            <http://www.w3.org/2004/02/skos/core#definition> "An aperture that controls the amount of light entering the condenser lens system in a microscope."@en ,
                                                                                             "Eine Blende, die die Lichtmenge steuert, die in das Kondensorlinsensystem eines Mikroskops eintritt."@de ;
                                            <https://w3id.org/pmd/co/definitionSource> "ChatGPT 3.5"@en .


###  https://w3id.org/pmd/mo/CondensorLense
<https://w3id.org/pmd/mo/CondensorLense> rdf:type owl:Class ;
                                         rdfs:subClassOf <https://w3id.org/pmd/mo/Lense> ;
                                         rdfs:isDefinedBy <https://w3id.org/pmd/mo> ;
                                         rdfs:label "Condensor Lens"@en ,
                                                    "Kondensorlinse"@de ;
                                         <http://www.w3.org/2004/02/skos/core#definition> "A condenser lens is an optical element used in microscopy and other optical systems to focus and control the illumination on the sample being observed. It is positioned below the light source and directs light rays onto the specimen, making the illumination uniform and optimizing the quality of the sample's image. The condenser lens helps enhance contrast, resolution, and overall image quality by ensuring that a consistent and concentrated light beam illuminates the specimen."@en ;
                                         <https://w3id.org/pmd/co/definitionSource> "ChatGPT 3.5"@en .


###  https://w3id.org/pmd/mo/ConfocalLaserScanningMicroscopy
<https://w3id.org/pmd/mo/ConfocalLaserScanningMicroscopy> rdf:type owl:Class ;
                                                          rdfs:subClassOf <https://w3id.org/pmd/mo/LightMicroscopy> ;
                                                          rdfs:isDefinedBy <https://w3id.org/pmd/mo> ;
                                                          rdfs:label "Confocal Laser Scanning Microscopy"@en ,
                                                                     "Konfokale Laser-Scanning-Mikroskopie"@de ;
                                                          <http://www.w3.org/2004/02/skos/core#definition> "Confocal Laser Scanning Microscopy (CLSM) is an optical imaging technique that enhances resolution and eliminates out-of-focus blur by using a spatial pinhole and laser illumination. A focused laser beam is scanned across the sample's surface or depth, and only the light emitted from the focal plane (or a defined section) passes through the pinhole to form an image. CLSM provides high-resolution three-dimensional images, making it popular for biological imaging and studying fluorescently labeled samples."@en ;
                                                          <https://w3id.org/pmd/co/definitionSource> "ChatGPT 3.5"@en ;
                                                          <https://w3id.org/pmd/mo/abbreviation> "CLSM"@en .


###  https://w3id.org/pmd/mo/Contrast
<https://w3id.org/pmd/mo/Contrast> rdf:type owl:Class ;
                                   rdfs:subClassOf <https://w3id.org/pmd/co/ValueObject> ;
                                   rdfs:isDefinedBy <https://w3id.org/pmd/mo> ;
                                   rdfs:label "Contrast"@en ,
                                              "Kontrast"@de ;
                                   <http://www.w3.org/2004/02/skos/core#definition> "Der Unterschied in der Leuchtdichte oder Farbe, der Objekte in einem Bild unterscheidbar macht."@de ,
                                                                                    "The difference in luminance or color that makes objects distinguishable in an image."@en ;
                                   <https://w3id.org/pmd/co/definitionSource> "ChatGPT 3.5"@en .


###  https://w3id.org/pmd/mo/ConvergenceAngle
<https://w3id.org/pmd/mo/ConvergenceAngle> rdf:type owl:Class ;
                                           rdfs:subClassOf <https://w3id.org/pmd/mo/Angle> ;
                                           rdfs:comment "Der Konvergenzwinkel beeinflusst die Schärfentiefe und die Auflösung des Bildes."@de ,
                                                        "The convergence angle affects the depth of field and resolution of the image."@en ;
                                           rdfs:isDefinedBy <https://w3id.org/pmd/mo> ;
                                           rdfs:label "Convergence Angle"@en ,
                                                      "Konvergenzwinkel"@de ;
                                           <http://www.w3.org/2004/02/skos/core#definition> "Der Winkel, in dem der Elektronenstrahl in einem Elektronenmikroskop auf die Probe trifft."@de ,
                                                                                            "The angle at which the electron beam converges onto the specimen in an electron microscope."@en ;
                                           <https://w3id.org/pmd/co/definitionSource> "ChatGPT 3.5" .


###  https://w3id.org/pmd/mo/ConvergentBeamElectronDiffraction
<https://w3id.org/pmd/mo/ConvergentBeamElectronDiffraction> rdf:type owl:Class ;
                                                            rdfs:subClassOf <https://w3id.org/pmd/mo/ElectronDiffraction> ;
                                                            <http://purl.obolibrary.org/obo/IAO_0000117> "PMDco Team"@en ;
                                                            <http://purl.obolibrary.org/obo/IAO_0000119> "ChatGPT 3.5"@en ;
                                                            rdfs:label "Convergent Beam Electron Diffraction"@en ,
                                                                       "Konvergente Strahl-Elektronenbeugung"@de ;
                                                            <http://www.w3.org/2004/02/skos/core#definition> "Convergent Beam Electron Diffraction is a technique in electron microscopy where a convergent electron beam is used to form diffraction patterns, allowing for precise analysis of crystal structures."@en ,
                                                                                                             "Konvergente Strahl-Elektronenbeugung ist eine Technik in der Elektronenmikroskopie, bei der ein konvergenter Elektronenstrahl verwendet wird, um Beugungsmuster zu erzeugen, die eine präzise Analyse von Kristallstrukturen ermöglichen."@de .


###  https://w3id.org/pmd/mo/Cryo-ScanningElectronMicroscope
<https://w3id.org/pmd/mo/Cryo-ScanningElectronMicroscope> rdf:type owl:Class ;
                                                          rdfs:subClassOf <https://w3id.org/pmd/mo/ScanningElectronMicroscope> ;
                                                          rdfs:comment "A cryo-scanning electron microscope is typically used for imaging biological samples."@en ,
                                                                       "Ein Kryo-Rasterelektronenmikroskop wird in der Regel zur Abbildung biologischer Proben verwendet."@de ,
                                                                       "Eine Art Elektronenmikroskop, das bei kryogenen Temperaturen arbeitet."@de ;
                                                          rdfs:isDefinedBy <https://w3id.org/pmd/mo> ;
                                                          rdfs:label "Cryo Scanning Electron Microscope"@en ,
                                                                     "Kryo-Rasterelektronenmikroskop"@de ,
                                                                     "cryo-SEM"@en ;
                                                          <http://www.w3.org/2004/02/skos/core#definition> "A type of electron microscope that operates under cryogenic temperatures."@en ;
                                                          <https://w3id.org/pmd/co/definitionSource> "ChatGPT 3.5"@en .


###  https://w3id.org/pmd/mo/CryoElectronTomography
<https://w3id.org/pmd/mo/CryoElectronTomography> rdf:type owl:Class ;
                                                 rdfs:subClassOf <https://w3id.org/pmd/mo/ElectronTomography> ;
                                                 rdfs:isDefinedBy <https://w3id.org/pmd/mo> ;
                                                 rdfs:label "Cryo Electron Tomography"@en ,
                                                            "Kryo-Elektronentomographie"@de ;
                                                 <http://www.w3.org/2004/02/skos/core#definition> "Cryo Electron Tomography is a form of electron tomography that is performed at cryogenic temperatures. It is used to study the three-dimensional structure of frozen-hydrated samples."@en ;
                                                 <https://w3id.org/pmd/co/definitionSource> "ChatGPT 3.5"@en ;
                                                 <https://w3id.org/pmd/mo/abbreviation> "cryo-ET"@en .


###  https://w3id.org/pmd/mo/CryoTransmissionElectronMicroscope
<https://w3id.org/pmd/mo/CryoTransmissionElectronMicroscope> rdf:type owl:Class ;
                                                             rdfs:subClassOf <https://w3id.org/pmd/mo/TransmissionElectronMicroscope> ;
                                                             rdfs:isDefinedBy <https://w3id.org/pmd/mo> ;
                                                             rdfs:label "Cryo Transmission Electron Microscope"@en ,
                                                                        "Kryo-Transmissionselektronenmikroskop"@de ;
                                                             <http://www.w3.org/2004/02/skos/core#definition> "A transmission electron microscope that operates at cryogenic temperatures."@en ,
                                                                                                              "Ein Transmissionselektronenmikroskop, das bei kryogenen Temperaturen arbeitet."@de ;
                                                             <https://w3id.org/pmd/co/definitionSource> "ChatGPT 3.5"@en ;
                                                             <https://w3id.org/pmd/mo/abbreviation> "cryo-TEM"@en .


###  https://w3id.org/pmd/mo/Current
<https://w3id.org/pmd/mo/Current> rdf:type owl:Class ;
                                  rdfs:subClassOf <https://w3id.org/pmd/co/ValueObject> ;
                                  rdfs:comment "Der Strom wird normalerweise in Ampere (A) gemessen."@de ,
                                               "The current is typically measured in amperes (A)."@en ;
                                  rdfs:isDefinedBy <https://w3id.org/pmd/mo> ;
                                  rdfs:label "Current"@en ,
                                             "Strom"@de ;
                                  <http://www.w3.org/2004/02/skos/core#altLabel> "Stromstärke"@de ;
                                  <http://www.w3.org/2004/02/skos/core#definition> "Der Fluss der elektrischen Ladung."@de ,
                                                                                   "The flow of electric charge."@en ;
                                  <https://w3id.org/pmd/co/definitionSource> "ChatGPT 3.5"@en .


###  https://w3id.org/pmd/mo/Detector
<https://w3id.org/pmd/mo/Detector> rdf:type owl:Class ;
                                   rdfs:subClassOf <https://w3id.org/pmd/co/ProcessingNode> ;
                                   rdfs:isDefinedBy <https://w3id.org/pmd/mo> ;
                                   rdfs:label "Detector"@en ,
                                              "Detektor"@de ;
                                   <http://www.w3.org/2004/02/skos/core#definition> "A device used to detect and measure properties such as light, radiation, or particles."@en ,
                                                                                    "Ein Gerät zur Erkennung und Messung von Eigenschaften wie Licht, Strahlung oder Teilchen."@de ;
                                   <https://w3id.org/pmd/co/definitionSource> "ChatGPT 3.5"@en .


###  https://w3id.org/pmd/mo/DetectorQuantumEfficiency
<https://w3id.org/pmd/mo/DetectorQuantumEfficiency> rdf:type owl:Class ;
                                                    rdfs:subClassOf <https://w3id.org/pmd/mo/Efficiency> ;
                                                    rdfs:isDefinedBy <https://w3id.org/pmd/mo> ;
                                                    rdfs:label "Detector Quantum Efficiency"@en ,
                                                               "Detektor Quantenausbeute"@de ;
                                                    <http://www.w3.org/2004/02/skos/core#definition> "Die Effizienz, mit der ein Detektor einfallende Strahlung in Nutzsignale umwandelt."@de ,
                                                                                                     "The efficiency with which a detector converts incident radiation into useful signals."@en ;
                                                    <https://w3id.org/pmd/co/definitionSource> "ChatGPT 3.5"@en .


###  https://w3id.org/pmd/mo/Diffraction
<https://w3id.org/pmd/mo/Diffraction> rdf:type owl:Class ;
                                      rdfs:subClassOf <https://w3id.org/pmd/mo/PhysicalProcess> ;
                                      rdfs:isDefinedBy <https://w3id.org/pmd/mo> ;
                                      rdfs:label "Diffraction"@en ,
                                                 "Diffraktion"@de ;
                                      <http://www.w3.org/2004/02/skos/core#altLabel> "Beugung"@de ,
                                                                                     "Scattering"@en ;
                                      <http://www.w3.org/2004/02/skos/core#definition> "Die Biegung von Elektronenwellen beim Durchgang durch eine kristalline Probe, was zur Bildung von Beugungsmustern führt, die Informationen über die Kristallstruktur liefern."@de ,
                                                                                       "The bending of electron waves as they pass through a crystalline sample, resulting in the formation of diffraction patterns that provide information about the crystal structure."@en ;
                                      <https://w3id.org/pmd/co/definitionSource> "ChatGPT 3.5" .


###  https://w3id.org/pmd/mo/DiffractionPattern
<https://w3id.org/pmd/mo/DiffractionPattern> rdf:type owl:Class ;
                                             rdfs:subClassOf <https://w3id.org/pmd/co/DigitalEntity> ;
                                             rdfs:isDefinedBy <https://w3id.org/pmd/mo> ;
                                             rdfs:label "Beugungsmuster"@de ,
                                                        "Diffraction Pattern"@en ;
                                             <http://www.w3.org/2004/02/skos/core#definition> "Das Muster von Flecken oder Banden, das auf einem Detektor entsteht, wenn Elektronen nach der Wechselwirkung mit einer kristallinen Probe gebeugt werden."@de ,
                                                                                              "The pattern of spots or bands produced on a detector when electrons diffract after interacting with a crystalline sample."@en ;
                                             <https://w3id.org/pmd/co/definitionSource> "ChatGPT 3.5" .


###  https://w3id.org/pmd/mo/DiscAperture
<https://w3id.org/pmd/mo/DiscAperture> rdf:type owl:Class ;
                                       rdfs:subClassOf <https://w3id.org/pmd/mo/Aperture> ;
                                       rdfs:isDefinedBy <https://w3id.org/pmd/mo> ;
                                       rdfs:label "Disc Aperture"@en ,
                                                  "Scheibenblende"@de ;
                                       <http://www.w3.org/2004/02/skos/core#definition> "A circular aperture used to limit the beam size in an optical instrument."@en ,
                                                                                        "Eine kreisförmige Blende zur Begrenzung der Strahlgröße in einem optischen Instrument."@de ;
                                       <https://w3id.org/pmd/co/definitionSource> "ChatGPT 3.5"@en .


###  https://w3id.org/pmd/mo/DiskOfLeastConfusion
<https://w3id.org/pmd/mo/DiskOfLeastConfusion> rdf:type owl:Class ;
                                               rdfs:subClassOf <https://w3id.org/pmd/co/CrossSectionArea> ;
                                               rdfs:isDefinedBy <https://w3id.org/pmd/mo> ;
                                               rdfs:label "Disk Of Least Confusion"@en ,
                                                          "Scheibe der geringsten Konfusion"@de ;
                                               <http://www.w3.org/2004/02/skos/core#definition> "Der Bereich in der Bildebene eines Elektronenmikroskops, in dem der Elektronenstrahl auf die kleinste Punktgröße fokussiert wird, wodurch die durch sphärische Aberration verursachte Unschärfe minimiert wird."@de ,
                                                                                                "The region in the image plane of an electron microscope where the electron beam is focused to the smallest spot size, minimizing the blurring effect due to spherical aberration."@en ;
                                               <https://w3id.org/pmd/co/definitionSource> "ChatGPT 3.5" .


###  https://w3id.org/pmd/mo/DriftCorrection
<https://w3id.org/pmd/mo/DriftCorrection> rdf:type owl:Class ;
                                          rdfs:subClassOf <https://w3id.org/pmd/co/AnalysingProcess> ;
                                          <http://purl.obolibrary.org/obo/IAO_0000117> "PMDco Team"@en ;
                                          <http://purl.obolibrary.org/obo/IAO_0000119> "ChatGPT 3.5"@en ;
                                          rdfs:label "Drift Correction"@en ,
                                                     "Driftkorrektur"@de ;
                                          <http://www.w3.org/2004/02/skos/core#definition> "Drift Correction refers to techniques used in electron microscopy to compensate for the slow movement of the sample or beam, ensuring image stability and accuracy."@en ,
                                                                                           "Driftkorrektur bezieht sich auf Techniken in der Elektronenmikroskopie, die dazu dienen, die langsame Bewegung der Probe oder des Strahls auszugleichen und so Bildstabilität und Genauigkeit zu gewährleisten."@de .


###  https://w3id.org/pmd/mo/DwellTime
<https://w3id.org/pmd/mo/DwellTime> rdf:type owl:Class ;
                                    rdfs:subClassOf <https://w3id.org/pmd/co/Duration> ;
                                    rdfs:isDefinedBy <https://w3id.org/pmd/mo> ;
                                    rdfs:label "Dwell Time"@en ,
                                               "Verweilzeit"@de ;
                                    <http://www.w3.org/2004/02/skos/core#altLabel> "Verweildauer"@de ;
                                    <http://www.w3.org/2004/02/skos/core#definition> "Die Zeitspanne, in der der Elektronenstrahl während der Bildgebung oder Analyse auf einen bestimmten Punkt oder einen interessierenden Bereich der Probe fokussiert wird."@de ,
                                                                                     "The amount of time that the electron beam is focused on a specific point or region of interest on the specimen during imaging or analysis."@en ;
                                    <https://w3id.org/pmd/co/definitionSource> "ChatGPT 3.5" .


###  https://w3id.org/pmd/mo/DynamicFocusCorrection
<https://w3id.org/pmd/mo/DynamicFocusCorrection> rdf:type owl:Class ;
                                                 rdfs:subClassOf <https://w3id.org/pmd/co/AnalysingProcess> ;
                                                 rdfs:isDefinedBy <https://w3id.org/pmd/mo> ;
                                                 rdfs:label "Dynamic Focus Correction"@en ,
                                                            "Dynamische Fokuskorrektur"@de ;
                                                 <http://www.w3.org/2004/02/skos/core#definition> "A technique used in electron microscopy to continuously adjust the focus of the electron beam in real-time to maintain optimal image quality, especially when imaging uneven or rough surfaces."@en ,
                                                                                                  "Eine Technik, die in der Elektronenmikroskopie eingesetzt wird, um den Fokus des Elektronenstrahls kontinuierlich in Echtzeit anzupassen und so eine optimale Bildqualität zu erhalten, insbesondere bei der Abbildung unebener oder rauer Oberflächen."@de ;
                                                 <https://w3id.org/pmd/co/definitionSource> "ChatGPT 3.5" .


###  https://w3id.org/pmd/mo/DynamicRefocusing
<https://w3id.org/pmd/mo/DynamicRefocusing> rdf:type owl:Class ;
                                            rdfs:subClassOf <https://w3id.org/pmd/co/AnalysingProcess> ;
                                            rdfs:isDefinedBy <https://w3id.org/pmd/mo> ;
                                            rdfs:label "Dynamic Refocusing"@en ,
                                                       "Dynamische Refokussierung"@de ;
                                            <http://www.w3.org/2004/02/skos/core#definition> "Der Prozess, bei dem der Fokus des Elektronenstrahls während der Bildgebung angepasst wird, um Änderungen der Probenhöhe oder -topografie zu kompensieren und sicherzustellen, dass die gesamte Probe im Fokus bleibt."@de ,
                                                                                             "The process of adjusting the focus of the electron beam during imaging to compensate for changes in the specimen height or topography, ensuring that the entire specimen remains in focus."@en ;
                                            <https://w3id.org/pmd/co/definitionSource> "ChatGPT 3.5" .


###  https://w3id.org/pmd/mo/DynamicTransmissionElectronMicroscopy
<https://w3id.org/pmd/mo/DynamicTransmissionElectronMicroscopy> rdf:type owl:Class ;
                                                                rdfs:subClassOf <https://w3id.org/pmd/mo/TransmissionElectronMicroscopy> ;
                                                                rdfs:isDefinedBy <https://w3id.org/pmd/mo> ;
                                                                rdfs:label "Dynamic Transmission Electron Microscopy"@en ,
                                                                           "Dynamische Transmissionselektronenmikroskopie"@de ;
                                                                <http://www.w3.org/2004/02/skos/core#definition> "Dynamic Transmission Electron Microscopy is a technique that uses ultrafast electron pulses to capture rapid processes in materials with nanosecond to picosecond time resolution."@en ;
                                                                <https://w3id.org/pmd/co/definitionSource> "ChatGPT 3.5"@en ;
                                                                <https://w3id.org/pmd/mo/abbreviation> "DTEM"@en .


###  https://w3id.org/pmd/mo/Efficiency
<https://w3id.org/pmd/mo/Efficiency> rdf:type owl:Class ;
                                     rdfs:subClassOf <https://w3id.org/pmd/co/ValueObject> ;
                                     rdfs:isDefinedBy <https://w3id.org/pmd/mo> ;
                                     rdfs:label "Efficiency"@en ,
                                                "Effizienz"@de ;
                                     <http://www.w3.org/2004/02/skos/core#definition> "Das Verhältnis von nützlichem / nutzbarem Output zum gesamten Input in einem System."@de ,
                                                                                      "The ratio of useful output to total input in any system."@en ;
                                     <https://w3id.org/pmd/co/definitionSource> "ChatGPT 3.5"@en .


###  https://w3id.org/pmd/mo/Electrode
<https://w3id.org/pmd/mo/Electrode> rdf:type owl:Class ;
                                    rdfs:subClassOf <https://w3id.org/pmd/co/ProcessingNode> ;
                                    rdfs:isDefinedBy <https://w3id.org/pmd/mo> ;
                                    rdfs:label "Electrode"@en ,
                                               "Elektrode"@de ;
                                    <http://www.w3.org/2004/02/skos/core#definition> "An electrode is a conductor through which electric current enters or exits a substance. In the context of electrochemical systems, an electrode facilitates the transfer of electrons between a solid material and an electrolyte. Electrodes are essential components in batteries, fuel cells, electroplating, and other electrochemical processes. They play a critical role in facilitating chemical reactions and energy storage or conversion."@en ;
                                    <https://w3id.org/pmd/co/definitionSource> "ChatGPT 3.5"@en .


###  https://w3id.org/pmd/mo/ElectronBackscatterDiffraction
<https://w3id.org/pmd/mo/ElectronBackscatterDiffraction> rdf:type owl:Class ;
                                                         rdfs:subClassOf <https://w3id.org/pmd/mo/ElectronDiffraction> ;
                                                         rdfs:isDefinedBy <https://w3id.org/pmd/mo> ;
                                                         rdfs:label "Electron Backscatter Diffraction"@en ,
                                                                    "Rückstreuelektronenbeugung"@de ;
                                                         <http://www.w3.org/2004/02/skos/core#definition> "Electron Backscatter Diffraction is a microscopy technique used to analyze the crystallographic orientation and microstructure of materials. It involves directing an electron beam onto a sample's surface and measuring the backscattered electrons. By analyzing the diffraction patterns of these electrons, researchers can determine the crystallographic orientation of the material's grains."@en ;
                                                         <https://w3id.org/pmd/co/definitionSource> "ChatGPT 3.5"@en ;
                                                         <https://w3id.org/pmd/mo/abbreviation> "EBSD"@en .


###  https://w3id.org/pmd/mo/ElectronBeam
<https://w3id.org/pmd/mo/ElectronBeam> rdf:type owl:Class ;
                                       rdfs:subClassOf <https://w3id.org/pmd/mo/Beam> ;
                                       rdfs:isDefinedBy <https://w3id.org/pmd/mo> ;
                                       rdfs:label "Electron Beam"@en ,
                                                  "Elektronenstrahl"@de ;
                                       <http://www.w3.org/2004/02/skos/core#definition> "A stream of electrons emitted from an electron source and accelerated towards the specimen in an electron microscope for imaging or analysis."@en ,
                                                                                        "Ein Strom von Elektronen, der von einer Elektronenquelle emittiert und in einem Elektronenmikroskop zur Abbildung oder Analyse auf die Probe beschleunigt wird."@de ;
                                       <https://w3id.org/pmd/co/definitionSource> "ChatGPT 3.5" .


###  https://w3id.org/pmd/mo/ElectronChannelingContrastImaging
<https://w3id.org/pmd/mo/ElectronChannelingContrastImaging> rdf:type owl:Class ;
                                                            rdfs:subClassOf <https://w3id.org/pmd/mo/ScanningElectronMicroscopy> ;
                                                            rdfs:isDefinedBy <https://w3id.org/pmd/mo> ;
                                                            rdfs:label "Electron Channeling Contrast Imaging"@en ,
                                                                       "Elektronenkanal-Kontrastbildgebung"@de ;
                                                            <http://www.w3.org/2004/02/skos/core#definition> "Electron Channeling Contrast Imaging is a technique used in SEM or TEM to study crystallographic defects, such as dislocations, in crystalline materials. It utilizes the contrast resulting from the deviation of electron trajectories due to crystal defects."@en ;
                                                            <https://w3id.org/pmd/co/definitionSource> "ChatGPT 3.5"@en ;
                                                            <https://w3id.org/pmd/mo/abbreviation> "ECCI"@en .


###  https://w3id.org/pmd/mo/ElectronDiffraction
<https://w3id.org/pmd/mo/ElectronDiffraction> rdf:type owl:Class ;
                                              rdfs:subClassOf <https://w3id.org/pmd/mo/Diffraction> ;
                                              rdfs:isDefinedBy <https://w3id.org/pmd/mo> ;
                                              rdfs:label "Electron Diffraction"@en ,
                                                         "Elektronenbeugung"@de ;
                                              <http://www.w3.org/2004/02/skos/core#definition> "Das Phänomen der Beugung von Elektronenwellen beim Durchgang durch eine kristalline Probe, das Informationen über die Kristallstruktur liefert."@de ,
                                                                                               "The phenomenon of electron waves diffracting as they pass through a crystalline sample, providing information about the crystal structure."@en ;
                                              <https://w3id.org/pmd/co/definitionSource> "ChatGPT 3.5" .


###  https://w3id.org/pmd/mo/ElectronDiffractionPattern
<https://w3id.org/pmd/mo/ElectronDiffractionPattern> rdf:type owl:Class ;
                                                     rdfs:subClassOf <https://w3id.org/pmd/mo/DiffractionPattern> ;
                                                     rdfs:isDefinedBy <https://w3id.org/pmd/mo> ;
                                                     rdfs:label "Electron Diffraction Pattern"@en ,
                                                                "Elektronenbeugungsmuster"@de ;
                                                     <http://www.w3.org/2004/02/skos/core#definition> "Das Muster von Flecken oder Ringen, das auf einem Detektor entsteht, wenn Elektronen nach der Wechselwirkung mit einer kristallinen Probe gebeugt werden, und das zur Bestimmung der Kristallstruktur verwendet wird."@de ,
                                                                                                      "The pattern of spots or rings produced on a detector when electrons diffract after interacting with a crystalline sample, used to determine the crystal structure."@en ;
                                                     <https://w3id.org/pmd/co/definitionSource> "ChatGPT 3.5" .


###  https://w3id.org/pmd/mo/ElectronEnergyLossSpectrometer
<https://w3id.org/pmd/mo/ElectronEnergyLossSpectrometer> rdf:type owl:Class ;
                                                         owl:equivalentClass [ rdf:type owl:Restriction ;
                                                                               owl:onProperty <https://w3id.org/pmd/co/hasFunction> ;
                                                                               owl:someValuesFrom <https://w3id.org/pmd/mo/EnergyFilter>
                                                                             ] ,
                                                                             [ rdf:type owl:Restriction ;
                                                                               owl:onProperty <https://w3id.org/pmd/co/hasFunction> ;
                                                                               owl:someValuesFrom <https://w3id.org/pmd/mo/ImageFilter>
                                                                             ] ,
                                                                             [ rdf:type owl:Restriction ;
                                                                               owl:onProperty <https://w3id.org/pmd/co/relatesTo> ;
                                                                               owl:someValuesFrom <https://w3id.org/pmd/mo/CEOS-CEFIDfilter>
                                                                             ] ,
                                                                             [ rdf:type owl:Restriction ;
                                                                               owl:onProperty <https://w3id.org/pmd/co/relatesTo> ;
                                                                               owl:someValuesFrom <https://w3id.org/pmd/mo/GatanImageFilter>
                                                                             ] ;
                                                         rdfs:subClassOf <https://w3id.org/pmd/mo/Spectrometer> ;
                                                         <http://purl.obolibrary.org/obo/IAO_0000117> "PMDco Team"@en ;
                                                         <http://purl.obolibrary.org/obo/IAO_0000119> "ChatGPT 3.5"@en ;
                                                         rdfs:label "Electron Energy Loss Spectrometer"@en ,
                                                                    "Elektronen-Energieverlust-Spektrometer"@de ;
                                                         <http://www.w3.org/2004/02/skos/core#definition> "An Electron Energy Loss Spectrometer is a device used to measure the energy loss of electrons as they pass through a sample, providing information on the sample's composition and electronic structure."@en ,
                                                                                                          "Ein Elektronen-Energieverlust-Spektrometer ist ein Gerät, das verwendet wird, um den Energieverlust von Elektronen beim Durchgang durch eine Probe zu messen, was Informationen über die Zusammensetzung und die elektronische Struktur der Probe liefert."@de .


###  https://w3id.org/pmd/mo/ElectronEnergyLossSpectroscopy
<https://w3id.org/pmd/mo/ElectronEnergyLossSpectroscopy> rdf:type owl:Class ;
                                                         rdfs:subClassOf <https://w3id.org/pmd/mo/Spectroscopy> ;
                                                         rdfs:isDefinedBy <https://w3id.org/pmd/mo> ;
                                                         rdfs:label "Electron Energy Loss Spectroscopy"@en ,
                                                                    "Elektronenenergieverlustspektroskopie"@de ;
                                                         <http://www.w3.org/2004/02/skos/core#definition> """Electron Energy Loss Spectroscopy (EELS) is a specialized analytical technique in the field of materials science and electron microscopy. It involves the measurement of the energy loss of electrons as they interact with a sample. EELS is commonly performed in transmission electron microscopy (TEM) setups.
In EELS, a focused beam of high-energy electrons is directed at a sample. As these electrons pass through the material, they can lose energy through various interactions, such as inelastic scattering and excitation of inner-shell electrons. The energy loss is measured and analyzed to gain information about the sample's composition, electronic structure, and bonding characteristics.
By studying the energy loss spectrum, researchers can identify the types of atoms present in the sample, determine their chemical states, and gather insights into the electronic properties of the material. EELS is particularly useful for investigating nanoscale materials, thin films, and interfaces, providing valuable information about their electronic and atomic structure. It is a powerful technique for understanding the behavior of materials at the nanometer scale and plays a significant role in advancing fields such as materials science, nanotechnology, and semiconductor research."""@en ;
                                                         <https://w3id.org/pmd/co/definitionSource> "ChatGPT 3.5"@en ;
                                                         <https://w3id.org/pmd/mo/abbreviation> "EELS"@en .


###  https://w3id.org/pmd/mo/ElectronMicroprobe
<https://w3id.org/pmd/mo/ElectronMicroprobe> rdf:type owl:Class ;
                                             rdfs:subClassOf <https://w3id.org/pmd/co/ElectronMicroscope> ;
                                             rdfs:isDefinedBy <https://w3id.org/pmd/mo> ;
                                             rdfs:label "Electron Microprobe"@en ,
                                                        "Elektronenmikrosonde"@de ;
                                             <http://www.w3.org/2004/02/skos/core#definition> "An analytical instrument used to determine the chemical composition of materials."@en ,
                                                                                              "Ein Analyseinstrument zur Bestimmung der chemischen Zusammensetzung von Materialien."@de ;
                                             <https://w3id.org/pmd/co/definitionSource> "ChatGPT 3.5"@en .


###  https://w3id.org/pmd/mo/ElectronProbe
<https://w3id.org/pmd/mo/ElectronProbe> rdf:type owl:Class ;
                                        rdfs:subClassOf <https://w3id.org/pmd/mo/Beam> ;
                                        rdfs:isDefinedBy <https://w3id.org/pmd/mo> ;
                                        rdfs:label "Electron Probe"@en ,
                                                   "Elektronensonde"@de ;
                                        <http://www.w3.org/2004/02/skos/core#definition> "Der fokussierte Elektronenstrahl, der zur Abbildung oder Analyse in einem Elektronenmikroskop verwendet wird."@de ,
                                                                                         "The focused electron beam used for imaging or analysis in an electron microscope."@en ;
                                        <https://w3id.org/pmd/co/definitionSource> "ChatGPT 3.5" .


###  https://w3id.org/pmd/mo/ElectronProbeMicroAnalyzer
<https://w3id.org/pmd/mo/ElectronProbeMicroAnalyzer> rdf:type owl:Class ;
                                                     rdfs:subClassOf <https://w3id.org/pmd/mo/ElectronMicroprobe> ;
                                                     rdfs:isDefinedBy <https://w3id.org/pmd/mo> ;
                                                     rdfs:label "Electron Probe Micro Analyzer"@en ,
                                                                "Elektronensonden-Mikro-Analysator"@de ;
                                                     <http://www.w3.org/2004/02/skos/core#definition> "An instrument used for elemental analysis of solid materials by bombarding them with a focused electron beam."@en ,
                                                                                                      "Ein Instrument zur Elementaranalyse fester Materialien durch Beschuss mit einem fokussierten Elektronenstrahl."@de ;
                                                     <https://w3id.org/pmd/co/definitionSource> "ChatGPT 3.5"@en .


###  https://w3id.org/pmd/mo/ElectronTomograph
<https://w3id.org/pmd/mo/ElectronTomograph> rdf:type owl:Class ;
                                            rdfs:subClassOf <https://w3id.org/pmd/mo/TransmissionElectronMicroscope> ;
                                            rdfs:isDefinedBy <https://w3id.org/pmd/mo> ;
                                            rdfs:label "Electron Tomograph"@en ,
                                                       "Elektronentomograph"@de ;
                                            <http://www.w3.org/2004/02/skos/core#definition> "An instrument used for tomographic imaging using electrons."@en ,
                                                                                             "Ein Instrument für die tomografische Bildgebung mit Elektronen."@de ;
                                            <https://w3id.org/pmd/co/definitionSource> "ChatGPT 3.5"@en ;
                                            <https://w3id.org/pmd/mo/abbreviation> "ET"@en .


###  https://w3id.org/pmd/mo/ElectronTomography
<https://w3id.org/pmd/mo/ElectronTomography> rdf:type owl:Class ;
                                             rdfs:subClassOf <https://w3id.org/pmd/mo/TransmissionElectronMicroscopy> ;
                                             rdfs:isDefinedBy <https://w3id.org/pmd/mo> ;
                                             rdfs:label "Electron Tomography"@en ,
                                                        "Elektronentomographie"@de ;
                                             <http://www.w3.org/2004/02/skos/core#definition> "Electron Tomography is a technique that involves collecting a series of transmission electron microscopy (TEM) images from different angles to reconstruct a three-dimensional image of a sample."@en ;
                                             <https://w3id.org/pmd/co/definitionSource> "ChatGPT 3.5"@en ;
                                             <https://w3id.org/pmd/mo/abbreviation> "ET"@en .


###  https://w3id.org/pmd/mo/EmissionCurrent
<https://w3id.org/pmd/mo/EmissionCurrent> rdf:type owl:Class ;
                                          rdfs:subClassOf <https://w3id.org/pmd/mo/Current> ;
                                          rdfs:comment "Der Emissionsstrom wird normalerweise in Mikroampere (μA) oder Milliampere (mA) gemessen."@de ,
                                                       "The emission current usually measured in microamperes (μA) or milliamperes (mA)." ;
                                          rdfs:isDefinedBy <https://w3id.org/pmd/mo> ;
                                          rdfs:label "Emission Current"@en ,
                                                     "Emissionsstrom"@de ;
                                          <http://www.w3.org/2004/02/skos/core#definition> "Der Strom der von der Elektronenquelle emittierten Elektronen."@de ,
                                                                                           "The current of electrons emitted from the electron source."@en ;
                                          <https://w3id.org/pmd/co/definitionSource> "ChatGPT 3.5" .


###  https://w3id.org/pmd/mo/Energy
<https://w3id.org/pmd/mo/Energy> rdf:type owl:Class ;
                                 rdfs:subClassOf <https://w3id.org/pmd/co/ValueObject> ;
                                 rdfs:comment "Die Energie wird üblicherweise in Joule (J) oder Elektronenvolt (eV) gemessen."@de ,
                                              "The energy is usually measured in joules (J) or electron volts (eV)."@en ;
                                 rdfs:isDefinedBy <https://w3id.org/pmd/mo> ;
                                 rdfs:label "Energie"@de ,
                                            "Energy"@en ;
                                 <http://www.w3.org/2004/02/skos/core#definition> "Die Fähigkeit eines physischen Systems, Arbeit zu verrichten."@de ,
                                                                                  "The capacity of a physical system to perform work."@en ;
                                 <https://w3id.org/pmd/co/definitionSource> "ChatGPT 3.5"@en .


###  https://w3id.org/pmd/mo/EnergyDispersiveXRaySpectroscopy
<https://w3id.org/pmd/mo/EnergyDispersiveXRaySpectroscopy> rdf:type owl:Class ;
                                                           rdfs:subClassOf <https://w3id.org/pmd/mo/Spectroscopy> ,
                                                                           <https://w3id.org/pmd/mo/XRayMicroanalysis> ;
                                                           rdfs:isDefinedBy <https://w3id.org/pmd/mo> ;
                                                           rdfs:label "Energy Dispersive X-ray Spectroscopy"@en ;
                                                           <http://www.w3.org/2004/02/skos/core#altLabel> "energiedispersive Röntgenmikroanalyse"@de ;
                                                           <http://www.w3.org/2004/02/skos/core#definition> "Energy Dispersive X-ray Spectroscopy is a technique used to analyze the elemental composition of a sample by detecting the X-rays emitted when the sample is bombarded with electrons in an electron microscope or other instrument. EDS provides information about the elements present in the sample and their relative concentrations."@en ;
                                                           <http://www.w3.org/2004/02/skos/core#prefLabel> "energiedispersive Röntgenanalyse"@de ;
                                                           <https://w3id.org/pmd/co/definitionSource> "ChatGPT 3.5"@en ;
                                                           <https://w3id.org/pmd/mo/abbreviation> "EDS"@en ,
                                                                                                  "EDX"@en ,
                                                                                                  "XEDS"@en .


###  https://w3id.org/pmd/mo/EnergyFilter
<https://w3id.org/pmd/mo/EnergyFilter> rdf:type owl:Class ;
                                       rdfs:subClassOf <https://w3id.org/pmd/mo/OpticalElement> ;
                                       <http://purl.obolibrary.org/obo/IAO_0000117> "PMDco Team"@en ;
                                       <http://purl.obolibrary.org/obo/IAO_0000119> "ChatGPT 3.5"@en ;
                                       rdfs:label "Energie-Filter"@de ,
                                                  "Energy Filter"@en ;
                                       <http://www.w3.org/2004/02/skos/core#definition> "An Energy Filter is a device used in electron microscopy to filter electrons by their energy, improving image quality and enabling specific analytical techniques."@en ,
                                                                                        "Ein Energie-Filter ist ein Gerät, das in der Elektronenmikroskopie verwendet wird, um Elektronen nach ihrer Energie zu filtern, die Bildqualität zu verbessern und spezifische Analysetechniken zu ermöglichen."@de .


###  https://w3id.org/pmd/mo/EnergyFilteredTransmissionElectronMicroscope
<https://w3id.org/pmd/mo/EnergyFilteredTransmissionElectronMicroscope> rdf:type owl:Class ;
                                                                       rdfs:subClassOf <https://w3id.org/pmd/mo/TransmissionElectronMicroscope> ;
                                                                       rdfs:isDefinedBy <https://w3id.org/pmd/mo> ;
                                                                       rdfs:label "Energiegefiltertes Transmissionselektronenmikroskop"@de ,
                                                                                  "Energy-filtered Transmission Electron Microscope"@en ;
                                                                       <http://www.w3.org/2004/02/skos/core#definition> "A transmission electron microscope equipped with an energy filter to select electrons of specific energy levels."@en ,
                                                                                                                        "Ein Transmissionselektronenmikroskop, das mit einem Energiefilter ausgestattet ist, um Elektronen bestimmter Energieniveaus zu selektieren."@de ;
                                                                       <https://w3id.org/pmd/co/definitionSource> "ChatGPT 3.5"@en .


###  https://w3id.org/pmd/mo/EnergyLoss
<https://w3id.org/pmd/mo/EnergyLoss> rdf:type owl:Class ;
                                     rdfs:subClassOf <https://w3id.org/pmd/mo/Energy> ;
                                     rdfs:isDefinedBy <https://w3id.org/pmd/mo> ;
                                     rdfs:label "Energieverlust"@de ,
                                                "Energy Loss"@en ;
                                     <http://www.w3.org/2004/02/skos/core#definition> "Der Energieverlust, den ein Teilchen beim Durchgang durch ein Medium erfährt."@de ,
                                                                                      "The loss of energy experienced by a particle as it passes through a medium."@en ;
                                     <https://w3id.org/pmd/co/definitionSource> "ChatGPT 3.5"@en .


###  https://w3id.org/pmd/mo/EnergyResolution
<https://w3id.org/pmd/mo/EnergyResolution> rdf:type owl:Class ;
                                           rdfs:subClassOf <https://w3id.org/pmd/mo/Resolution> ;
                                           rdfs:isDefinedBy <https://w3id.org/pmd/mo> ;
                                           rdfs:label "Energieauflösung"@de ,
                                                      "Energy Resolution"@en ;
                                           <http://www.w3.org/2004/02/skos/core#definition> "Die Fähigkeit eines Detektors, zwischen verschiedenen Energieniveaus der einfallenden Strahlung zu unterscheiden."@de ,
                                                                                            "The ability of a detector to distinguish between different energy levels of incident radiation."@en ;
                                           <https://w3id.org/pmd/co/definitionSource> "ChatGPT 3.5"@en .


###  https://w3id.org/pmd/mo/EnvironmentalScanningElectronMicroscope
<https://w3id.org/pmd/mo/EnvironmentalScanningElectronMicroscope> rdf:type owl:Class ;
                                                                  rdfs:subClassOf <https://w3id.org/pmd/mo/ScanningElectronMicroscope> ;
                                                                  rdfs:isDefinedBy <https://w3id.org/pmd/mo> ;
                                                                  rdfs:label "Environmental Scanning Electron Microscope"@en ,
                                                                             "Umwelt-Rasterelektronenmikroskop"@de ;
                                                                  <http://www.w3.org/2004/02/skos/core#definition> "A type of electron microscope that can image non-conductive samples in their natural state."@en ,
                                                                                                                   "Eine Art Elektronenmikroskop, das nicht leitende Proben in ihrem natürlichen Zustand abbilden kann."@de ;
                                                                  <https://w3id.org/pmd/co/definitionSource> "ChatGPT 3.5"@en ;
                                                                  <https://w3id.org/pmd/mo/abbreviation> "ESEM"@en .


###  https://w3id.org/pmd/mo/EnvironmentalScanningElectronMicroscopy
<https://w3id.org/pmd/mo/EnvironmentalScanningElectronMicroscopy> rdf:type owl:Class ;
                                                                  rdfs:subClassOf <https://w3id.org/pmd/mo/ScanningElectronMicroscopy> ;
                                                                  rdfs:isDefinedBy <https://w3id.org/pmd/mo> ;
                                                                  rdfs:label "Environmental Scanning Electron Microscopy"@en ,
                                                                             "Umgebungs-Rasterelektronenmikroskopie"@de ;
                                                                  <http://www.w3.org/2004/02/skos/core#definition> "Environmental Scanning Electron Microscopy is a technique that allows imaging of samples in a gaseous environment. It is particularly useful for observing hydrated or non-conductive samples without the need for extensive sample preparation."@en ;
                                                                  <https://w3id.org/pmd/co/definitionSource> "ChatGPT 3.5"@en ;
                                                                  <https://w3id.org/pmd/mo/abbreviation> "ESEM"@en .


###  https://w3id.org/pmd/mo/EnvironmentalTransmissionElectronMicroscopy
<https://w3id.org/pmd/mo/EnvironmentalTransmissionElectronMicroscopy> rdf:type owl:Class ;
                                                                      rdfs:subClassOf <https://w3id.org/pmd/mo/TransmissionElectronMicroscopy> ;
                                                                      rdfs:isDefinedBy <https://w3id.org/pmd/mo> ;
                                                                      rdfs:label "Environmental Transmission Electron Microscopy"@en ,
                                                                                 "Umgebungs-Transmissionselektronenmikroskopie"@de ;
                                                                      <http://www.w3.org/2004/02/skos/core#definition> "Environmental Transmission Electron Microscopy allows imaging and analysis of materials in controlled gaseous environments, simulating real-world conditions."@en ;
                                                                      <https://w3id.org/pmd/co/definitionSource> "ChatGPT 3.5"@en ;
                                                                      <https://w3id.org/pmd/mo/abbreviation> "ETEM"@en .


###  https://w3id.org/pmd/mo/ExposureTime
<https://w3id.org/pmd/mo/ExposureTime> rdf:type owl:Class ;
                                       rdfs:subClassOf <https://w3id.org/pmd/co/Duration> ;
                                       rdfs:isDefinedBy <https://w3id.org/pmd/mo> ;
                                       rdfs:label "Belichtungszeit"@de ,
                                                  "Exposure Time"@en ;
                                       <http://www.w3.org/2004/02/skos/core#definition> "Die Dauer, während der der Bildsensor dem Licht ausgesetzt ist, gemessen in Sekunden (s)."@de ,
                                                                                        "The duration for which the imaging sensor is exposed to light, measured in seconds (s)."@en ;
                                       <https://w3id.org/pmd/co/definitionSource> "ChatGPT 3.5"@en .


###  https://w3id.org/pmd/mo/ExtractionVoltage
<https://w3id.org/pmd/mo/ExtractionVoltage> rdf:type owl:Class ;
                                            rdfs:subClassOf <https://w3id.org/pmd/mo/Voltage> ;
                                            rdfs:isDefinedBy <https://w3id.org/pmd/mo> ;
                                            rdfs:label "Extraction Voltage"@en ,
                                                       "Extraktionsspannung"@de ;
                                            <http://www.w3.org/2004/02/skos/core#definition> "Die Spannung, die an die Elektronenquelle in einem Elektronenmikroskop angelegt wird, um Elektronen aus der Kathode zu extrahieren und sie auf die Probe zu beschleunigen."@de ,
                                                                                             "The voltage applied to the electron source in an electron microscope to extract electrons from the cathode and accelerate them towards the specimen."@en ;
                                            <https://w3id.org/pmd/co/definitionSource> "ChatGPT 3.5" .


###  https://w3id.org/pmd/mo/FieldEmissionGun
<https://w3id.org/pmd/mo/FieldEmissionGun> rdf:type owl:Class ;
                                           rdfs:subClassOf <https://w3id.org/pmd/mo/Gun> ;
                                           rdfs:isDefinedBy <https://w3id.org/pmd/mo> ;
                                           rdfs:label "Feldemissionskanone"@de ,
                                                      "Field Emission Gun"@en ;
                                           <http://www.w3.org/2004/02/skos/core#definition> "A Field Emission Gun is an electron gun used in electron microscopes to produce an electron beam with extremely high brightness and coherence. It relies on the phenomenon of field emission, where electrons are emitted from a sharp emitter tip under the influence of a strong electric field. FEGs are capable of producing highly focused electron beams, leading to enhanced imaging resolution and analytical capabilities."@en ;
                                           <https://w3id.org/pmd/co/definitionSource> "ChatGPT 3.5"@en ;
                                           <https://w3id.org/pmd/mo/abbreviation> "FEG"@en .


###  https://w3id.org/pmd/mo/FieldEmissionScanningElectronMicroscopy
<https://w3id.org/pmd/mo/FieldEmissionScanningElectronMicroscopy> rdf:type owl:Class ;
                                                                  rdfs:subClassOf <https://w3id.org/pmd/mo/ScanningElectronMicroscopy> ;
                                                                  rdfs:isDefinedBy <https://w3id.org/pmd/mo> ;
                                                                  rdfs:label "Feldemissions-Rasterelektronenmikroskopie"@de ,
                                                                             "Field Emission Scanning Electron Microscopy"@en ;
                                                                  <http://www.w3.org/2004/02/skos/core#definition> "Field Emission Scanning Electron Microscopy is an advanced form of SEM that uses a field emitter to produce a highly focused electron beam, enabling high-resolution imaging and surface analysis."@en ;
                                                                  <https://w3id.org/pmd/co/definitionSource> "ChatGPT 3.5"@en ;
                                                                  <https://w3id.org/pmd/mo/abbreviation> "FESEM"@en .


###  https://w3id.org/pmd/mo/FieldIonMicroscope
<https://w3id.org/pmd/mo/FieldIonMicroscope> rdf:type owl:Class ;
                                             rdfs:subClassOf <https://w3id.org/pmd/mo/IonMicroscope> ;
                                             rdfs:isDefinedBy <https://w3id.org/pmd/mo> ;
                                             rdfs:label "Feldionenmikroskop"@de ,
                                                        "Field Ion Microscope"@en ;
                                             <http://www.w3.org/2004/02/skos/core#definition> "A type of microscope that uses the phenomenon of field ionization to image surfaces with atomic resolution."@en ,
                                                                                              "Ein Mikroskoptyp, der das Phänomen der Feldionisation nutzt, um Oberflächen mit atomarer Auflösung abzubilden."@de ;
                                             <https://w3id.org/pmd/co/definitionSource> "ChatGPT 3.5"@en ;
                                             <https://w3id.org/pmd/mo/abbreviation> "FIM"@en .


###  https://w3id.org/pmd/mo/FieldIonMicroscopy
<https://w3id.org/pmd/mo/FieldIonMicroscopy> rdf:type owl:Class ;
                                             rdfs:subClassOf <https://w3id.org/pmd/mo/IonMicroscopy> ;
                                             rdfs:isDefinedBy <https://w3id.org/pmd/mo> ;
                                             rdfs:label "Feldionenmikroskopie"@de ,
                                                        "Field Ion Microscopy"@en ;
                                             <http://www.w3.org/2004/02/skos/core#definition> "Field Ion Microscopy is a specialized microscopy technique that uses a strong electric field to ionize atoms on the surface of a metal sample. These ionized atoms are then repelled from the surface and can be detected to create an image of the sample's surface topography at atomic resolution. FIM is especially powerful for imaging the arrangement of atoms on metallic surfaces."@en ;
                                             <https://w3id.org/pmd/co/definitionSource> "ChatGPT 3.5"@en ;
                                             <https://w3id.org/pmd/mo/abbreviation> "FIM"@en .


###  https://w3id.org/pmd/mo/FieldWidth
<https://w3id.org/pmd/mo/FieldWidth> rdf:type owl:Class ;
                                     rdfs:subClassOf <https://w3id.org/pmd/co/Width> ;
                                     <http://purl.obolibrary.org/obo/IAO_0000117> "PMDco Team"@en ;
                                     <http://purl.obolibrary.org/obo/IAO_0000119> "ChatGPT 3.5"@en ;
                                     rdfs:label "Feldbreite"@de ,
                                                "Field Width"@en ;
                                     <http://www.w3.org/2004/02/skos/core#definition> "Feldbreite bezieht sich auf den horizontalen Umfang des beobachtbaren Feldes in einem Elektronenmikroskop."@de ,
                                                                                      "Field Width refers to the horizontal extent of the observable field in an electron microscope."@en .


###  https://w3id.org/pmd/mo/Filament
<https://w3id.org/pmd/mo/Filament> rdf:type owl:Class ;
                                   rdfs:subClassOf <https://w3id.org/pmd/co/Component> ;
                                   rdfs:isDefinedBy <https://w3id.org/pmd/mo> ;
                                   rdfs:label "Filament"@de ,
                                              "Filament"@en ;
                                   <http://www.w3.org/2004/02/skos/core#definition> "A thin wire or thread that emits electrons when heated in a vacuum tube or electron microscope."@en ,
                                                                                    "Ein dünner Draht oder Faden, der Elektronen emittiert, wenn er in einer Vakuumröhre oder einem Elektronenmikroskop erhitzt wird."@de ;
                                   <https://w3id.org/pmd/co/definitionSource> "ChatGPT 3.5"@en .


###  https://w3id.org/pmd/mo/FilamentCurrent
<https://w3id.org/pmd/mo/FilamentCurrent> rdf:type owl:Class ;
                                          rdfs:subClassOf <https://w3id.org/pmd/mo/Current> ;
                                          rdfs:isDefinedBy <https://w3id.org/pmd/mo> ;
                                          rdfs:label "Filament Current"@en ,
                                                     "Glühfadenstrom"@de ;
                                          <http://www.w3.org/2004/02/skos/core#definition> "Der Strom, der durch den Glühfaden der Elektronenkanone in einem Elektronenmikroskop fließt und den Glühfaden erhitzt, um Elektronen zu emittieren."@de ,
                                                                                           "The current passing through the filament of the electron gun in an electron microscope, which heats up the filament to emit electrons."@en ;
                                          <https://w3id.org/pmd/co/definitionSource> "ChatGPT 3.5" .


###  https://w3id.org/pmd/mo/FluorescenceMicroscopy
<https://w3id.org/pmd/mo/FluorescenceMicroscopy> rdf:type owl:Class ;
                                                 rdfs:subClassOf <https://w3id.org/pmd/mo/LightMicroscopy> ;
                                                 rdfs:isDefinedBy <https://w3id.org/pmd/mo> ;
                                                 rdfs:label "Fluorescence Microscopy"@en ,
                                                            "Fluoreszenzmikroskopie"@de ;
                                                 <http://www.w3.org/2004/02/skos/core#definition> "Fluorescence Microscopy is an optical imaging technique used to visualize biological structures and molecules that fluoresce when illuminated with specific wavelengths of light. Fluorescent molecules absorb light energy and then emit light of a longer wavelength, allowing the visualization of specific molecules or cellular components. Fluorescence microscopy is widely used in cell biology, molecular biology, and medical research."@en ;
                                                 <https://w3id.org/pmd/co/definitionSource> "ChatGPT 3.5"@en .


###  https://w3id.org/pmd/mo/FlybackTime
<https://w3id.org/pmd/mo/FlybackTime> rdf:type owl:Class ;
                                      rdfs:subClassOf <https://w3id.org/pmd/co/Duration> ;
                                      rdfs:isDefinedBy <https://w3id.org/pmd/mo> ;
                                      rdfs:label "Flyback Time"@en ,
                                                 "Rücklaufzeit"@de ;
                                      <http://www.w3.org/2004/02/skos/core#definition> "Die Zeit, die der Elektronenstrahl benötigt, um nach dem Abtasten einer Zeile oder eines Bildes in einem Elektronenmikroskop in seine Ausgangsposition zurückzukehren."@de ,
                                                                                       "The time taken for the electron beam to return to its starting position after scanning a line or frame in an electron microscope."@en ;
                                      <https://w3id.org/pmd/co/definitionSource> "ChatGPT 3.5" .


###  https://w3id.org/pmd/mo/FocalLength
<https://w3id.org/pmd/mo/FocalLength> rdf:type owl:Class ;
                                      rdfs:subClassOf <https://w3id.org/pmd/co/Length> ;
                                      rdfs:isDefinedBy <https://w3id.org/pmd/mo> ;
                                      rdfs:label "Brennweite"@de ,
                                                 "Focal Length"@en ;
                                      <http://www.w3.org/2004/02/skos/core#definition> "Der Abstand zwischen dem Brennpunkt (wo der Elektronenstrahl fokussiert wird) und der Linse oder Blende in einem Elektronenmikroskop."@de ,
                                                                                       "The distance between the focal point (where the electron beam is focused) and the lens or aperture in an electron microscope."@en ;
                                      <https://w3id.org/pmd/co/definitionSource> "ChatGPT 3.5" .


###  https://w3id.org/pmd/mo/FocalPlane
<https://w3id.org/pmd/mo/FocalPlane> rdf:type owl:Class ;
                                     rdfs:subClassOf <https://w3id.org/pmd/co/Area> ;
                                     rdfs:isDefinedBy <https://w3id.org/pmd/mo> ;
                                     rdfs:label "Brennebene"@de ,
                                                "Focal Plane"@en ;
                                     <http://www.w3.org/2004/02/skos/core#definition> "Die Ebene senkrecht zur optischen Achse eines Elektronenmikroskops, in der der Elektronenstrahl fokussiert wird, um ein Bild zu erzeugen."@de ,
                                                                                      "The plane perpendicular to the optical axis of an electron microscope where the electron beam is focused to form an image."@en ;
                                     <https://w3id.org/pmd/co/definitionSource> "ChatGPT 3.5" .


###  https://w3id.org/pmd/mo/FocalPoint
<https://w3id.org/pmd/mo/FocalPoint> rdf:type owl:Class ;
                                     rdfs:subClassOf <https://w3id.org/pmd/co/DigitalEntity> ;
                                     rdfs:isDefinedBy <https://w3id.org/pmd/mo> ;
                                     rdfs:label "Brennpunkt"@de ,
                                                "Focal Point"@en ;
                                     <http://www.w3.org/2004/02/skos/core#definition> "Der Punkt, an dem der Elektronenstrahl in einem Elektronenmikroskop fokussiert wird, um ein Bild der Probe zu erzeugen."@de ,
                                                                                      "The point at which the electron beam is focused in an electron microscope to form an image of the specimen."@en ;
                                     <https://w3id.org/pmd/co/definitionSource> "ChatGPT 3.5" .


###  https://w3id.org/pmd/mo/FocusedBeam
<https://w3id.org/pmd/mo/FocusedBeam> rdf:type owl:Class ;
                                      rdfs:subClassOf <https://w3id.org/pmd/mo/Beam> ;
                                      rdfs:isDefinedBy <https://w3id.org/pmd/mo> ;
                                      rdfs:label "Focused Beam"@en ,
                                                 "Fokussierter Strahl"@de ;
                                      <http://www.w3.org/2004/02/skos/core#definition> "An electron beam that has been narrowed or focused to a small spot size on the specimen surface."@en ,
                                                                                       "Ein Elektronenstrahl, der auf einen kleinen Punkt auf der Probenoberfläche eingeengt oder fokussiert wurde."@de ;
                                      <https://w3id.org/pmd/co/definitionSource> "ChatGPT 3.5" .


###  https://w3id.org/pmd/mo/FocusedIonBeam-ScanningElectronMicroscope
<https://w3id.org/pmd/mo/FocusedIonBeam-ScanningElectronMicroscope> rdf:type owl:Class ;
                                                                    rdfs:subClassOf <https://w3id.org/pmd/mo/IonMicroscope> ;
                                                                    rdfs:isDefinedBy <https://w3id.org/pmd/mo> ;
                                                                    rdfs:label "Focus(ed) Ion Beam - Scanning Electron Microscope"@en ,
                                                                               "Fokussierter Ionenstrahl - Rasterelektronenmikroskop"@de ;
                                                                    <http://www.w3.org/2004/02/skos/core#definition> "A dual-beam microscope that combines a focused ion beam with a scanning electron microscope."@en ,
                                                                                                                     "Ein Zweistrahlmikroskop, das einen fokussierten Ionenstrahl mit einem Rasterelektronenmikroskop kombiniert."@de ;
                                                                    <https://w3id.org/pmd/co/definitionSource> "ChatGPT 3.5"@en ;
                                                                    <https://w3id.org/pmd/mo/abbreviation> "FIB-SEM"@en .


###  https://w3id.org/pmd/mo/FocusedIonBeamScanningElectronMicroscopy
<https://w3id.org/pmd/mo/FocusedIonBeamScanningElectronMicroscopy> rdf:type owl:Class ;
                                                                   rdfs:subClassOf <https://w3id.org/pmd/mo/IonMicroscopy> ;
                                                                   rdfs:isDefinedBy <https://w3id.org/pmd/mo> ;
                                                                   rdfs:label "Focused Ion Beam Scanning Electron Microscopy"@en ,
                                                                              "Fokussierte Ionenstrahl-Rasterelektronenmikroskopie"@de ;
                                                                   <http://www.w3.org/2004/02/skos/core#definition> "Focused Ion Beam Scanning Electron Microscopy is a combination of two techniques: focused ion beam (FIB) and scanning electron microscopy (SEM). FIB-SEM systems use a focused ion beam to both image and modify a sample's surface. The ion beam can be used for milling, cutting, and deposition processes, making FIB-SEM a versatile tool for materials analysis, sample preparation, and three-dimensional imaging."@en ;
                                                                   <https://w3id.org/pmd/co/definitionSource> "ChatGPT 3.5"@en ;
                                                                   <https://w3id.org/pmd/mo/abbreviation> "FIB-SEM"@en .


###  https://w3id.org/pmd/mo/FourierTransformInfraredSpectroscopy
<https://w3id.org/pmd/mo/FourierTransformInfraredSpectroscopy> rdf:type owl:Class ;
                                                               rdfs:subClassOf <https://w3id.org/pmd/mo/Spectroscopy> ;
                                                               rdfs:isDefinedBy <https://w3id.org/pmd/mo> ;
                                                               rdfs:label "Fourier Transform Infrared Spectroscopy"@en ,
                                                                          "Fourier-Transformations-Infrarotspektroskopie"@de ;
                                                               <http://www.w3.org/2004/02/skos/core#definition> """Fourier Transform Infrared Spectroscopy (FTIR) is a powerful analytical technique used in various scientific disciplines to study the molecular composition and properties of materials. It is based on the interaction between infrared radiation and a sample, providing information about the vibrational modes of molecules.
In FTIR spectroscopy, an infrared beam is directed through a sample, and the interaction between the radiation and the sample's molecules leads to absorption of specific infrared frequencies. Each type of molecular bond and functional group in the sample absorbs infrared radiation at characteristic frequencies, which correspond to the energies of molecular vibrations. The resulting absorption spectrum represents a fingerprint of the sample's molecular structure.
The Fourier transform technique is used to convert the raw data obtained from the absorption measurements into a Fourier-transformed spectrum. This transformation improves the signal-to-noise ratio and enhances the accuracy of spectral analysis.
FTIR is extensively used in a wide range of fields, including chemistry, biology, materials science, pharmaceuticals, and environmental science. It is employed for qualitative and quantitative analysis, identification of compounds, monitoring chemical reactions, and studying molecular interactions. FTIR spectroscopy provides valuable insights into molecular bonding, functional groups, and the chemical composition of substances, making it an indispensable tool in modern analytical science."""@en ;
                                                               <https://w3id.org/pmd/co/definitionSource> "ChatGPT 3.5"@en ;
                                                               <https://w3id.org/pmd/mo/abbreviation> "FTIR"@en .


###  https://w3id.org/pmd/mo/Frame
<https://w3id.org/pmd/mo/Frame> rdf:type owl:Class ;
                                rdfs:subClassOf <https://w3id.org/pmd/co/DigitalEntity> ;
                                rdfs:isDefinedBy <https://w3id.org/pmd/mo> ;
                                rdfs:label "Bildrahmen"@de ,
                                           "Frame"@en ;
                                <http://www.w3.org/2004/02/skos/core#definition> "A single image or capture in a sequence of images."@en ,
                                                                                 "Ein einzelnes Bild oder eine Aufnahme in einer Bildsequenz."@de ;
                                <https://w3id.org/pmd/co/definitionSource> "ChatGPT 3.5"@en .


###  https://w3id.org/pmd/mo/FrameCount
<https://w3id.org/pmd/mo/FrameCount> rdf:type owl:Class ;
                                     rdfs:subClassOf <https://w3id.org/pmd/co/ValueObject> ;
                                     rdfs:isDefinedBy <https://w3id.org/pmd/mo> ;
                                     rdfs:label "Bildanzahl"@de ,
                                                "Frame Count"@en ;
                                     <http://www.w3.org/2004/02/skos/core#definition> "Die Gesamtanzahl der Bilder oder Aufnahmen in einer Sequenz."@de ,
                                                                                      "The total number of frames or images in a sequence."@en ;
                                     <https://w3id.org/pmd/co/definitionSource> "ChatGPT 3.5"@en .


###  https://w3id.org/pmd/mo/FrameTime
<https://w3id.org/pmd/mo/FrameTime> rdf:type owl:Class ;
                                    rdfs:subClassOf <https://w3id.org/pmd/co/Duration> ;
                                    rdfs:isDefinedBy <https://w3id.org/pmd/mo> ;
                                    rdfs:label "Frame Time"@en ,
                                               "Rahmenscanzeit"@de ;
                                    <http://www.w3.org/2004/02/skos/core#definition> "Die Zeit, die benötigt wird, um ein Einzelbild in einem Elektronenmikroskop aufzunehmen und anzuzeigen."@de ,
                                                                                     "The time required to capture and display a single frame of an image in an electron microscope."@en ;
                                    <https://w3id.org/pmd/co/definitionSource> "ChatGPT 3.5" .


###  https://w3id.org/pmd/mo/Gamma
<https://w3id.org/pmd/mo/Gamma> rdf:type owl:Class ;
                                rdfs:subClassOf <https://w3id.org/pmd/co/ValueObject> ;
                                rdfs:isDefinedBy <https://w3id.org/pmd/mo> ;
                                rdfs:label "Gamma"@de ,
                                           "Gamma"@en ;
                                <http://www.w3.org/2004/02/skos/core#definition> "The nonlinear operation used to encode and decode luminance or color values in an image."@en ;
                                <https://w3id.org/pmd/co/definitionSource> "ChatGPT 3.5"@en .


###  https://w3id.org/pmd/mo/GatanImageFilter
<https://w3id.org/pmd/mo/GatanImageFilter> rdf:type owl:Class ;
                                           rdfs:subClassOf <https://w3id.org/pmd/mo/EnergyFilter> ,
                                                           <https://w3id.org/pmd/mo/ImageFilter> ;
                                           rdfs:isDefinedBy <https://w3id.org/pmd/mo> ;
                                           rdfs:label "Gatan Abbildungsfilter"@de ,
                                                      "Gatan Image Filter"@en ;
                                           <http://www.w3.org/2004/02/skos/core#definition> "A Gatan Image Filter refers to an image filter manufactured by Gatan, Inc., a company specializing in electron microscopy and related products. Gatan's image filters are designed for electron microscopes and electron energy loss spectroscopy (EELS) applications. These filters allow researchers to control and enhance the acquisition of electron energy loss spectra while obtaining high-resolution images of the sample under investigation."@en ;
                                           <https://w3id.org/pmd/co/definitionSource> "ChatGPT 3.5"@en .


###  https://w3id.org/pmd/mo/GridVoltage
<https://w3id.org/pmd/mo/GridVoltage> rdf:type owl:Class ;
                                      rdfs:subClassOf <https://w3id.org/pmd/mo/Voltage> ;
                                      <http://purl.obolibrary.org/obo/IAO_0000117> "PMDco Team"@en ;
                                      <http://purl.obolibrary.org/obo/IAO_0000119> "ChatGPT 3.5"@en ;
                                      rdfs:label "Gitterspannung"@de ,
                                                 "Grid Voltage"@en ;
                                      <http://www.w3.org/2004/02/skos/core#definition> "Gitterspannung bezieht sich auf die Spannung, die an das Steuergitter in einem Elektronenmikroskop angelegt wird und die den Fokus und die Intensität des Elektronenstrahls beeinflusst."@de ,
                                                                                       "Grid Voltage refers to the voltage applied to the control grid in an electron microscope, which influences the electron beam's focus and intensity."@en .


###  https://w3id.org/pmd/mo/Gun
<https://w3id.org/pmd/mo/Gun> rdf:type owl:Class ;
                              owl:equivalentClass [ rdf:type owl:Restriction ;
                                                    owl:onProperty <https://w3id.org/pmd/co/component> ;
                                                    owl:someValuesFrom <https://w3id.org/pmd/mo/Source>
                                                  ] ;
                              rdfs:subClassOf <https://w3id.org/pmd/co/ProcessingNode> ;
                              rdfs:isDefinedBy <https://w3id.org/pmd/mo> ;
                              rdfs:label "Gun"@en ,
                                         "Kanone"@de ;
                              <http://www.w3.org/2004/02/skos/core#definition> "In the context of electron microscopy and particle acceleration, a \"gun\" typically refers to an electron or particle source that generates and emits the particles. In electron microscopy, an electron gun is used to generate a beam of electrons for imaging or analysis. In particle accelerators, a particle gun generates and launches particles at high speeds for various experimental purposes."@en ;
                              <https://w3id.org/pmd/co/definitionSource> "ChatGPT 3.5"@en .


###  https://w3id.org/pmd/mo/GunVacuum
<https://w3id.org/pmd/mo/GunVacuum> rdf:type owl:Class ;
                                    rdfs:subClassOf <https://w3id.org/pmd/mo/Vacuum> ;
                                    rdfs:isDefinedBy <https://w3id.org/pmd/mo> ;
                                    rdfs:label "Gun Vacuum"@en ,
                                               "Kanonen-Vakuum"@de ;
                                    <http://www.w3.org/2004/02/skos/core#definition> "Das Vakuumniveau im Inneren der Elektronenkanone eines Elektronenmikroskops."@de ,
                                                                                     "The vacuum level inside the electron gun of an electron microscope."@en ;
                                    <https://w3id.org/pmd/co/definitionSource> "ChatGPT 3.5"@en .


###  https://w3id.org/pmd/mo/HeliumIonMicroscope
<https://w3id.org/pmd/mo/HeliumIonMicroscope> rdf:type owl:Class ;
                                              rdfs:subClassOf <https://w3id.org/pmd/mo/FocusedIonBeam-ScanningElectronMicroscope> ;
                                              rdfs:isDefinedBy <https://w3id.org/pmd/mo> ;
                                              rdfs:label "Helium Ion Microscope"@en ,
                                                         "Helium-Ionen-Mikroskop"@de ;
                                              <http://www.w3.org/2004/02/skos/core#definition> "A type of microscope that uses helium ions to image samples with high resolution."@en ,
                                                                                               "Eine Art Mikroskop, das Helium-Ionen verwendet, um Proben mit hoher Auflösung abzubilden."@de ;
                                              <https://w3id.org/pmd/co/definitionSource> "ChatGPT 3.5"@en ;
                                              <https://w3id.org/pmd/mo/abbreviation> "HIM"@en .


###  https://w3id.org/pmd/mo/HeliumIonMicroscopy
<https://w3id.org/pmd/mo/HeliumIonMicroscopy> rdf:type owl:Class ;
                                              rdfs:subClassOf <https://w3id.org/pmd/mo/IonMicroscopy> ;
                                              rdfs:isDefinedBy <https://w3id.org/pmd/mo> ;
                                              rdfs:label "Helium Ion Microscopy"@en ,
                                                         "Helium-Ionen-Mikroskopie"@de ;
                                              <http://www.w3.org/2004/02/skos/core#definition> "Helium Ion Microscopy is a microscopy technique that uses a beam of helium ions instead of electrons to interact with a sample's surface. The smaller mass of helium ions compared to electrons allows for higher resolution imaging and reduced sample damage. HIM provides high-resolution images and is often used for imaging delicate or sensitive samples."@en ;
                                              <https://w3id.org/pmd/co/definitionSource> "ChatGPT 3.5"@en ;
                                              <https://w3id.org/pmd/mo/abbreviation> "HIM"@en .


###  https://w3id.org/pmd/mo/HighAngleAnnularDarkFieldScanningTransmissionElectronMicroscope
<https://w3id.org/pmd/mo/HighAngleAnnularDarkFieldScanningTransmissionElectronMicroscope> rdf:type owl:Class ;
                                                                                          rdfs:subClassOf <https://w3id.org/pmd/mo/ScanningTransmissionElectronMicroscope> ;
                                                                                          rdfs:isDefinedBy <https://w3id.org/pmd/mo> ;
                                                                                          rdfs:label "High-angle Annular Dark-field Scanning Transmission Electron Microscope"@en ,
                                                                                                     "Hochwinkel-Dunkelfeld-Rastertransmissionselektronenmikroskop mit annularem Winkel"@de ;
                                                                                          <http://www.w3.org/2004/02/skos/core#definition> "A type of scanning transmission electron microscope that detects scattered electrons at high angles."@en ,
                                                                                                                                           "Eine Art Rastertransmissionselektronenmikroskop, das gestreute Elektronen in hohen Winkeln erkennt."@de ;
                                                                                          <https://w3id.org/pmd/co/definitionSource> "ChatGPT 3.5"@en ;
                                                                                          <https://w3id.org/pmd/mo/abbreviation> "HAADF-STEM"@en .


###  https://w3id.org/pmd/mo/HighResolutionTransmissionElectronMicroscope
<https://w3id.org/pmd/mo/HighResolutionTransmissionElectronMicroscope> rdf:type owl:Class ;
                                                                       rdfs:subClassOf <https://w3id.org/pmd/mo/TransmissionElectronMicroscope> ;
                                                                       rdfs:isDefinedBy <https://w3id.org/pmd/mo> ;
                                                                       rdfs:label "High Resolution Transmission Electron Microscope"@en ,
                                                                                  "Hochauflösendes Transmissionselektronenmikroskop"@de ;
                                                                       <http://www.w3.org/2004/02/skos/core#definition> "A transmission electron microscope capable of achieving high-resolution images."@en ,
                                                                                                                        "Ein Transmissionselektronenmikroskop, das hochauflösende Bilder liefert."@de ;
                                                                       <https://w3id.org/pmd/co/definitionSource> "ChatGPT 3.5"@en ;
                                                                       <https://w3id.org/pmd/mo/abbreviation> "HRTEM"@en .


###  https://w3id.org/pmd/mo/HighResolutionTransmissionElectronMicroscopy
<https://w3id.org/pmd/mo/HighResolutionTransmissionElectronMicroscopy> rdf:type owl:Class ;
                                                                       rdfs:subClassOf <https://w3id.org/pmd/mo/TransmissionElectronMicroscopy> ;
                                                                       rdfs:isDefinedBy <https://w3id.org/pmd/mo> ;
                                                                       rdfs:label "High Resolution Transmission Electron Microscopy"@en ,
                                                                                  "Hochauflösende Transmissionselektronenmikroskopie"@de ;
                                                                       <http://www.w3.org/2004/02/skos/core#definition> "High Resolution TEM is a technique that provides exceptionally high-resolution images of a sample's internal structure, revealing atomic-level details."@en ;
                                                                       <https://w3id.org/pmd/co/definitionSource> "ChatGPT 3.5"@en ;
                                                                       <https://w3id.org/pmd/mo/abbreviation> "HRTEM"@en .


###  https://w3id.org/pmd/mo/Holder
<https://w3id.org/pmd/mo/Holder> rdf:type owl:Class ;
                                 rdfs:subClassOf <https://w3id.org/pmd/co/Component> ;
                                 rdfs:isDefinedBy <https://w3id.org/pmd/mo> ;
                                 rdfs:label "Halter"@de ,
                                            "Holder"@en ;
                                 <http://www.w3.org/2004/02/skos/core#definition> "A device used to support or secure a specimen or component in place."@en ,
                                                                                  "Ein Gerät, das verwendet wird, um eine Probe oder ein Bauteil zu stützen oder zu sichern."@de ;
                                 <https://w3id.org/pmd/co/definitionSource> "ChatGPT 3.5"@en .


###  https://w3id.org/pmd/mo/HorizontalFieldWidth
<https://w3id.org/pmd/mo/HorizontalFieldWidth> rdf:type owl:Class ;
                                               rdfs:subClassOf <https://w3id.org/pmd/mo/FieldWidth> ;
                                               <http://purl.obolibrary.org/obo/IAO_0000117> "PMDco Team"@en ;
                                               <http://purl.obolibrary.org/obo/IAO_0000119> "ChatGPT 3.5"@en ;
                                               rdfs:label "Horizontal Field Width"@en ,
                                                          "Horizontale Feldbreite"@de ;
                                               <http://www.w3.org/2004/02/skos/core#definition> "Horizontal Field Width refers to the horizontal extent of the observable field in an electron microscope."@en ,
                                                                                                "Horizontale Feldbreite bezieht sich auf den horizontalen Umfang des beobachtbaren Feldes in einem Elektronenmikroskop."@de .


###  https://w3id.org/pmd/mo/IMAGEPATH
<https://w3id.org/pmd/mo/IMAGEPATH> rdf:type owl:Class ;
                                    rdfs:subClassOf <https://w3id.org/pmd/co/Identifier> ;
                                    rdfs:isDefinedBy <https://w3id.org/pmd/mo> ;
                                    rdfs:label "Bildpfad"@de ,
                                               "Image Path"@en ;
                                    <http://www.w3.org/2004/02/skos/core#definition> "Der Speicherort oder Verzeichnispfad, an dem eine Bilddatei gespeichert ist."@de ,
                                                                                     "The location or directory path where an image file is stored."@en ;
                                    <https://w3id.org/pmd/co/definitionSource> "ChatGPT 3.5"@en .


###  https://w3id.org/pmd/mo/ImageFilter
<https://w3id.org/pmd/mo/ImageFilter> rdf:type owl:Class ;
                                      rdfs:subClassOf <https://w3id.org/pmd/mo/OpticalElement> ;
                                      rdfs:isDefinedBy <https://w3id.org/pmd/mo> ;
                                      rdfs:label "Abbildungsfilter"@de ,
                                                 "Image Filter"@en ;
                                      <http://www.w3.org/2004/02/skos/core#definition> "An image filter is a device or component used in imaging systems, such as microscopy or photography, to modify the appearance of an image by selectively altering certain characteristics. Filters can be used to adjust contrast, brightness, color balance, and other image properties. They are often used to enhance specific features or to correct for distortions caused by lighting conditions or optical imperfections."@en ;
                                      <https://w3id.org/pmd/co/definitionSource> "ChatGPT 3.5"@en .


###  https://w3id.org/pmd/mo/ImageName
<https://w3id.org/pmd/mo/ImageName> rdf:type owl:Class ;
                                    rdfs:subClassOf <https://w3id.org/pmd/co/Identifier> ;
                                    rdfs:isDefinedBy <https://w3id.org/pmd/mo> ;
                                    rdfs:label "Bildname"@de ,
                                               "Image Name"@en ;
                                    <http://www.w3.org/2004/02/skos/core#definition> "The designated name or title for an image."@en ;
                                    <https://w3id.org/pmd/co/definitionSource> "ChatGPT 3.5"@en .


###  https://w3id.org/pmd/mo/ImageSizeXAxis
<https://w3id.org/pmd/mo/ImageSizeXAxis> rdf:type owl:Class ;
                                         rdfs:subClassOf <https://w3id.org/pmd/co/ValueObject> ;
                                         rdfs:isDefinedBy <https://w3id.org/pmd/mo> ;
                                         rdfs:label "Bildgröße X-Achse"@de ,
                                                    "Image Size X-Axis"@en ;
                                         <http://www.w3.org/2004/02/skos/core#definition> "The size of the image along the X-axis."@en ;
                                         <https://w3id.org/pmd/co/definitionSource> "ChatGPT 3.5"@en .


###  https://w3id.org/pmd/mo/ImageSizeYAxis
<https://w3id.org/pmd/mo/ImageSizeYAxis> rdf:type owl:Class ;
                                         rdfs:subClassOf <https://w3id.org/pmd/co/ValueObject> ;
                                         rdfs:isDefinedBy <https://w3id.org/pmd/mo> ;
                                         rdfs:label "Bildgröße Y-Achse"@de ,
                                                    "Image Size Y-Axis"@en ;
                                         <http://www.w3.org/2004/02/skos/core#definition> "The size of the image along the Y-axis."@en ;
                                         <https://w3id.org/pmd/co/definitionSource> "ChatGPT 3.5"@en .


###  https://w3id.org/pmd/mo/IncidentBeam
<https://w3id.org/pmd/mo/IncidentBeam> rdf:type owl:Class ;
                                       rdfs:subClassOf <https://w3id.org/pmd/mo/Beam> ;
                                       rdfs:isDefinedBy <https://w3id.org/pmd/mo> ;
                                       rdfs:label "Einfallender Strahl"@de ,
                                                  "Incident Beam"@en ;
                                       <http://www.w3.org/2004/02/skos/core#definition> "Der Elektronenstrahl, der in einem Elektronenmikroskop auf die Probenoberfläche trifft und Wechselwirkungen hervorruft, die Signale für die Abbildung oder Analyse erzeugen."@de ,
                                                                                        "The electron beam that strikes the specimen surface in an electron microscope, causing interactions that produce signals for imaging or analysis."@en ;
                                       <https://w3id.org/pmd/co/definitionSource> "ChatGPT 3.5" .


###  https://w3id.org/pmd/mo/IndicatedMagnification
<https://w3id.org/pmd/mo/IndicatedMagnification> rdf:type owl:Class ;
                                                 rdfs:subClassOf <https://w3id.org/pmd/mo/Magnification> ;
                                                 <http://purl.obolibrary.org/obo/IAO_0000117> "PMDco Team"@en ;
                                                 <http://purl.obolibrary.org/obo/IAO_0000119> "ChatGPT 3.5"@en ;
                                                 rdfs:label "Angegebene Vergrößerung"@de ,
                                                            "Indicated Magnification"@en ;
                                                 <http://www.w3.org/2004/02/skos/core#definition> "Angegebene Vergrößerung bezieht sich auf den Vergrößerungsgrad, der von den Steuerungen oder Anzeigen des Instruments in einem Elektronenmikroskop angezeigt wird."@de ,
                                                                                                  "Indicated Magnification refers to the magnification level shown by the instrument's controls or display in an electron microscope."@en .


###  https://w3id.org/pmd/mo/InelasticScattering
<https://w3id.org/pmd/mo/InelasticScattering> rdf:type owl:Class ;
                                              rdfs:subClassOf <https://w3id.org/pmd/mo/PhysicalProcess> ;
                                              rdfs:isDefinedBy <https://w3id.org/pmd/mo> ;
                                              rdfs:label "Inelastic Scattering"@en ,
                                                         "Inelastische Streuung"@de ;
                                              <http://www.w3.org/2004/02/skos/core#definition> "Inelastic scattering is a scattering process that involves the transfer of energy and momentum between the incident particle (e.g., photon, electron) and the target particle. During inelastic scattering, the energy of the scattered particle changes, and the interaction may result in various outcomes, such as excitation, emission, or other energy transfers that alter the internal state of the target particle."@en ;
                                              <https://w3id.org/pmd/co/definitionSource> "ChatGPT 3.5"@en .


###  https://w3id.org/pmd/mo/InteractionVolume
<https://w3id.org/pmd/mo/InteractionVolume> rdf:type owl:Class ;
                                            rdfs:subClassOf <https://w3id.org/pmd/mo/Volume> ;
                                            rdfs:isDefinedBy <https://w3id.org/pmd/mo> ;
                                            rdfs:label "Interaction Volume"@en ,
                                                       "Überlagerungsvolumen"@de ;
                                            <http://www.w3.org/2004/02/skos/core#definition> "Der Bereich innerhalb einer Probe, in dem ein Teilchenstrahl mit dem Material in Wechselwirkung tritt."@de ,
                                                                                             "The region within a sample where a particle beam interacts with the material."@en ;
                                            <https://w3id.org/pmd/co/definitionSource> "ChatGPT 3.5"@en .


###  https://w3id.org/pmd/mo/IntermediateLense
<https://w3id.org/pmd/mo/IntermediateLense> rdf:type owl:Class ;
                                            rdfs:subClassOf <https://w3id.org/pmd/mo/Lense> ;
                                            rdfs:isDefinedBy <https://w3id.org/pmd/mo> ;
                                            rdfs:label "Intermediate Lens"@en ,
                                                       "Zwischenlinse"@de ;
                                            <http://www.w3.org/2004/02/skos/core#definition> "A lens that is positioned between the objective lens and the projector lens in an optical system."@en ,
                                                                                             "Eine Linse, die zwischen der Objektivlinse und der Projektorlinse in einem optischen System positioniert ist."@de ;
                                            <https://w3id.org/pmd/co/definitionSource> "ChatGPT 3.5"@en .


###  https://w3id.org/pmd/mo/IonBeam
<https://w3id.org/pmd/mo/IonBeam> rdf:type owl:Class ;
                                  rdfs:subClassOf <https://w3id.org/pmd/mo/Beam> ;
                                  rdfs:isDefinedBy <https://w3id.org/pmd/mo> ;
                                  rdfs:label "Ion Beam"@en ,
                                             "Ionenstrahl"@de ;
                                  <http://www.w3.org/2004/02/skos/core#definition> "A stream of ions used for grinding or analysis, especially in ion microscopy techniques for imaging."@en ,
                                                                                   "Ein Ionenstrom, der zum Mahlen oder zur Analyse verwendet wird, insbesondere bei Ionenmikroskopietechniken zur Bildgebung."@de ;
                                  <https://w3id.org/pmd/co/definitionSource> "ChatGPT 3.5" .


###  https://w3id.org/pmd/mo/IonMicroscope
<https://w3id.org/pmd/mo/IonMicroscope> rdf:type owl:Class ;
                                        rdfs:subClassOf <https://w3id.org/pmd/co/Micropscope> ;
                                        rdfs:isDefinedBy <https://w3id.org/pmd/mo> ;
                                        rdfs:label "Ion Microscope"@en ,
                                                   "Ionenmikroskop"@de ;
                                        <http://www.w3.org/2004/02/skos/core#definition> "A microscope that uses ions to create images of samples."@en ,
                                                                                         "Ein Mikroskop, das mit Hilfe von Ionen Bilder von Proben erzeugt."@de ;
                                        <https://w3id.org/pmd/co/definitionSource> "ChatGPT 3.5"@en .


###  https://w3id.org/pmd/mo/IonMicroscopy
<https://w3id.org/pmd/mo/IonMicroscopy> rdf:type owl:Class ;
                                        rdfs:subClassOf <https://w3id.org/pmd/co/MicroscopyProcess> ;
                                        rdfs:isDefinedBy <https://w3id.org/pmd/mo> ;
                                        rdfs:label "Ion Microscopy"@en ,
                                                   "Ionenmikroskopie"@de ;
                                        <http://www.w3.org/2004/02/skos/core#definition> "Ion Microscopy refers to a group of microscopy techniques that use focused ion beams to image and analyze samples. These techniques utilize ions, such as protons or heavy ions, instead of electrons or photons to interact with the sample, providing valuable information about its composition and structure."@en ;
                                        <https://w3id.org/pmd/co/definitionSource> "ChatGPT 3.5"@en .


###  https://w3id.org/pmd/mo/Lense
<https://w3id.org/pmd/mo/Lense> rdf:type owl:Class ;
                                rdfs:subClassOf <https://w3id.org/pmd/mo/OpticalElement> ;
                                rdfs:isDefinedBy <https://w3id.org/pmd/mo> ;
                                rdfs:label "Lens"@en ,
                                           "Linse"@de ;
                                <http://www.w3.org/2004/02/skos/core#definition> "A piece of optical glass or other transparent material used to focus or magnify light in optical instruments."@en ,
                                                                                 "Ein Stück optisches Glas oder anderes transparentes Material, das zum Fokussieren oder Vergrößern von Licht in optischen Geräten verwendet wird."@de ;
                                <https://w3id.org/pmd/co/definitionSource> "ChatGPT 3.5"@en .


###  https://w3id.org/pmd/mo/LightMicroscope
<https://w3id.org/pmd/mo/LightMicroscope> rdf:type owl:Class ;
                                          rdfs:subClassOf <https://w3id.org/pmd/mo/OpticalMicroscope> ;
                                          rdfs:isDefinedBy <https://w3id.org/pmd/mo> ;
                                          rdfs:label "Lichtmikroskop"@de ,
                                                     "Light Microscope"@en ;
                                          <http://www.w3.org/2004/02/skos/core#definition> "An optical microscope that uses visible light to illuminate and magnify samples."@en ,
                                                                                           "Ein optisches Mikroskop, das sichtbares Licht verwendet, um Proben zu beleuchten und zu vergrößern."@de ;
                                          <https://w3id.org/pmd/co/definitionSource> "ChatGPT 3.5"@en .


###  https://w3id.org/pmd/mo/LightMicroscopy
<https://w3id.org/pmd/mo/LightMicroscopy> rdf:type owl:Class ;
                                          rdfs:subClassOf <https://w3id.org/pmd/co/OpticalMicroscopy> ;
                                          rdfs:isDefinedBy <https://w3id.org/pmd/mo> ;
                                          rdfs:label "Lichtmikroskopie"@de ,
                                                     "Light Microscopy"@en ;
                                          <http://www.w3.org/2004/02/skos/core#definition> "Die Verwendung von sichtbarem Licht zur Beobachtung und Untersuchung kleiner Objekte oder Strukturen."@de ,
                                                                                           "The use of visible light to observe and study small objects or structures."@en ;
                                          <https://w3id.org/pmd/co/definitionSource> "ChatGPT 3.5"@en .


###  https://w3id.org/pmd/mo/Magnification
<https://w3id.org/pmd/mo/Magnification> rdf:type owl:Class ;
                                        rdfs:subClassOf <https://w3id.org/pmd/co/ValueObject> ;
                                        rdfs:isDefinedBy <https://w3id.org/pmd/mo> ;
                                        rdfs:label "Magnification"@en ,
                                                   "Vergrößerung"@de ;
                                        <http://www.w3.org/2004/02/skos/core#definition> "Das Verhältnis zwischen der Größe eines von einem optischen System erzeugten Bildes und der Größe des Objekts."@de ,
                                                                                         "The process of enlarging the appearance of an image."@en ,
                                                                                         "The ratio of the size of an image produced by an optical system to the size of the object."@en ;
                                        <https://w3id.org/pmd/co/definitionSource> "ChatGPT 3.5"@en .


###  https://w3id.org/pmd/mo/MaximumExposure
<https://w3id.org/pmd/mo/MaximumExposure> rdf:type owl:Class ;
                                          rdfs:subClassOf <https://w3id.org/pmd/co/ValueObject> ;
                                          rdfs:isDefinedBy <https://w3id.org/pmd/mo> ;
                                          rdfs:label "Maximale Belichtung"@de ,
                                                     "Maximum Exposure"@en ;
                                          <http://www.w3.org/2004/02/skos/core#definition> "The maximum duration for which the imaging sensor can be exposed to light, measured in seconds."@en ;
                                          <https://w3id.org/pmd/co/definitionSource> "ChatGPT 3.5"@en .


###  https://w3id.org/pmd/mo/MechanicalPolishing
<https://w3id.org/pmd/mo/MechanicalPolishing> rdf:type owl:Class ;
                                              rdfs:subClassOf <https://w3id.org/pmd/co/ManufacturingProcess> ;
                                              rdfs:isDefinedBy <https://w3id.org/pmd/mo> ;
                                              rdfs:label "Mechanical Polishing"@en ,
                                                         "Mechanisches Polieren"@de ;
                                              <http://www.w3.org/2004/02/skos/core#definition> """Mechanical polishing is a material preparation technique used to enhance the surface quality and finish of a sample by removing thin layers of material through abrasion. It involves using abrasive materials, such as polishing cloths, diamond suspensions, or abrasive pastes, along with a polishing machine or device. The process typically includes several steps, each using progressively finer abrasives to achieve a smooth and mirror-like surface.

During mechanical polishing, the sample is pressed against the rotating polishing medium with controlled pressure. The abrasive particles embedded in the medium gradually remove surface irregularities, scratches, and imperfections, resulting in improved flatness, clarity, and reflectivity. The process can be adjusted to target specific levels of surface roughness and precision.

Mechanical polishing is commonly used in various scientific and industrial applications, such as metallography, materials science, electronics, and optics. It is an essential step before further analyses like microscopy, spectroscopy, or surface profiling, as it provides a pristine surface for accurate characterization and observation of material properties."""@en ;
                                              <https://w3id.org/pmd/co/definitionSource> "ChatGPT 3.5"@en .


###  https://w3id.org/pmd/mo/MonochromaticBeam
<https://w3id.org/pmd/mo/MonochromaticBeam> rdf:type owl:Class ;
                                            rdfs:subClassOf <https://w3id.org/pmd/mo/Beam> ;
                                            rdfs:isDefinedBy <https://w3id.org/pmd/mo> ;
                                            rdfs:label "Monochromatic Beam"@en ,
                                                       "Monochromatischer Strahl"@de ;
                                            <http://www.w3.org/2004/02/skos/core#definition> "An electron beam consisting of electrons with a narrow range of energies, typically achieved using electron energy filters or monochromators."@en ,
                                                                                             "Ein Elektronenstrahl, der aus Elektronen mit einem engen Energiebereich besteht, der in der Regel durch Elektronenenergiefilter oder Monochromatoren erreicht wird."@de ;
                                            <https://w3id.org/pmd/co/definitionSource> "ChatGPT 3.5" .


###  https://w3id.org/pmd/mo/Monochromator
<https://w3id.org/pmd/mo/Monochromator> rdf:type owl:Class ;
                                        rdfs:subClassOf <https://w3id.org/pmd/mo/OpticalElement> ;
                                        rdfs:isDefinedBy <https://w3id.org/pmd/mo> ;
                                        rdfs:label "Monochromator"@de ,
                                                   "Monochromator"@en ;
                                        <http://www.w3.org/2004/02/skos/core#definition> "An optical device that transmits a narrow range of wavelengths of light."@en ,
                                                                                         "Ein optisches Gerät, das einen engen Wellenlängenbereich von Licht überträgt."@de ;
                                        <https://w3id.org/pmd/co/definitionSource> "ChatGPT 3.5"@en .


###  https://w3id.org/pmd/mo/ObjectiveAperture
<https://w3id.org/pmd/mo/ObjectiveAperture> rdf:type owl:Class ;
                                            rdfs:subClassOf <https://w3id.org/pmd/mo/Aperture> ;
                                            rdfs:isDefinedBy <https://w3id.org/pmd/mo> ;
                                            rdfs:label "Objective Aperture"@en ,
                                                       "Objektivblende"@de ;
                                            <http://www.w3.org/2004/02/skos/core#definition> "An aperture in the objective lens system of a microscope."@en ,
                                                                                             "Eine Blende im Objektivlinsensystem eines Mikroskops."@de ;
                                            <https://w3id.org/pmd/co/definitionSource> "ChatGPT 3.5"@en .


###  https://w3id.org/pmd/mo/ObjectiveLense
<https://w3id.org/pmd/mo/ObjectiveLense> rdf:type owl:Class ;
                                         rdfs:subClassOf <https://w3id.org/pmd/mo/Lense> ;
                                         rdfs:isDefinedBy <https://w3id.org/pmd/mo> ;
                                         rdfs:label "Objective Lens"@en ,
                                                    "Objektivlinse"@de ;
                                         <http://www.w3.org/2004/02/skos/core#definition> "A lens in a microscope or similar optical device that is closest to the specimen."@en ,
                                                                                          "Eine Linse in einem Mikroskop oder ähnlichen optischen Gerät, die am nächsten zur Probe liegt."@de ;
                                         <https://w3id.org/pmd/co/definitionSource> "ChatGPT 3.5"@en .


###  https://w3id.org/pmd/mo/OpticalElement
<https://w3id.org/pmd/mo/OpticalElement> rdf:type owl:Class ;
                                         rdfs:subClassOf <https://w3id.org/pmd/co/ProcessingNode> ;
                                         <http://purl.obolibrary.org/obo/IAO_0000117> "PMDco Team"@en ;
                                         <http://purl.obolibrary.org/obo/IAO_0000119> "ChatGPT 3.5"@en ;
                                         rdfs:label "Optical Element"@en ,
                                                    "Optisches Element"@de ;
                                         <http://www.w3.org/2004/02/skos/core#definition> "An Optical Element is a component of an optical system that affects the propagation of light, such as lenses, mirrors, or prisms."@en ,
                                                                                          "Ein optisches Element ist eine Komponente eines optischen Systems, das die Ausbreitung von Licht beeinflusst, wie Linsen, Spiegel oder Prismen."@de .


###  https://w3id.org/pmd/mo/OpticalMicroscope
<https://w3id.org/pmd/mo/OpticalMicroscope> rdf:type owl:Class ;
                                            rdfs:subClassOf <https://w3id.org/pmd/co/Micropscope> ;
                                            rdfs:isDefinedBy <https://w3id.org/pmd/mo> ;
                                            rdfs:label "Optical Microscope"@en ,
                                                       "Optisches Mikroskop"@de ;
                                            <http://www.w3.org/2004/02/skos/core#definition> "A microscope that uses visible light and lenses to magnify specimens."@en ,
                                                                                             "Ein Mikroskop, das sichtbares Licht und Linsen zur Vergrößerung von Proben verwendet."@de ;
                                            <https://w3id.org/pmd/co/definitionSource> "ChatGPT 3.5"@en .


###  https://w3id.org/pmd/mo/OrientationImagingMicroscopy
<https://w3id.org/pmd/mo/OrientationImagingMicroscopy> rdf:type owl:Class ;
                                                       rdfs:subClassOf <https://w3id.org/pmd/mo/ScanningElectronMicroscopy> ;
                                                       rdfs:isDefinedBy <https://w3id.org/pmd/mo> ;
                                                       rdfs:label "Bildgebende Orientierungsmikroskopie"@de ,
                                                                  "Orientation Imaging Microscopy"@en ;
                                                       <http://www.w3.org/2004/02/skos/core#definition> "Orientation Imaging Microscopy is a microscopy technique used to map the crystallographic orientations of grains within a material. It is commonly applied in SEM to study the microstructural properties of polycrystalline materials."@en ;
                                                       <https://w3id.org/pmd/co/definitionSource> "ChatGPT 3.5"@en ;
                                                       <https://w3id.org/pmd/mo/abbreviation> "OIM"@en .


###  https://w3id.org/pmd/mo/Palette
<https://w3id.org/pmd/mo/Palette> rdf:type owl:Class ;
                                  rdfs:subClassOf <https://w3id.org/pmd/co/ValueObject> ;
                                  rdfs:isDefinedBy <https://w3id.org/pmd/mo> ;
                                  rdfs:label "Palette"@de ,
                                             "Palette"@en ;
                                  <http://www.w3.org/2004/02/skos/core#altLabel> "Color Lookup Table"@en ,
                                                                                 "Farbzuordnungstabelle"@de ;
                                  <http://www.w3.org/2004/02/skos/core#definition> "In computer graphics, a palette is the set of available colors from which an image can be made. In some systems, the palette is fixed by the hardware design, and in others it is dynamic, typically implemented via a color lookup table (CLUT), a correspondence table in which selected colors from a certain color space's color reproduction range are assigned an index, by which they can be referenced."@en ;
                                  <http://www.w3.org/2004/02/skos/core#example> "Typical colorscales may be, e.g., greyscale, RGB, or CMYK."@en ;
                                  <https://w3id.org/pmd/co/definitionSource> "https://en.wikipedia.org/wiki/Palette_(computing)"@en ;
                                  <https://w3id.org/pmd/mo/abbreviation> "CLUT"@en .


###  https://w3id.org/pmd/mo/PhysicalProcess
<https://w3id.org/pmd/mo/PhysicalProcess> rdf:type owl:Class ;
                                          rdfs:subClassOf <https://w3id.org/pmd/co/Process> ;
                                          rdfs:isDefinedBy <https://w3id.org/pmd/mo> ;
                                          rdfs:label "Physical Process"@en ,
                                                     "Physikalischer Prozess"@de ;
                                          <http://www.w3.org/2004/02/skos/core#definition> "A physical process refers to a sequence of events or interactions that occur in the physical world and can be described and analyzed based on the principles of physics. These processes involve the transformation of energy, matter, or both, and they often follow established laws and theories of physics. In particular, a physical process may just occur due to natural circumstances and does not necessarily have to be induced by human activities or interactions."@en ;
                                          <https://w3id.org/pmd/co/definitionSource> "ChatGPT 3.5"@en .


###  https://w3id.org/pmd/mo/PixelSize
<https://w3id.org/pmd/mo/PixelSize> rdf:type owl:Class ;
                                    rdfs:subClassOf <https://w3id.org/pmd/co/ValueObject> ;
                                    rdfs:isDefinedBy <https://w3id.org/pmd/mo> ;
                                    rdfs:label "Pixel Size"@en ,
                                               "Pixelgröße"@en ;
                                    <http://www.w3.org/2004/02/skos/core#definition> "Die Größe der einzelnen Pixel in einem digitalen Bild oder einer Anzeige."@de ,
                                                                                     "The size of individual pixels in a digital image or display."@en ;
                                    <https://w3id.org/pmd/co/definitionSource> "ChatGPT 3.5"@en .


###  https://w3id.org/pmd/mo/PolarizedLightMicroscope
<https://w3id.org/pmd/mo/PolarizedLightMicroscope> rdf:type owl:Class ;
                                                   rdfs:subClassOf <https://w3id.org/pmd/mo/LightMicroscope> ;
                                                   rdfs:isDefinedBy <https://w3id.org/pmd/mo> ;
                                                   rdfs:label "Polarisiertes Lichtmikroskop"@de ,
                                                              "Polarized Light Microscope"@en ;
                                                   <http://www.w3.org/2004/02/skos/core#definition> "A microscope that uses polarized light to observe and analyze samples."@en ,
                                                                                                    "Ein Mikroskop, das polarisiertes Licht zur Beobachtung und Analyse von Proben verwendet."@de ;
                                                   <https://w3id.org/pmd/co/definitionSource> "ChatGPT 3.5"@en ;
                                                   <https://w3id.org/pmd/mo/abbreviation> "PLM"@en .


###  https://w3id.org/pmd/mo/PolarizedLightMicroscopy
<https://w3id.org/pmd/mo/PolarizedLightMicroscopy> rdf:type owl:Class ;
                                                   rdfs:subClassOf <https://w3id.org/pmd/mo/LightMicroscopy> ;
                                                   rdfs:isDefinedBy <https://w3id.org/pmd/mo> ;
                                                   rdfs:label "Polarisationslichtmikroskopie"@de ,
                                                              "Polarized Light Microscopy"@en ;
                                                   <http://www.w3.org/2004/02/skos/core#definition> "Polarized Light Microscopy is a technique that uses polarized light to enhance the contrast and reveal structural information in transparent samples. Light waves vibrate in specific directions, and by using polarizers to control the orientation of light waves, polarized light microscopy can highlight birefringent materials, anisotropic structures, and stress patterns within samples. This technique is valuable for studying crystalline structures, fibers, and anisotropic materials."@en ;
                                                   <https://w3id.org/pmd/co/definitionSource> "ChatGPT 3.5"@en ;
                                                   <https://w3id.org/pmd/mo/abbreviation> "PLM"@en .


###  https://w3id.org/pmd/mo/PolePiece
<https://w3id.org/pmd/mo/PolePiece> rdf:type owl:Class ;
                                    rdfs:subClassOf <https://w3id.org/pmd/mo/OpticalElement> ;
                                    rdfs:isDefinedBy <https://w3id.org/pmd/mo> ;
                                    rdfs:label "Pole Piece"@en ,
                                               "Polschuh"@de ;
                                    <http://www.w3.org/2004/02/skos/core#definition> "A component of the electron column in an electron microscope that focuses and guides the electron beam onto the specimen."@en ,
                                                                                     "Eine Komponente der Elektronensäule in einem Elektronenmikroskop, die den Elektronenstrahl fokussiert und auf die Probe lenkt."@de ;
                                    <https://w3id.org/pmd/co/definitionSource> "ChatGPT 3.5" .


###  https://w3id.org/pmd/mo/PrecessionElectronDiffraction
<https://w3id.org/pmd/mo/PrecessionElectronDiffraction> rdf:type owl:Class ;
                                                        rdfs:subClassOf <https://w3id.org/pmd/mo/ElectronDiffraction> ;
                                                        <http://purl.obolibrary.org/obo/IAO_0000117> "PMDco Team"@en ;
                                                        <http://purl.obolibrary.org/obo/IAO_0000119> "ChatGPT 3.5"@en ;
                                                        rdfs:label "Precession Electron Diffraction"@en ,
                                                                   "Präzessionselektronenbeugung"@de ;
                                                        <http://www.w3.org/2004/02/skos/core#definition> "Precession Electron Diffraction is a technique used in electron microscopy where the electron beam is tilted in a precession motion, improving the quality of diffraction patterns and reducing dynamical effects."@en ,
                                                                                                         "Präzessionselektronenbeugung ist eine Technik in der Elektronenmikroskopie, bei der der Elektronenstrahl in einer Präzessionsbewegung geneigt wird, wodurch die Qualität der Beugungsmuster verbessert und dynamische Effekte reduziert werden."@de .


###  https://w3id.org/pmd/mo/Pressure
<https://w3id.org/pmd/mo/Pressure> rdf:type owl:Class ;
                                   rdfs:subClassOf <https://w3id.org/pmd/co/ValueObject> ;
                                   rdfs:isDefinedBy <https://w3id.org/pmd/mo> ;
                                   rdfs:label "Druck"@de ,
                                              "Pressure"@en ;
                                   <http://www.w3.org/2004/02/skos/core#definition> "Die auf eine Fläche ausgeübte Kraft in einem System, typischerweise gemessen in Pascal oder anderen Einheiten."@de ,
                                                                                    "The force exerted per unit area in a system, typically measured in pascals or other units."@en ;
                                   <https://w3id.org/pmd/co/definitionSource> "ChatGPT 3.5"@en .


###  https://w3id.org/pmd/mo/PrimaryBeam
<https://w3id.org/pmd/mo/PrimaryBeam> rdf:type owl:Class ;
                                      rdfs:subClassOf <https://w3id.org/pmd/mo/Beam> ;
                                      rdfs:isDefinedBy <https://w3id.org/pmd/mo> ;
                                      rdfs:label "Primary Beam"@en ,
                                                 "Primärstrahl"@de ;
                                      <http://www.w3.org/2004/02/skos/core#definition> "Der Hauptelektronenstrahl, der von der Elektronenquelle ausgesandt und auf die Probe in einem Elektronenmikroskop gerichtet wird."@de ,
                                                                                       "The main electron beam emitted from the electron source and directed towards the specimen in an electron microscope."@en ;
                                      <https://w3id.org/pmd/co/definitionSource> "ChatGPT 3.5" .


###  https://w3id.org/pmd/mo/ProbeCurrent
<https://w3id.org/pmd/mo/ProbeCurrent> rdf:type owl:Class ;
                                       rdfs:subClassOf <https://w3id.org/pmd/mo/Current> ;
                                       rdfs:comment "The current in the probe is typically measured in nanoamperes (nA)."@en ;
                                       rdfs:isDefinedBy <https://w3id.org/pmd/mo> ;
                                       rdfs:label "Probe Current"@en ,
                                                  "Sondenstrom"@de ;
                                       <http://www.w3.org/2004/02/skos/core#definition> "Der Strom der Elektronen im fokussierten Elektronenstrahl, der zur Abbildung oder Analyse in einem Elektronenmikroskop verwendet wird."@de ,
                                                                                        "The current of electrons in the focused electron beam used for imaging or analysis in an electron microscope."@en ;
                                       <https://w3id.org/pmd/co/definitionSource> "ChatGPT 3.5" .


###  https://w3id.org/pmd/mo/ProbeSize
<https://w3id.org/pmd/mo/ProbeSize> rdf:type owl:Class ;
                                    rdfs:subClassOf <https://w3id.org/pmd/co/ValueObject> ;
                                    rdfs:isDefinedBy <https://w3id.org/pmd/mo> ;
                                    rdfs:label "Probe Size"@en ,
                                               "Sensorgröße"@de ,
                                               "Sondengröße"@de ;
                                    <http://www.w3.org/2004/02/skos/core#altLabel> "Messfühlergröße"@de ;
                                    <http://www.w3.org/2004/02/skos/core#definition> "Die Größe der Sonde oder des Strahls, die bei Mikroskopie- oder Spektroskopieverfahren verwendet werden."@de ,
                                                                                     "The size of the probe or beam used in microscopy or spectroscopy techniques. It is typically measured in nanometers (nm)."@en ;
                                    <https://w3id.org/pmd/co/definitionSource> "ChatGPT 3.5"@en .


###  https://w3id.org/pmd/mo/ProjectorLense
<https://w3id.org/pmd/mo/ProjectorLense> rdf:type owl:Class ;
                                         rdfs:subClassOf <https://w3id.org/pmd/mo/Lense> ;
                                         rdfs:isDefinedBy <https://w3id.org/pmd/mo> ;
                                         rdfs:label "Projector Lens"@en ,
                                                    "Projektorlinse"@de ;
                                         <http://www.w3.org/2004/02/skos/core#definition> "A lens used to project the image from the intermediate lens onto a viewing screen or detector."@en ,
                                                                                          "Eine Linse, die verwendet wird, um das Bild von der Zwischenlinse auf einen Bildschirm oder Detektor zu projizieren."@de ;
                                         <https://w3id.org/pmd/co/definitionSource> "ChatGPT 3.5"@en .


###  https://w3id.org/pmd/mo/ReadoutTime
<https://w3id.org/pmd/mo/ReadoutTime> rdf:type owl:Class ;
                                      rdfs:subClassOf <https://w3id.org/pmd/co/Time> ;
                                      rdfs:isDefinedBy <https://w3id.org/pmd/mo> ;
                                      rdfs:label "Auslesezeit"@de ,
                                                 "Readout Time"@en ;
                                      <http://www.w3.org/2004/02/skos/core#definition> "The time taken to read out data from a sensor, typically measured in nanoseconds (ns)."@en ;
                                      <https://w3id.org/pmd/co/definitionSource> "ChatGPT 3.5"@en .


###  https://w3id.org/pmd/mo/Reconstruction
<https://w3id.org/pmd/mo/Reconstruction> rdf:type owl:Class ;
                                         rdfs:subClassOf <https://w3id.org/pmd/co/AnalysingProcess> ;
                                         rdfs:isDefinedBy <https://w3id.org/pmd/mo> ;
                                         rdfs:label "Reconstruction"@en ,
                                                    "Rekonstruktion"@de ;
                                         <http://www.w3.org/2004/02/skos/core#definition> "Der Prozess der Erstellung eines dreidimensionalen Bildes oder Modells aus zweidimensionalen Daten."@de ,
                                                                                          "The process of creating a three-dimensional image or model from two-dimensional data."@en ;
                                         <https://w3id.org/pmd/co/definitionSource> "ChatGPT 3.5"@en .


###  https://w3id.org/pmd/mo/Resolution
<https://w3id.org/pmd/mo/Resolution> rdf:type owl:Class ;
                                     rdfs:subClassOf <https://w3id.org/pmd/co/ValueObject> ;
                                     rdfs:isDefinedBy <https://w3id.org/pmd/mo> ;
                                     rdfs:label "Auflösung"@de ,
                                                "Resolution"@en ;
                                     <http://www.w3.org/2004/02/skos/core#definition> "In various contexts, resolution refers to the degree of detail that can be discerned in an image, measurement, or other representation of an object or phenomenon."@en ,
                                                                                      "In verschiedenen Zusammenhängen bezieht sich die Auflösung auf den Grad der Detailgenauigkeit, die in einem Bild, einer Messung oder einer anderen Darstellung eines Objekts oder Phänomens erkennbar ist."@de ;
                                     <https://w3id.org/pmd/co/definitionSource> "ChatGPT 3.5"@en .


###  https://w3id.org/pmd/mo/RotationAngle
<https://w3id.org/pmd/mo/RotationAngle> rdf:type owl:Class ;
                                        rdfs:subClassOf <https://w3id.org/pmd/mo/Angle> ;
                                        rdfs:isDefinedBy <https://w3id.org/pmd/mo> ;
                                        rdfs:label "Rotation Angle"@en ,
                                                   "Rotationswinkel"@de ;
                                        <http://www.w3.org/2004/02/skos/core#definition> "Der Winkel, um den ein Objekt um eine bestimmte Achse rotiert wird."@de ,
                                                                                         "The angle by which an object is rotated around a specific axis."@en ;
                                        <https://w3id.org/pmd/co/definitionSource> "ChatGPT 3.5"@en .


###  https://w3id.org/pmd/mo/ScanRate
<https://w3id.org/pmd/mo/ScanRate> rdf:type owl:Class ;
                                   rdfs:subClassOf <https://w3id.org/pmd/co/TestingRate> ;
                                   rdfs:isDefinedBy <https://w3id.org/pmd/mo> ;
                                   rdfs:label "Abtastrate"@de ,
                                              "Scan Rate"@en ;
                                   <http://www.w3.org/2004/02/skos/core#definition> "Die Geschwindigkeit, mit der Daten gescannt oder aufgezeichnet werden."@de ,
                                                                                    "The speed at which data is scanned or recorded."@en ;
                                   <https://w3id.org/pmd/co/definitionSource> "ChatGPT 3.5"@en .


###  https://w3id.org/pmd/mo/ScanningElectronMicroscope
<https://w3id.org/pmd/mo/ScanningElectronMicroscope> rdf:type owl:Class ;
                                                     rdfs:subClassOf <https://w3id.org/pmd/co/ElectronMicroscope> ;
                                                     rdfs:isDefinedBy <https://w3id.org/pmd/mo> ;
                                                     rdfs:label "Rasterelektronenmikroskop"@de ,
                                                                "Scanning Electron Microscope"@en ;
                                                     <http://www.w3.org/2004/02/skos/core#definition> "A microscope that produces images of a sample by scanning it with a focused beam of electrons."@en ,
                                                                                                      "Ein Mikroskop, das Bilder einer Probe erzeugt, indem es diese mit einem fokussierten Elektronenstrahl abtastet."@de ;
                                                     <https://w3id.org/pmd/co/definitionSource> "ChatGPT 3.5"@en ;
                                                     <https://w3id.org/pmd/mo/abbreviation> "REM"@de ,
                                                                                            "SEM"@en .


###  https://w3id.org/pmd/mo/ScanningElectronMicroscopy
<https://w3id.org/pmd/mo/ScanningElectronMicroscopy> rdf:type owl:Class ;
                                                     rdfs:subClassOf <https://w3id.org/pmd/co/ElectronMicroscopy> ;
                                                     rdfs:isDefinedBy <https://w3id.org/pmd/mo> ;
                                                     rdfs:label "Rasterelektronenmikroskopie"@de ,
                                                                "Scanning Electron Microscopy"@en ;
                                                     <http://www.w3.org/2004/02/skos/core#definition> "Scanning Electron Microscopy is a microscopy technique that uses a focused beam of electrons to scan the surface of a sample. The interaction of the electrons with the sample generates signals that provide information about the sample's topography, morphology, and composition."@en ;
                                                     <https://w3id.org/pmd/co/definitionSource> "ChatGPT 3.5"@en ;
                                                     <https://w3id.org/pmd/mo/abbreviation> "SEM"@en .


###  https://w3id.org/pmd/mo/ScanningProbeMicroscope
<https://w3id.org/pmd/mo/ScanningProbeMicroscope> rdf:type owl:Class ;
                                                  rdfs:subClassOf <https://w3id.org/pmd/co/ElectronMicroscope> ;
                                                  rdfs:isDefinedBy <https://w3id.org/pmd/mo> ;
                                                  rdfs:label "Rastersondenmikroskop"@de ,
                                                             "Scanning Probe Microscope"@en ;
                                                  <http://www.w3.org/2004/02/skos/core#definition> "A type of microscope that images surfaces by scanning a probe over the sample."@en ,
                                                                                                   "Ein Mikroskoptyp, der Oberflächen abbildet, indem er eine Sonde über die Probe führt."@de ;
                                                  <https://w3id.org/pmd/co/definitionSource> "ChatGPT 3.5"@en .


###  https://w3id.org/pmd/mo/ScanningProbeMicroscopy
<https://w3id.org/pmd/mo/ScanningProbeMicroscopy> rdf:type owl:Class ;
                                                  rdfs:subClassOf <https://w3id.org/pmd/co/ElectronMicroscopy> ;
                                                  rdfs:isDefinedBy <https://w3id.org/pmd/mo> ;
                                                  rdfs:label "Rastersondenmikroskopie"@de ,
                                                             "Scanning Probe Microscopy"@en ;
                                                  <http://www.w3.org/2004/02/skos/core#definition> "Scanning Probe Microscopy encompasses various techniques, such as Atomic Force Microscopy (AFM) and Scanning Tunneling Microscopy (STM), that use a sharp probe to scan a sample's surface. These techniques provide high-resolution images and information about surface properties on the nanometer scale."@en ;
                                                  <https://w3id.org/pmd/co/definitionSource> "ChatGPT 3.5"@en ;
                                                  <https://w3id.org/pmd/mo/abbreviation> "SPM"@en .


###  https://w3id.org/pmd/mo/ScanningTransmissionElectronMicroscope
<https://w3id.org/pmd/mo/ScanningTransmissionElectronMicroscope> rdf:type owl:Class ;
                                                                 rdfs:subClassOf <https://w3id.org/pmd/mo/TransmissionElectronMicroscope> ;
                                                                 rdfs:isDefinedBy <https://w3id.org/pmd/mo> ;
                                                                 rdfs:label "Rastertransmissionselektronenmikroskop"@de ,
                                                                            "Scanning Transmission Electron Microscope"@en ;
                                                                 <http://www.w3.org/2004/02/skos/core#definition> "A type of transmission electron microscope where a focused electron beam is scanned across the sample."@en ,
                                                                                                                  "Eine Art von Transmissionselektronenmikroskop, bei dem ein fokussierter Elektronenstrahl über die Probe gescannt wird."@de ;
                                                                 <https://w3id.org/pmd/co/definitionSource> "ChatGPT 3.5"@en ;
                                                                 <https://w3id.org/pmd/mo/abbreviation> "STEM"@en .


###  https://w3id.org/pmd/mo/ScanningTransmissionElectronMicroscopy
<https://w3id.org/pmd/mo/ScanningTransmissionElectronMicroscopy> rdf:type owl:Class ;
                                                                 rdfs:subClassOf <https://w3id.org/pmd/mo/TransmissionElectronMicroscopy> ;
                                                                 rdfs:isDefinedBy <https://w3id.org/pmd/mo> ;
                                                                 rdfs:label "Rastertransmissionselektronenmikroskopie"@de ,
                                                                            "Scanning Transmission Electron Microscopy"@en ;
                                                                 <http://www.w3.org/2004/02/skos/core#definition> "Scanning Transmission Electron Microscopy is a technique that combines the principles of scanning and transmission electron microscopy. It allows imaging and spectroscopy with high spatial resolution."@en ;
                                                                 <https://w3id.org/pmd/co/definitionSource> "ChatGPT 3.5"@en ;
                                                                 <https://w3id.org/pmd/mo/abbreviation> "STEM"@en .


###  https://w3id.org/pmd/mo/ScanningTransmissionElectronMicroscopy-ElectronEnergyLossSpectroscopy
<https://w3id.org/pmd/mo/ScanningTransmissionElectronMicroscopy-ElectronEnergyLossSpectroscopy> rdf:type owl:Class ;
                                                                                                rdfs:subClassOf <https://w3id.org/pmd/mo/ScanningTransmissionElectronMicroscopy> ;
                                                                                                rdfs:isDefinedBy <https://w3id.org/pmd/mo> ;
                                                                                                rdfs:label "Rastertransmissionselektronenmikroskopie Elektronen-Energieverlust-Spektroskopie"@de ,
                                                                                                           "Scanning Transmission Electron Microscopy Electron Energy Loss Spectroscopy"@en ;
                                                                                                <http://www.w3.org/2004/02/skos/core#definition> "STEM-EELS combines STEM imaging with electron energy loss spectroscopy to provide information about the elemental composition and electronic structure of a sample at high spatial resolution."@en ;
                                                                                                <https://w3id.org/pmd/co/definitionSource> "ChatGPT 3.5"@en ;
                                                                                                <https://w3id.org/pmd/mo/abbreviation> "STEM-EELS"@en .


###  https://w3id.org/pmd/mo/ScanningTunnelingMicroscope
<https://w3id.org/pmd/mo/ScanningTunnelingMicroscope> rdf:type owl:Class ;
                                                      rdfs:subClassOf <https://w3id.org/pmd/mo/ScanningProbeMicroscope> ;
                                                      rdfs:isDefinedBy <https://w3id.org/pmd/mo> ;
                                                      rdfs:label "Rastertunnelmikroskop"@de ,
                                                                 "Scanning Tunneling Microscope"@en ;
                                                      <http://www.w3.org/2004/02/skos/core#definition> "A microscope that uses quantum tunneling to image surfaces at the atomic level."@en ,
                                                                                                       "Ein Mikroskop, das Quanten-Tunneling nutzt, um Oberflächen auf atomarer Ebene abzubilden."@de ;
                                                      <https://w3id.org/pmd/co/definitionSource> "ChatGPT 3.5"@en ;
                                                      <https://w3id.org/pmd/mo/abbreviation> "STM"@en .


###  https://w3id.org/pmd/mo/ScanningTunnelingMicroscopy
<https://w3id.org/pmd/mo/ScanningTunnelingMicroscopy> rdf:type owl:Class ;
                                                      rdfs:subClassOf <https://w3id.org/pmd/mo/ScanningProbeMicroscopy> ;
                                                      rdfs:isDefinedBy <https://w3id.org/pmd/mo> ;
                                                      rdfs:label "Rastertunnelmikroskopie"@de ,
                                                                 "Scanning Tunneling Microscopy"@en ;
                                                      <http://www.w3.org/2004/02/skos/core#definition> "Scanning Tunneling Microscopy is a technique that uses a conducting probe to measure the tunneling current between the probe and the sample's surface. It provides atomic-scale images of surfaces and is often used to study conductive materials."@en ;
                                                      <https://w3id.org/pmd/co/definitionSource> "ChatGPT 3.5"@en ;
                                                      <https://w3id.org/pmd/mo/abbreviation> "STM"@en .


###  https://w3id.org/pmd/mo/SchottkyEmissionGun
<https://w3id.org/pmd/mo/SchottkyEmissionGun> rdf:type owl:Class ;
                                              rdfs:subClassOf <https://w3id.org/pmd/mo/Gun> ;
                                              <http://purl.obolibrary.org/obo/IAO_0000117> "PMDco Team"@en ;
                                              <http://purl.obolibrary.org/obo/IAO_0000119> "ChatGPT 3.5"@en ;
                                              rdfs:label "Schottky Emission Gun"@en ,
                                                         "Schottky-Emissionsquelle"@de ;
                                              <http://www.w3.org/2004/02/skos/core#definition> "A Schottky Emission Gun is a device in electron microscopes that produces electrons by field-induced thermionic emission, using a Schottky emitter."@en ,
                                                                                               "Eine Schottky-Emissionsquelle ist ein Gerät in Elektronenmikroskopen, das durch feldinduzierte thermionische Emission Elektronen erzeugt und einen Schottky-Emitter verwendet."@de .


###  https://w3id.org/pmd/mo/Scintillator
<https://w3id.org/pmd/mo/Scintillator> rdf:type owl:Class ;
                                       rdfs:subClassOf <https://w3id.org/pmd/mo/Detector> ;
                                       rdfs:isDefinedBy <https://w3id.org/pmd/mo> ;
                                       rdfs:label "Scintillator"@en ,
                                                  "Szintillator"@de ;
                                       <http://www.w3.org/2004/02/skos/core#definition> "A material that emits light when it absorbs ionizing radiation."@en ,
                                                                                        "Ein Material, das Licht aussendet, wenn es ionisierende Strahlung absorbiert."@de ;
                                       <https://w3id.org/pmd/co/definitionSource> "ChatGPT 3.5"@en .


###  https://w3id.org/pmd/mo/SecondaryIonMassSpectrometry
<https://w3id.org/pmd/mo/SecondaryIonMassSpectrometry> rdf:type owl:Class ;
                                                       rdfs:subClassOf <https://w3id.org/pmd/mo/Spectroscopy> ;
                                                       rdfs:isDefinedBy <https://w3id.org/pmd/mo> ;
                                                       rdfs:label "Secondary Ion Mass Spectrometry"@en ,
                                                                  "Sekundärionen-Massenspektrometrie"@de ;
                                                       <http://www.w3.org/2004/02/skos/core#definition> """Secondary Ion Mass Spectrometry (SIMS) is an advanced analytical technique used to determine the elemental and isotopic composition of solid surfaces and thin films at a very high sensitivity and spatial resolution. It is widely employed in various scientific and industrial applications, including materials science, semiconductor research, and surface analysis.
In SIMS, a focused beam of high-energy primary ions is directed at a sample's surface. The impact of these primary ions causes the ejection of secondary ions from the sample's surface. These secondary ions are then extracted, mass-separated, and detected using a mass spectrometer. The mass spectrometer measures the mass-to-charge ratios of the secondary ions, providing information about the elemental and isotopic composition of the sample.
The sensitivity and spatial resolution of SIMS allow researchers to analyze very small areas, often down to the micrometer or nanometer scale. This makes SIMS particularly valuable for investigating surface composition, depth profiling of layered structures, and detecting trace elements in complex materials. The technique is non-destructive in its elemental analysis, which is beneficial for studying delicate samples or preserving valuable materials.
SIMS has applications in diverse fields, including materials characterization, semiconductor device analysis, biological and medical research, and geological studies. It provides essential information about the chemical composition, structure, and distribution of elements in complex samples, contributing to advancements in materials science and various technological developments."""@en ;
                                                       <https://w3id.org/pmd/co/definitionSource> "ChatGPT 3.5"@en ;
                                                       <https://w3id.org/pmd/mo/abbreviation> "SIMS"@en .


###  https://w3id.org/pmd/mo/SelectedAreaElectronDiffraction
<https://w3id.org/pmd/mo/SelectedAreaElectronDiffraction> rdf:type owl:Class ;
                                                          rdfs:subClassOf <https://w3id.org/pmd/mo/ElectronDiffraction> ;
                                                          rdfs:isDefinedBy <https://w3id.org/pmd/mo> ;
                                                          rdfs:label "Elektronenbeugung ausgewählter Regionen"@de ,
                                                                     "Selected Area Electron Diffraction"@en ;
                                                          <http://www.w3.org/2004/02/skos/core#definition> "Selected Area Electron Diffraction is a technique used in transmission electron microscopy (TEM) to study the crystallographic orientation of small regions within a sample. By selecting a specific area of the sample and directing an electron beam onto it, diffraction patterns are generated. These patterns offer insights into the sample's crystal structure and orientation."@en ;
                                                          <https://w3id.org/pmd/co/definitionSource> "ChatGPT 3.5"@en ;
                                                          <https://w3id.org/pmd/mo/abbreviation> "SAD"@en ,
                                                                                                 "SAED"@en .


###  https://w3id.org/pmd/mo/Sharpness
<https://w3id.org/pmd/mo/Sharpness> rdf:type owl:Class ;
                                    rdfs:subClassOf <https://w3id.org/pmd/co/ValueObject> ;
                                    rdfs:isDefinedBy <https://w3id.org/pmd/mo> ;
                                    rdfs:label "Schärfe"@de ,
                                               "Sharpness"@en ;
                                    <http://www.w3.org/2004/02/skos/core#definition> "Die Qualität, klar und gut definiert in einem Bild oder einer Probe zu sein."@de ,
                                                                                     "The quality of being clear and well-defined in an image or specimen."@en ;
                                    <https://w3id.org/pmd/co/definitionSource> "ChatGPT 3.5"@en .


###  https://w3id.org/pmd/mo/SiliconDriftDetector
<https://w3id.org/pmd/mo/SiliconDriftDetector> rdf:type owl:Class ;
                                               rdfs:subClassOf <https://w3id.org/pmd/mo/Detector> ;
                                               rdfs:isDefinedBy <https://w3id.org/pmd/mo> ;
                                               rdfs:label "Silicon Drift Detector"@en ,
                                                          "Silizium-Driftdetektor"@de ;
                                               <http://www.w3.org/2004/02/skos/core#definition> "A type of X-ray detector that offers high-speed performance and high energy resolution."@en ,
                                                                                                "Eine Art Röntgendetektor, der Hochgeschwindigkeitsleistung und hohe Energieauflösung bietet."@de ;
                                               <https://w3id.org/pmd/co/definitionSource> "ChatGPT 3.5"@en ;
                                               <https://w3id.org/pmd/mo/abbreviation> "SDD"@en .


###  https://w3id.org/pmd/mo/SoftXRayEmissionSpectrometer
<https://w3id.org/pmd/mo/SoftXRayEmissionSpectrometer> rdf:type owl:Class ;
                                                       rdfs:subClassOf <https://w3id.org/pmd/mo/Spectrometer> ;
                                                       rdfs:isDefinedBy <https://w3id.org/pmd/mo> ;
                                                       rdfs:label "Röntgenemissionsspektrometer mit weicher Röntgenstrahlung"@de ,
                                                                  "Soft X-ray Emission Spectrometer"@en ;
                                                       <http://www.w3.org/2004/02/skos/core#definition> "An instrument used to analyze the emission of soft X-rays from a sample."@en ,
                                                                                                        "Ein Instrument zur Analyse der Emission weicher Röntgenstrahlen aus einer Probe."@de ;
                                                       <https://w3id.org/pmd/co/definitionSource> "ChatGPT 3.5"@en ;
                                                       <https://w3id.org/pmd/mo/abbreviation> "SXES"@en .


###  https://w3id.org/pmd/mo/Source
<https://w3id.org/pmd/mo/Source> rdf:type owl:Class ;
                                 rdfs:subClassOf <https://w3id.org/pmd/co/ProcessingNode> ;
                                 rdfs:isDefinedBy <https://w3id.org/pmd/mo> ;
                                 rdfs:label "Quelle"@de ,
                                            "Source"@en ;
                                 <http://www.w3.org/2004/02/skos/core#definition> "Die Elektronenquelle, z. B. ein Wolframfaden oder eine Feldemissionskathode, die in einem Elektronenmikroskop Elektronen emittiert."@de ,
                                                                                  "The electron source, such as a tungsten filament or field-emission cathode, that emits electrons in an electron microscope."@en ;
                                 <https://w3id.org/pmd/co/definitionSource> "ChatGPT 3.5" .


###  https://w3id.org/pmd/mo/SpatialResolution
<https://w3id.org/pmd/mo/SpatialResolution> rdf:type owl:Class ;
                                            rdfs:subClassOf <https://w3id.org/pmd/mo/Resolution> ;
                                            rdfs:isDefinedBy <https://w3id.org/pmd/mo> ;
                                            rdfs:label "Ortsauflösung"@de ,
                                                       "Spatial Resolution"@en ;
                                            <http://www.w3.org/2004/02/skos/core#definition> "Die Fähigkeit eines Bildgebungssystems, feine Details in einem Objekt anzuzeigen. Sie bezieht sich auf das kleinste wahrnehmbare Detail in einem Bild."@de ,
                                                                                             "The ability of an imaging system to discern fine details in an object. It refers to the smallest discernible detail in an image."@en ;
                                            <https://w3id.org/pmd/co/definitionSource> "ChatGPT 3.5"@en .


###  https://w3id.org/pmd/mo/Spectrometer
<https://w3id.org/pmd/mo/Spectrometer> rdf:type owl:Class ;
                                       rdfs:subClassOf <https://w3id.org/pmd/mo/Detector> ;
                                       rdfs:isDefinedBy <https://w3id.org/pmd/mo> ;
                                       rdfs:label "Spectrometer"@en ,
                                                  "Spektrometer"@de ;
                                       <http://www.w3.org/2004/02/skos/core#definition> "An instrument used to measure properties of light over a specific portion of the electromagnetic spectrum."@en ,
                                                                                        "Ein Instrument zur Messung der Eigenschaften von Licht in einem bestimmten Teil des elektromagnetischen Spektrums."@de ;
                                       <https://w3id.org/pmd/co/definitionSource> "ChatGPT 3.5"@en .


###  https://w3id.org/pmd/mo/Spectroscopy
<https://w3id.org/pmd/mo/Spectroscopy> rdf:type owl:Class ;
                                       rdfs:subClassOf <https://w3id.org/pmd/co/AnalysingProcess> ;
                                       rdfs:isDefinedBy <https://w3id.org/pmd/mo> ;
                                       <http://www.w3.org/2004/02/skos/core#altLabel> "Spectrometry"@en ,
                                                                                      "Spektrometrie"@de ;
                                       <http://www.w3.org/2004/02/skos/core#definition> "Spectroscopy is a scientific technique used to study and analyze the interaction of matter with electromagnetic radiation, such as light. It involves measuring the way in which different substances absorb, emit, or scatter light at various wavelengths or frequencies. By examining the spectrum of light emitted, absorbed, or transmitted by a sample, scientists can gain insights into its chemical composition, molecular structure, and physical properties. Spectroscopy is widely utilized in various fields, including chemistry, physics, astronomy, and biochemistry, to investigate the characteristics and behavior of materials at the atomic and molecular level."@en ;
                                       <http://www.w3.org/2004/02/skos/core#prefLabel> "Spectroscopy"@en ,
                                                                                       "Spektroskopie"@de ;
                                       <https://w3id.org/pmd/co/definitionSource> "ChatGPT 3.5"@en .


###  https://w3id.org/pmd/mo/SphericalAberration
<https://w3id.org/pmd/mo/SphericalAberration> rdf:type owl:Class ;
                                              rdfs:subClassOf <https://w3id.org/pmd/mo/Aberration> ;
                                              rdfs:isDefinedBy <https://w3id.org/pmd/mo> ;
                                              rdfs:label "Spherical Aberration"@en ,
                                                         "Sphärische Aberration"@de ;
                                              <http://www.w3.org/2004/02/skos/core#definition> "A type of optical aberration caused by deviations from the ideal spherical shape in lenses or mirrors."@en ,
                                                                                               "Eine Art von optischer Aberration, die durch Abweichungen von der idealen sphärischen Form in Linsen oder Spiegeln verursacht wird."@de ;
                                              <https://w3id.org/pmd/co/definitionSource> "ChatGPT 3.5"@en .


###  https://w3id.org/pmd/mo/Spot
<https://w3id.org/pmd/mo/Spot> rdf:type owl:Class ;
                               rdfs:subClassOf <https://w3id.org/pmd/co/Object> ;
                               <http://purl.obolibrary.org/obo/IAO_0000117> "PMDco Team"@en ;
                               <http://purl.obolibrary.org/obo/IAO_0000119> "ChatGPT 3.5"@en ;
                               rdfs:label "Spot"@de ,
                                          "Spot"@en ,
                                          "Strahlfleck"@de ;
                               <http://www.w3.org/2004/02/skos/core#definition> "Spot refers to the focused point of the electron beam in an electron microscope, where the beam interacts with the specimen."@en ,
                                                                                "Strahlfleck bezieht sich auf den fokussierten Punkt des Elektronenstrahls in einem Elektronenmikroskop, an dem der Strahl mit der Probe interagiert."@de .


###  https://w3id.org/pmd/mo/SpotSize
<https://w3id.org/pmd/mo/SpotSize> rdf:type owl:Class ;
                                   rdfs:subClassOf <https://w3id.org/pmd/co/ValueObject> ;
                                   <http://purl.obolibrary.org/obo/IAO_0000117> "PMDco Team"@en ;
                                   <http://purl.obolibrary.org/obo/IAO_0000119> "ChatGPT 3.5"@en ;
                                   rdfs:label "Spot Size"@en ,
                                              "Spotgröße"@de ,
                                              "Strahlfleckgröße"@de ;
                                   <http://www.w3.org/2004/02/skos/core#definition> "Spot Size refers to the diameter of the electron beam at the point where it is focused on the specimen in an electron microscope."@en ,
                                                                                    "Strahlfleckgröße bezieht sich auf den Durchmesser des Elektronenstrahls an dem Punkt, an dem er auf die Probe fokussiert wird."@de .


###  https://w3id.org/pmd/mo/Stage
<https://w3id.org/pmd/mo/Stage> rdf:type owl:Class ;
                                rdfs:subClassOf <https://w3id.org/pmd/co/Component> ;
                                rdfs:isDefinedBy <https://w3id.org/pmd/mo> ;
                                rdfs:label "Bühne"@de ,
                                           "Stage"@en ;
                                <http://www.w3.org/2004/02/skos/core#definition> "A platform or support used to hold and position a specimen in a microscope."@en ,
                                                                                 "Eine Plattform oder Unterstützung, die verwendet wird, um eine Probe in einem Mikroskop zu halten und zu positionieren."@de ;
                                <https://w3id.org/pmd/co/definitionSource> "ChatGPT 3.5"@en .


###  https://w3id.org/pmd/mo/StigmationX
<https://w3id.org/pmd/mo/StigmationX> rdf:type owl:Class ;
                                      rdfs:subClassOf <https://w3id.org/pmd/co/ValueObject> ;
                                      rdfs:isDefinedBy <https://w3id.org/pmd/mo> ;
                                      rdfs:label "Stigmation X"@de ,
                                                 "Stigmation X"@en ;
                                      <http://www.w3.org/2004/02/skos/core#altLabel> "Stigmator X Value"@en ,
                                                                                     "Stigmator X Wert"@de ;
                                      <http://www.w3.org/2004/02/skos/core#definition> "Die Einstellung des Astigmatismus in der X-Achse eines Elektronenstrahls in der Mikroskopie."@de ,
                                                                                       "The adjustment of astigmatism in the X-axis of an electron beam in microscopy."@en ;
                                      <https://w3id.org/pmd/co/definitionSource> "ChatGPT 3.5"@en .


###  https://w3id.org/pmd/mo/StigmationY
<https://w3id.org/pmd/mo/StigmationY> rdf:type owl:Class ;
                                      rdfs:subClassOf <https://w3id.org/pmd/co/ValueObject> ;
                                      rdfs:isDefinedBy <https://w3id.org/pmd/mo> ;
                                      rdfs:label "Stigmation Y"@de ,
                                                 "Stigmation Y"@en ;
                                      <http://www.w3.org/2004/02/skos/core#altLabel> "Stigmator X Wert"@de ,
                                                                                     "Stigmator Y Value"@en ;
                                      <http://www.w3.org/2004/02/skos/core#definition> "Die Einstellung des Astigmatismus in der Y-Achse eines Elektronenstrahls in der Mikroskopie."@de ,
                                                                                       "The adjustment of astigmatism in the Y-axis of an electron beam in microscopy."@en ;
                                      <https://w3id.org/pmd/co/definitionSource> "ChatGPT 3.5"@en .


###  https://w3id.org/pmd/mo/Stigmator
<https://w3id.org/pmd/mo/Stigmator> rdf:type owl:Class ;
                                    rdfs:subClassOf <https://w3id.org/pmd/co/ProcessingNode> ;
                                    rdfs:isDefinedBy <https://w3id.org/pmd/mo> ;
                                    rdfs:label "Stigmator"@de ,
                                               "Stigmator"@en ;
                                    <http://www.w3.org/2004/02/skos/core#definition> "A device in electron microscopy used to correct astigmatism in the electron beam."@en ,
                                                                                     "Ein Gerät in der Elektronenmikroskopie zur Korrektur des Astigmatismus im Elektronenstrahl."@de ;
                                    <https://w3id.org/pmd/co/definitionSource> "ChatGPT 3.5"@en .


###  https://w3id.org/pmd/mo/SurfaceStructure
<https://w3id.org/pmd/mo/SurfaceStructure> rdf:type owl:Class ;
                                           rdfs:subClassOf <https://w3id.org/pmd/co/Object> ;
                                           rdfs:isDefinedBy <https://w3id.org/pmd/mo> ;
                                           rdfs:label "Oberflächenstruktur"@de ,
                                                      "Surface Structure"@en ;
                                           <http://www.w3.org/2004/02/skos/core#definition> "Die Anordnung und die Merkmale der äußersten Schicht eines Materials."@de ,
                                                                                            "The arrangement and features of the outermost layer of a material."@en ;
                                           <https://w3id.org/pmd/co/definitionSource> "ChatGPT 3.5"@en .


###  https://w3id.org/pmd/mo/SystemVacuum
<https://w3id.org/pmd/mo/SystemVacuum> rdf:type owl:Class ;
                                       rdfs:subClassOf <https://w3id.org/pmd/mo/Vacuum> ;
                                       rdfs:isDefinedBy <https://w3id.org/pmd/mo> ;
                                       rdfs:label "System Vacuum"@en ,
                                                  "Systemvakuum"@de ;
                                       <http://www.w3.org/2004/02/skos/core#definition> "Das allgemeine Vakuumniveau im gesamten System eines Elektronenmikroskops."@de ,
                                                                                        "The overall vacuum level in the entire system of an electron microscope."@en ;
                                       <https://w3id.org/pmd/co/definitionSource> "ChatGPT 3.5"@en .


###  https://w3id.org/pmd/mo/TemporalResolution
<https://w3id.org/pmd/mo/TemporalResolution> rdf:type owl:Class ;
                                             rdfs:subClassOf <https://w3id.org/pmd/mo/Resolution> ;
                                             <http://purl.obolibrary.org/obo/IAO_0000117> "PMDco Team"@en ;
                                             <http://purl.obolibrary.org/obo/IAO_0000119> "ChatGPT 3.5"@en ;
                                             rdfs:label "Temporal Resolution"@en ,
                                                        "Zeitliche Auflösung"@de ;
                                             <http://www.w3.org/2004/02/skos/core#definition> "Temporal Resolution is the ability of a microscopy or imaging system to distinguish between events or changes occurring at different times, critical in capturing dynamic processes."@en ,
                                                                                              "Zeitliche Auflösung ist die Fähigkeit eines Mikroskopie- oder Bildgebungssystems, zwischen Ereignissen oder Änderungen zu unterscheiden, die zu unterschiedlichen Zeiten auftreten, was entscheidend für die Erfassung dynamischer Prozesse ist."@de .


###  https://w3id.org/pmd/mo/ThermionicEmissionGun
<https://w3id.org/pmd/mo/ThermionicEmissionGun> rdf:type owl:Class ;
                                                rdfs:subClassOf <https://w3id.org/pmd/mo/Gun> ;
                                                <http://purl.obolibrary.org/obo/IAO_0000117> "PMDco Team"@en ;
                                                <http://purl.obolibrary.org/obo/IAO_0000119> "ChatGPT 3.5"@en ;
                                                rdfs:label "Thermionic Emission Gun"@en ,
                                                           "Thermionische Emissionsquelle"@de ;
                                                <http://www.w3.org/2004/02/skos/core#definition> "A Thermionic Emission Gun is a device in electron microscopes that produces electrons by heating a filament to emit electrons through thermionic emission."@en ,
                                                                                                 "Eine thermionische Emissionsquelle ist ein Gerät in Elektronenmikroskopen, das durch Erhitzen eines Filaments Elektronen durch thermionische Emission erzeugt."@de .


###  https://w3id.org/pmd/mo/ThinFoilAperture
<https://w3id.org/pmd/mo/ThinFoilAperture> rdf:type owl:Class ;
                                           rdfs:subClassOf <https://w3id.org/pmd/mo/Aperture> ;
                                           rdfs:isDefinedBy <https://w3id.org/pmd/mo> ;
                                           rdfs:label "Dünnfolienblende"@de ,
                                                      "Thin Foil Aperture"@en ;
                                           <http://www.w3.org/2004/02/skos/core#definition> "An aperture used in electron microscopy to control the electron beam passing through a thin foil specimen."@en ,
                                                                                            "Eine Blende in der Elektronenmikroskopie zur Steuerung des Elektronenstrahls, der durch eine Dünnfolienprobe geht."@de ;
                                           <https://w3id.org/pmd/co/definitionSource> "ChatGPT 3.5"@en .


###  https://w3id.org/pmd/mo/Threshold
<https://w3id.org/pmd/mo/Threshold> rdf:type owl:Class ;
                                    rdfs:subClassOf <https://w3id.org/pmd/co/ValueObject> ;
                                    rdfs:isDefinedBy <https://w3id.org/pmd/mo> ;
                                    rdfs:label "Schwelle"@de ,
                                               "Threshold"@en ;
                                    <http://www.w3.org/2004/02/skos/core#definition> "A value or limit at which a specific effect or result occurs."@en ,
                                                                                     "Ein Wert oder eine Grenze, bei der ein bestimmter Effekt oder ein Ergebnis eintritt."@de ;
                                    <https://w3id.org/pmd/co/definitionSource> "ChatGPT 3.5"@en .


###  https://w3id.org/pmd/mo/TiltAngle
<https://w3id.org/pmd/mo/TiltAngle> rdf:type owl:Class ;
                                    rdfs:subClassOf <https://w3id.org/pmd/mo/Angle> ;
                                    rdfs:isDefinedBy <https://w3id.org/pmd/mo> ;
                                    rdfs:label "Neigungswinkel"@de ,
                                               "Tilt Angle"@en ;
                                    <http://www.w3.org/2004/02/skos/core#definition> "Der Winkel, um den ein Objekt von seiner vertikalen oder horizontalen Position geneigt ist."@de ,
                                                                                     "The angle at which an object is tilted from its vertical or horizontal position."@en ;
                                    <https://w3id.org/pmd/co/definitionSource> "ChatGPT 3.5"@en .


###  https://w3id.org/pmd/mo/TiltCorrection
<https://w3id.org/pmd/mo/TiltCorrection> rdf:type owl:Class ;
                                         rdfs:subClassOf <https://w3id.org/pmd/co/AnalysingProcess> ;
                                         rdfs:isDefinedBy <https://w3id.org/pmd/mo> ;
                                         rdfs:label "Neigungskorrektur"@de ,
                                                    "Tilt Correction"@en ;
                                         <http://www.w3.org/2004/02/skos/core#definition> "A correction applied to images obtained from tilted specimens in electron microscopy to compensate for distortions caused by the tilt angle."@en ,
                                                                                          "Eine Korrektur, die bei Bildern von gekippten Proben in der Elektronenmikroskopie angewendet wird, um durch den Kippwinkel verursachte Verzerrungen zu kompensieren."@de ;
                                         <https://w3id.org/pmd/co/definitionSource> "ChatGPT 3.5" .


###  https://w3id.org/pmd/mo/TimeOfFlightSecondaryIonMassSpectrometry
<https://w3id.org/pmd/mo/TimeOfFlightSecondaryIonMassSpectrometry> rdf:type owl:Class ;
                                                                   rdfs:subClassOf <https://w3id.org/pmd/mo/Spectroscopy> ;
                                                                   rdfs:isDefinedBy <https://w3id.org/pmd/mo> ;
                                                                   rdfs:label "Flugzeit-Sekundärionen-Massenspektrometrie"@de ,
                                                                              "Time Of Flight Secondary Ion Mass Spectrometry"@en ;
                                                                   <http://www.w3.org/2004/02/skos/core#definition> """Time-of-Flight Secondary Ion Mass Spectrometry (TOF-SIMS) is an advanced surface analysis technique used to determine the elemental and molecular composition of solid surfaces and thin films with high sensitivity and spatial resolution. It is employed in various scientific and industrial fields, including materials science, nanotechnology, biomedicine, and semiconductor research.
TOF-SIMS builds upon the principles of Secondary Ion Mass Spectrometry (SIMS), where a focused beam of high-energy primary ions is directed at a sample's surface, causing the ejection of secondary ions. In TOF-SIMS, the flight time of these secondary ions is measured as they travel through a field-free region and enter a time-of-flight mass spectrometer. The mass spectrometer measures the time taken by the ions to reach the detector, which is directly proportional to their mass-to-charge ratio.
By analyzing the flight times of the secondary ions, TOF-SIMS can determine the elemental, isotopic, and molecular composition of the sample's surface. It provides information about the presence of specific elements, chemical compounds, and molecular fragments, along with their spatial distribution. The high sensitivity of TOF-SIMS allows for the detection of trace elements and molecular species in complex samples.
TOF-SIMS is valuable for characterizing surfaces at the nanoscale, profiling layered structures, investigating organic and inorganic materials, and studying biological specimens. Its ability to provide detailed chemical information while maintaining spatial resolution makes it an essential tool for understanding surface properties and material interactions in a wide range of applications."""@en ;
                                                                   <https://w3id.org/pmd/co/definitionSource> "ChatGPT 3.5"@en ;
                                                                   <https://w3id.org/pmd/mo/abbreviation> "TOF-SIMS"@en .


###  https://w3id.org/pmd/mo/TomographicReconstruction
<https://w3id.org/pmd/mo/TomographicReconstruction> rdf:type owl:Class ;
                                                    rdfs:subClassOf <https://w3id.org/pmd/mo/Reconstruction> ;
                                                    rdfs:isDefinedBy <https://w3id.org/pmd/mo> ;
                                                    rdfs:label "Tomographic Reconstruction"@en ,
                                                               "Tomographische Rekonstruktion"@de ;
                                                    <http://www.w3.org/2004/02/skos/core#definition> "Der Prozess der Rekonstruktion einer dreidimensionalen Struktur aus einer Reihe von zweidimensionalen Bildern, die aus verschiedenen Winkeln aufgenommen wurden."@de ,
                                                                                                     "The process of reconstructing a three-dimensional structure from a series of two-dimensional images taken at different angles."@en ;
                                                    <https://w3id.org/pmd/co/definitionSource> "ChatGPT 3.5"@en .


###  https://w3id.org/pmd/mo/TransmissionElectronAberrationCorrectedMicroscope
<https://w3id.org/pmd/mo/TransmissionElectronAberrationCorrectedMicroscope> rdf:type owl:Class ;
                                                                            rdfs:subClassOf <https://w3id.org/pmd/mo/TransmissionElectronMicroscope> ;
                                                                            rdfs:isDefinedBy <https://w3id.org/pmd/mo> ;
                                                                            rdfs:label "Transmission Electron Aberration-corrected Microscope"@en ,
                                                                                       "Transmissionselektronen-Aberrations-korrigiertes Mikroskop"@de ;
                                                                            <http://www.w3.org/2004/02/skos/core#definition> "A transmission electron microscope equipped with aberration correction to achieve high-resolution imaging."@en ,
                                                                                                                             "Ein Transmissions-Elektronenmikroskop mit Aberrationskorrektur zur Erzielung hochauflösender Bilder."@de ;
                                                                            <https://w3id.org/pmd/co/definitionSource> "ChatGPT 3.5"@en ;
                                                                            <https://w3id.org/pmd/mo/abbreviation> "TEAM"@en .


###  https://w3id.org/pmd/mo/TransmissionElectronMicroscope
<https://w3id.org/pmd/mo/TransmissionElectronMicroscope> rdf:type owl:Class ;
                                                         rdfs:subClassOf <https://w3id.org/pmd/co/ElectronMicroscope> ;
                                                         rdfs:isDefinedBy <https://w3id.org/pmd/mo> ;
                                                         rdfs:label "Transmission Electron Microscope"@en ,
                                                                    "Transmissionelektronenmikroskop"@de ;
                                                         <http://www.w3.org/2004/02/skos/core#definition> "A microscope that transmits a beam of electrons through a specimen, forming an image."@en ,
                                                                                                          "Ein Mikroskop, das einen Elektronenstrahl durch eine Probe sendet und ein Bild erzeugt."@de ;
                                                         <https://w3id.org/pmd/co/definitionSource> "ChatGPT 3.5"@en ;
                                                         <https://w3id.org/pmd/mo/abbreviation> "TEM" .


###  https://w3id.org/pmd/mo/TransmissionElectronMicroscopy
<https://w3id.org/pmd/mo/TransmissionElectronMicroscopy> rdf:type owl:Class ;
                                                         rdfs:subClassOf <https://w3id.org/pmd/co/ElectronMicroscopy> ;
                                                         rdfs:isDefinedBy <https://w3id.org/pmd/mo> ;
                                                         <http://www.w3.org/2004/02/skos/core#definition> "Transmission Electron Microscopy is a microscopy technique that involves transmitting a beam of electrons through a thin sample to create high-resolution images. It is used to study the internal structure and morphology of materials at the nanometer scale."@en ;
                                                         <https://w3id.org/pmd/co/definitionSource> "ChatGPT 3.5"@en ;
                                                         <https://w3id.org/pmd/mo/abbreviation> "TEM"@en .


###  https://w3id.org/pmd/mo/Vacuum
<https://w3id.org/pmd/mo/Vacuum> rdf:type owl:Class ;
                                 rdfs:subClassOf <https://w3id.org/pmd/co/Object> ;
                                 rdfs:isDefinedBy <https://w3id.org/pmd/mo> ;
                                 rdfs:label "Vacuum"@en ,
                                            "Vakuum"@de ;
                                 <http://www.w3.org/2004/02/skos/core#definition> "A space entirely devoid of matter, or where the pressure is significantly lower than atmospheric pressure."@en ,
                                                                                  "Ein Raum, der völlig materiefrei ist oder in dem der Druck deutlich unter dem atmosphärischen Druck liegt."@de ;
                                 <https://w3id.org/pmd/co/definitionSource> "ChatGPT 3.5"@en .


###  https://w3id.org/pmd/mo/VacuumPump
<https://w3id.org/pmd/mo/VacuumPump> rdf:type owl:Class ;
                                     rdfs:subClassOf <https://w3id.org/pmd/co/ProcessingNode> ;
                                     <http://purl.obolibrary.org/obo/IAO_0000117> "PMDco Team"@en ;
                                     <http://purl.obolibrary.org/obo/IAO_0000119> "ChatGPT 3.5"@en ;
                                     rdfs:label "Vacuum Pump"@en ,
                                                "Vakuumpumpe"@de ;
                                     <http://www.w3.org/2004/02/skos/core#definition> "A Vacuum Pump is a device used in electron microscopes to evacuate air from the chamber, creating the necessary vacuum conditions for electron beam operation."@en ,
                                                                                      "Eine Vakuumpumpe ist ein Gerät, das in Elektronenmikroskopen verwendet wird, um Luft aus der Kammer zu evakuieren und die notwendigen Vakuumbedingungen für den Betrieb des Elektronenstrahls zu schaffen."@de .


###  https://w3id.org/pmd/mo/VerticalFieldWidth
<https://w3id.org/pmd/mo/VerticalFieldWidth> rdf:type owl:Class ;
                                             rdfs:subClassOf <https://w3id.org/pmd/mo/FieldWidth> ;
                                             <http://purl.obolibrary.org/obo/IAO_0000117> "PMDco Team"@en ;
                                             <http://purl.obolibrary.org/obo/IAO_0000119> "ChatGPT 3.5"@en ;
                                             rdfs:label "Vertical Field Width"@en ,
                                                        "Vertikale Feldbreite"@de ;
                                             <http://www.w3.org/2004/02/skos/core#definition> "Vertical Field Width refers to the vertical extent of the observable field in an electron microscope."@en ,
                                                                                              "Vertikale Feldbreite bezieht sich auf den vertikalen Umfang des beobachtbaren Feldes in einem Elektronenmikroskop."@de .


###  https://w3id.org/pmd/mo/Voltage
<https://w3id.org/pmd/mo/Voltage> rdf:type owl:Class ;
                                  rdfs:subClassOf <https://w3id.org/pmd/co/ValueObject> ;
                                  rdfs:comment "Die Spannung wird in Volt (V) gemessen und in Kilovolt (kV) repräsentiert und stellt die potenzielle Energiedifferenz zwischen zwei Punkten in einem Stromkreis dar. Je höher die Spannung ist, desto größer ist die Kraft, die die elektrischen Ladungen antreibt, und desto höher ist folglich auch das Potenzial für einen Stromfluss."@de ,
                                               "Voltage is measured in volts (V) and typically represented in kilovolts (kV), and it represents the potential energy difference between two points in a circuit. The higher the voltage, the greater the force pushing the electric charges, and consequently, the higher the potential for current to flow."@en ;
                                  rdfs:isDefinedBy <https://w3id.org/pmd/mo> ;
                                  rdfs:label "Spannung"@de ,
                                             "Voltage"@en ;
                                  <http://www.w3.org/2004/02/skos/core#altLabel> "Stromspannung"@de ;
                                  <http://www.w3.org/2004/02/skos/core#definition> "Die Spannung, auch elektrische Potentialdifferenz, ist ein Maß für die elektrische potentielle Energie pro Ladungseinheit in einem elektrischen Stromkreis. Sie ist die Kraft, die den elektrischen Strom durch einen Leiter treibt."@de ,
                                                                                   "Voltage, also known as electric potential difference, is a measure of the electric potential energy per unit charge in an electrical circuit. It is the force or pressure that drives electric current through a conductor."@en ;
                                  <https://w3id.org/pmd/co/definitionSource> "ChatGPT 3.5"@en .


###  https://w3id.org/pmd/mo/Volume
<https://w3id.org/pmd/mo/Volume> rdf:type owl:Class ;
                                 rdfs:subClassOf <https://w3id.org/pmd/co/ValueObject> ;
                                 rdfs:isDefinedBy <https://w3id.org/pmd/mo> ;
                                 rdfs:label "Volume"@en ,
                                            "Volumen"@de ;
                                 <http://www.w3.org/2004/02/skos/core#definition> "Die Menge an Raum, die ein Stoff oder Gegenstand einnimmt."@de ,
                                                                                  "The amount of space that a substance or object occupies."@en ;
                                 <https://w3id.org/pmd/co/definitionSource> "ChatGPT 3.5"@en .


###  https://w3id.org/pmd/mo/WaitTime
<https://w3id.org/pmd/mo/WaitTime> rdf:type owl:Class ;
                                   rdfs:subClassOf <https://w3id.org/pmd/co/Duration> ;
                                   rdfs:comment "Die Wartezeit wird häufig genutzt, um die Probe zu stabilisieren oder um die Beschädigung der Probe zu minimieren."@de ,
                                                "The wait time is often used to allow the specimen to stabilize or to minimize sample damage."@en ;
                                   rdfs:isDefinedBy <https://w3id.org/pmd/mo> ;
                                   rdfs:label "Wait Time"@en ,
                                              "Wartezeit"@de ;
                                   <http://www.w3.org/2004/02/skos/core#definition> "Das Zeitintervall zwischen aufeinander folgenden Messungen oder Operationen in einem Elektronenmikroskop."@de ,
                                                                                    "The time interval between successive measurements or operations in an electron microscope."@en ;
                                   <https://w3id.org/pmd/co/definitionSource> "ChatGPT 3.5" .


###  https://w3id.org/pmd/mo/WorkingDistance
<https://w3id.org/pmd/mo/WorkingDistance> rdf:type owl:Class ;
                                          rdfs:subClassOf <https://w3id.org/pmd/co/Distance> ;
                                          rdfs:comment "Der Arbeitsabstand wirkt sich auf die Tiefenschärfe und die Auflösung des Bildes aus. In der Regel wird der Arbeitsabstand in Millimetern (mm) angegeben."@de ,
                                                       "The working distance affects the depth of field and the resolution of the image. Usually, the working distance is specified in millimeters (mm)."@en ;
                                          rdfs:isDefinedBy <https://w3id.org/pmd/mo> ;
                                          rdfs:label "Arbeitsabstand"@de ,
                                                     "Working Distance"@en ;
                                          <http://www.w3.org/2004/02/skos/core#definition> "Der Abstand zwischen der Objektivlinse des Elektronenmikroskops und der Probenoberfläche, wenn der Elektronenstrahl auf die Probe fokussiert wird."@de ,
                                                                                           "The distance between the electron microscope objective lens and the specimen surface when the electron beam is focused on the specimen."@en ;
                                          <https://w3id.org/pmd/co/definitionSource> "ChatGPT 3.5" .


###  https://w3id.org/pmd/mo/XRayAbsorptionNearEdgeSpectroscopy
<https://w3id.org/pmd/mo/XRayAbsorptionNearEdgeSpectroscopy> rdf:type owl:Class ;
                                                             rdfs:subClassOf <https://w3id.org/pmd/mo/Spectroscopy> ;
                                                             rdfs:isDefinedBy <https://w3id.org/pmd/mo> ;
                                                             rdfs:label "Röntgenabsorptionsspektroskopie im Nahbereich"@de ,
                                                                        "X-ray Absorption Near Edge Spectroscopy"@en ;
                                                             <http://www.w3.org/2004/02/skos/core#definition> """X-ray Absorption Near Edge Spectroscopy (XANES) is a specialized technique used in the field of materials science and spectroscopy to study the electronic and structural properties of materials. It focuses on the X-ray absorption spectra of atoms within a sample, particularly the region just above the absorption edge of an element's X-ray absorption spectrum.
In XANES, a sample is irradiated with X-rays, typically generated by a synchrotron radiation source. These X-rays are tuned to specific energy levels corresponding to the absorption edges of the elements of interest in the sample. As the X-rays are absorbed by the sample, the energy levels of the atoms are altered, leading to various transitions in their electron configurations. The resulting X-ray absorption spectrum is measured, specifically targeting the energies just above the absorption edge.
XANES provides information about the electronic structure of the atoms within the sample, including the oxidation state, chemical bonding, and local environment of the absorbing element. The fine details of the XANES spectrum offer insights into the atomic and molecular interactions, as well as the coordination and symmetry of atoms in different chemical environments.
This technique is widely used in various scientific fields, including chemistry, solid-state physics, and materials science. XANES helps researchers understand the properties and behavior of materials at the atomic level, making it an invaluable tool for investigating the characteristics of complex materials, catalysts, minerals, and biomolecules."""@en ;
                                                             <https://w3id.org/pmd/co/definitionSource> "ChatGPT 3.5"@en ;
                                                             <https://w3id.org/pmd/mo/abbreviation> "XANES"@en .


###  https://w3id.org/pmd/mo/XRayAbsorptionSpectroscopy
<https://w3id.org/pmd/mo/XRayAbsorptionSpectroscopy> rdf:type owl:Class ;
                                                     rdfs:subClassOf <https://w3id.org/pmd/mo/XRayMapping> ;
                                                     rdfs:isDefinedBy <https://w3id.org/pmd/mo> ;
                                                     rdfs:label "Röntgenabsorptionsspektroskopie"@de ,
                                                                "X-ray Absorption Spectroscopy"@en ;
                                                     <http://www.w3.org/2004/02/skos/core#definition> "X-ray Absorption Spectroscopy is a technique used to study the electronic and local structural properties of materials by analyzing the absorption of X-rays. It involves measuring how X-rays are absorbed by a sample at various energies, providing insights into the electronic states and chemical environments of specific elements."@en ;
                                                     <https://w3id.org/pmd/co/definitionSource> "ChatGPT 3.5"@en ;
                                                     <https://w3id.org/pmd/mo/abbreviation> "XAS"@en .


###  https://w3id.org/pmd/mo/XRayAnalysis
<https://w3id.org/pmd/mo/XRayAnalysis> rdf:type owl:Class ;
                                       rdfs:subClassOf <https://w3id.org/pmd/co/AnalysingProcess> ;
                                       rdfs:isDefinedBy <https://w3id.org/pmd/mo> ;
                                       rdfs:label "Röntgenanalyse"@de ,
                                                  "X-ray Analysis"@en ;
                                       <http://www.w3.org/2004/02/skos/core#definition> "X-ray analysis is a technique used to investigate the composition and structure of materials by exposing them to X-rays. When X-rays interact with a material, they can be absorbed, scattered, or diffracted in ways that provide information about the material's internal arrangement of atoms and its elemental composition."@en ;
                                       <https://w3id.org/pmd/co/definitionSource> "ChatGPT 3.5"@en .


###  https://w3id.org/pmd/mo/XRayDiffraction
<https://w3id.org/pmd/mo/XRayDiffraction> rdf:type owl:Class ;
                                          rdfs:subClassOf <https://w3id.org/pmd/mo/Diffraction> ;
                                          rdfs:isDefinedBy <https://w3id.org/pmd/mo> ;
                                          rdfs:label "X-ray Diffraction"@en ;
                                          <http://www.w3.org/2004/02/skos/core#altLabel> "Röntgenstrahlbeugung"@de ;
                                          <http://www.w3.org/2004/02/skos/core#definition> "X-ray Diffraction is a technique that utilizes the diffraction of X-rays by crystals to determine their atomic arrangement and lattice structure. X-ray diffraction patterns are produced when X-rays strike a crystalline sample, and the resulting pattern provides information about the arrangement of atoms in the crystal lattice."@en ;
                                          <http://www.w3.org/2004/02/skos/core#prefLabel> "Röntgenbeugung"@de ;
                                          <https://w3id.org/pmd/co/definitionSource> "ChatGPT 3.5"@en ;
                                          <https://w3id.org/pmd/mo/abbreviation> "XRD"@en .


###  https://w3id.org/pmd/mo/XRayFluorescence
<https://w3id.org/pmd/mo/XRayFluorescence> rdf:type owl:Class ;
                                           rdfs:subClassOf <https://w3id.org/pmd/mo/XRayMapping> ;
                                           rdfs:isDefinedBy <https://w3id.org/pmd/mo> ;
                                           rdfs:label "Röntgenfluoreszenz"@de ,
                                                      "X-ray Fluorescence"@en ;
                                           <http://www.w3.org/2004/02/skos/core#definition> "X-ray Fluorescence is a method used to determine the elemental composition of a sample by analyzing the X-rays emitted when the sample is exposed to high-energy X-rays. The X-rays emitted are characteristic of the elements present, allowing for quantitative analysis of the sample's elemental composition."@en ;
                                           <https://w3id.org/pmd/co/definitionSource> "ChatGPT 3.5"@en ;
                                           <https://w3id.org/pmd/mo/abbreviation> "XRF"@en .


###  https://w3id.org/pmd/mo/XRayMapping
<https://w3id.org/pmd/mo/XRayMapping> rdf:type owl:Class ;
                                      rdfs:subClassOf <https://w3id.org/pmd/mo/XRayAnalysis> ;
                                      rdfs:isDefinedBy <https://w3id.org/pmd/mo> ;
                                      rdfs:label "Röntgen-Mapping"@de ,
                                                 "X-ray Mapping"@en ;
                                      <http://www.w3.org/2004/02/skos/core#definition> "X-ray mapping is a process that involves generating spatially resolved images of the distribution of specific elements within a sample. By collecting X-ray signals emitted or scattered from a sample at different points, an elemental map can be created, showing the varying concentrations of elements across the sample's surface."@en ;
                                      <https://w3id.org/pmd/co/definitionSource> "ChatGPT 3.5"@en .


###  https://w3id.org/pmd/mo/XRayMicroanalysis
<https://w3id.org/pmd/mo/XRayMicroanalysis> rdf:type owl:Class ;
                                            rdfs:subClassOf <https://w3id.org/pmd/mo/XRayAnalysis> ;
                                            rdfs:isDefinedBy <https://w3id.org/pmd/mo> ;
                                            rdfs:label "Röntgen-Mikroanalyse"@de ,
                                                       "X-ray Microanalysis"@en ;
                                            <http://www.w3.org/2004/02/skos/core#definition> "X-ray Microanalysis is a technique that combines microscopy and X-ray analysis to study the elemental composition of small regions within a sample. It involves focusing an electron or X-ray beam on a specific area of the sample and measuring the X-rays emitted from that area to determine the elemental composition."@en ;
                                            <https://w3id.org/pmd/co/definitionSource> "ChatGPT 3.5"@en .


###  https://w3id.org/pmd/mo/XRayPhotoelectronSpectroscopy
<https://w3id.org/pmd/mo/XRayPhotoelectronSpectroscopy> rdf:type owl:Class ;
                                                        rdfs:subClassOf <https://w3id.org/pmd/mo/XRayMapping> ;
                                                        rdfs:isDefinedBy <https://w3id.org/pmd/mo> ;
                                                        rdfs:label "Röntgenphotoelektronenspektroskopie"@de ,
                                                                   "X-ray Photoelectron Spectroscopy"@en ;
                                                        <http://www.w3.org/2004/02/skos/core#definition> "X-ray Photoelectron Spectroscopy, also known as Electron Spectroscopy for Chemical Analysis (ESCA), is a technique used to study the surface chemistry of materials. XPS involves bombarding a sample's surface with X-rays to emit photoelectrons, which are then analyzed to determine the elemental composition and chemical states of the elements on the surface."@en ;
                                                        <https://w3id.org/pmd/co/definitionSource> "ChatGPT 3.5"@en ;
                                                        <https://w3id.org/pmd/mo/abbreviation> "XPS"@en .


###  https://w3id.org/pmd/mo/XrayEnergyDispersiveSpectrometer
<https://w3id.org/pmd/mo/XrayEnergyDispersiveSpectrometer> rdf:type owl:Class ;
                                                           owl:equivalentClass [ rdf:type owl:Restriction ;
                                                                                 owl:onProperty <https://w3id.org/pmd/co/hasFunction> ;
                                                                                 owl:someValuesFrom <https://w3id.org/pmd/mo/EnergyFilter>
                                                                               ] ,
                                                                               [ rdf:type owl:Restriction ;
                                                                                 owl:onProperty <https://w3id.org/pmd/co/hasFunction> ;
                                                                                 owl:someValuesFrom <https://w3id.org/pmd/mo/ImageFilter>
                                                                               ] ;
                                                           rdfs:subClassOf <https://w3id.org/pmd/mo/Spectrometer> ;
                                                           <http://purl.obolibrary.org/obo/IAO_0000117> "PMDco Team"@en ;
                                                           <http://purl.obolibrary.org/obo/IAO_0000119> "ChatGPT 3.5"@en ;
                                                           rdfs:label "Röntgen-Energie-dispersiver Spektrometer"@de ,
                                                                      "X-ray Energy Dispersive Spectrometer"@en ;
                                                           <http://www.w3.org/2004/02/skos/core#definition> "An X-ray Energy Dispersive Spectrometer is a device used in electron microscopes to analyze the elemental composition of samples by detecting X-rays emitted from the sample."@en ,
                                                                                                            "Ein Röntgen-Energie-dispersiver Spektrometer ist ein Gerät, das in Elektronenmikroskopen verwendet wird, um die Elementzusammensetzung von Proben durch Detektion der vom Probenmaterial emittierten Röntgenstrahlen zu analysieren."@de .


###  https://w3id.org/pmd/mo/3DCoordinates
<https://w3id.org/pmd/mo/3DCoordinates> rdf:type owl:Class ;
                                        rdfs:subClassOf <https://w3id.org/pmd/co/Coordinates> ;
                                        rdfs:isDefinedBy <https://w3id.org/pmd/mo> ;
                                        rdfs:label "3D Coordinates"@en ,
                                                   "3D-Koordinaten"@de ;
                                        <http://www.w3.org/2004/02/skos/core#definition> "Coordinates that specify a point in three-dimensional space."@en ,
                                                                                         "Koordinaten, die einen Punkt im dreidimensionalen Raum spezifizieren."@de ;
                                        <https://w3id.org/pmd/co/definitionSource> "ChatGPT 3.5"@en .


###  https://w3id.org/pmd/mo/3DReconstruction
<https://w3id.org/pmd/mo/3DReconstruction> rdf:type owl:Class ;
                                           rdfs:subClassOf <https://w3id.org/pmd/mo/Reconstruction> ;
                                           rdfs:isDefinedBy <https://w3id.org/pmd/mo> ;
                                           rdfs:label "Dreidimensionale Rekonstruktion"@de ,
                                                      "Three dimensional reconstruction"@en ;
                                           <http://www.w3.org/2004/02/skos/core#definition> "Der Prozess der Erstellung einer dreidimensionalen Darstellung eines Objekts oder einer Szene aus zweidimensionalen Bildern oder Daten."@de ,
                                                                                            "The process of creating a three-dimensional representation of an object or scene from two-dimensional images or data."@en ;
                                           <https://w3id.org/pmd/co/definitionSource> "ChatGPT 3.5"@en .


###  https://w3id.org/pmd/mo/3DXCoordinate
<https://w3id.org/pmd/mo/3DXCoordinate> rdf:type owl:Class ;
                                        rdfs:subClassOf <https://w3id.org/pmd/mo/3DCoordinates> ;
                                        rdfs:isDefinedBy <https://w3id.org/pmd/mo> ;
                                        rdfs:label "3D X Coordinate"@en ,
                                                   "3D X-Koordinate"@de ;
                                        <http://www.w3.org/2004/02/skos/core#definition> "Die X-Koordinate in einem dreidimensionalen Koordinatensystem."@de ,
                                                                                         "The X-coordinate in a three-dimensional coordinate system."@en ;
                                        <https://w3id.org/pmd/co/definitionSource> "ChatGPT 3.5"@en .


###  https://w3id.org/pmd/mo/3DYCoordinate
<https://w3id.org/pmd/mo/3DYCoordinate> rdf:type owl:Class ;
                                        rdfs:subClassOf <https://w3id.org/pmd/mo/3DCoordinates> ;
                                        rdfs:isDefinedBy <https://w3id.org/pmd/mo> ;
                                        rdfs:label "3D Y Coordinate"@en ,
                                                   "3D Y-Koordinate"@de ;
                                        <http://www.w3.org/2004/02/skos/core#definition> "Die Y-Koordinate in einem dreidimensionalen Koordinatensystem."@de ,
                                                                                         "The Y-coordinate in a three-dimensional coordinate system."@en ;
                                        <https://w3id.org/pmd/co/definitionSource> "ChatGPT 3.5"@en .


###  https://w3id.org/pmd/mo/3DZCoordinate
<https://w3id.org/pmd/mo/3DZCoordinate> rdf:type owl:Class ;
                                        rdfs:subClassOf <https://w3id.org/pmd/mo/3DCoordinates> ;
                                        rdfs:isDefinedBy <https://w3id.org/pmd/mo> ;
                                        rdfs:label "3D Z Coordinate"@en ,
                                                   "3D Z-Koordinate"@de ;
                                        <http://www.w3.org/2004/02/skos/core#definition> "Die Z-Koordinate in einem dreidimensionalen Koordinatensystem."@de ,
                                                                                         "The Z-coordinate in a three-dimensional coordinate system."@en ;
                                        <https://w3id.org/pmd/co/definitionSource> "ChatGPT 3.5"@en .


###  https://w3id.org/pmd/mo/4D-ScanningTransmissionElectronMicroscopy
<https://w3id.org/pmd/mo/4D-ScanningTransmissionElectronMicroscopy> rdf:type owl:Class ;
                                                                    rdfs:subClassOf <https://w3id.org/pmd/mo/ScanningTransmissionElectronMicroscopy> ;
                                                                    rdfs:isDefinedBy <https://w3id.org/pmd/mo> ;
                                                                    rdfs:label "4D Scanning Transmission Electron Microscopy"@en ,
                                                                               "4D-Rastertransmissionselektronenmikroskopie"@de ;
                                                                    <http://www.w3.org/2004/02/skos/core#definition> "4D-STEM is a technique that adds an additional dimension of information, time, to STEM imaging, allowing the study of dynamic processes in materials at high spatial and temporal resolutions."@en ;
                                                                    <https://w3id.org/pmd/co/definitionSource> "ChatGPT 3.5"@en ;
                                                                    <https://w3id.org/pmd/mo/abbreviation> "4D-STEM"@en .


###  Generated by the OWL API (version 5.1.18) https://github.com/owlcs/owlapi/
